<?xml version="1.0" encoding="UTF-8" ?>

<!-- Copyright 2018 Joel Feldman, Andrew Rechnitzer and Elyse Yeager -->
<!-- This work is licensed under the Creative Commons Attribution-NonCommercial-ShareAlike 4.0 International License-->
<!-- https://creativecommons.org/licenses/by-nc-sa/4.0 -->

<exercises>
<exercisegroup> <introduction><application/></introduction>

<exercise><title><fromexam>M317 2010A</fromexam></title>
<statement><p>
Let <m>\vr(t) = x(t)\,\hi + y (t)\,\hj + z(t)\,\hk</m> be the position
of a particle at time <m>t</m> . Suppose the motion of the particle satisfies
the differential equation
<m>\difftwo{\vr}{t} = f (r) \vr</m>
where <m>r = |\vr|</m> .
<ol marker="a">
<li><p>
Suppose <m>f(r)</m> is an arbitrary function of <m>r</m> . Prove or disprove each
of the following statements.
<ol marker="(i)">
<li>
The motion of the particle is planar.
</li>
<li>
The path of the particle sweeps out equal areas in equal times.
</li>
</ol></p>
</li>
<li>
Find all forms of <m>f(r)</m> for which the motion of the particle always lies
on a straight line.
</li>
<li>
Give a specific form of <m>f(r)</m> for which the motion of the particle could
lie on an ellipse.
</li>
</ol>
</p></statement>

<hint><p>
(a) Review ยง<xref ref="sec_central_forces"/>.
</p>

<p>(b) Any straight line can be parametrized as <m>\vr(s) = \vr_0+\hat\vT\, s</m>.
</p>

<p>(c) Review ยง<xref ref="sec_planet"/>.
</p></hint>

<answer><p>
(a) See the solutions.
</p>

<p>(b) <m>f(r)=0</m> for all <m>r\ge 0</m>.
</p>

<p>(c) Any <m>f(r)</m> which is a positive constant times <m>-\frac{1}{r^3}</m> works.
</p></answer>

<solution><p> (a)
Both (i) and (ii) were proven in ยง<xref ref="sec_central_forces"/>. Here are those arguments.
</p>

<p>Define
<me>
\vOm(t) = \vr(t)\times\vv(t)
</me>
By the product rule,
<md>
<mrow>
\diff{\vOm}{t}(t) &amp;=\diff{\ }{t}\big(\vr(t)\times\vv(t)\big)
=\vv(t)\times\vv(t) + \vr(t)\times\va(t)
</mrow><mrow>
&amp;=m\vr(t)\times f\big(r(t))\vr(t)\big)
=\vZero
</mrow>
</md>
So <m>\vOm(t)</m> is in fact independent of <m>t</m>. It is a constant vector that
we'll just denote <m>\vOm</m>.
</p>

<p>As <m>\vr(t)\times\vv(t)=\vOm</m>, we have that
<m>\vr(t)</m> is always perpendicular to <m>\vOm</m> and
<me>
\vr(t)\cdot\vOm =0
</me>
<ul>
<li>
If <m>\vOm\ne \vZero</m>, this is exactly the statement that <m>\vr(t)</m> always
lies in the plane through the origin with normal vector <m>\vOm</m>.
</li>
<li>
If <m>\vOm=\vZero</m>, then <m>\vr(t)</m> is always parallel to <m>\vv(t)</m> and there
is some function <m>\alpha(t)</m> such that
<me>
\diff{\vr}{t}(t) = \vv(t) = \alpha(t)\,\vr(t)
</me>
This is a first order, linear, ordinary differential equation that we can solve
by using an integrating factor. Set
<me>
\beta(t) = \int_0^t\alpha(t)\ \dee{t}
</me>
Then
<md>
<mrow>
\diff{\vr}{t}(t) = \alpha(t)\,\vr(t)
&amp;\iff e^{-\beta(t)} \diff{\vr}{t}(t) -\alpha(t)e^{-\beta(t)}\,\vr(t)=0
</mrow><mrow>
&amp;\iff \diff{\ }{t}\big[e^{-\beta(t)}\vr(t)\big] = 0
</mrow><mrow>
&amp;\iff e^{-\beta(t)}\vr(t) = \vr(0)
</mrow><mrow>
&amp;\iff \vr(t) =  e^{\beta(t)}\vr(0)
</mrow>
</md>
so that <m>\vr(t)</m> lies on a line through the origin. This makes sense <mdash/>
the particle is always moving parallel to its radius vector.
</li>
</ul>
This completes the verification that <m>\vr(t)</m> lies in a plane.
</p>

<p>Now we show that the radius vector <m>\vr(t)</m> sweeps out equal areas in
equal times. In other words, we now verify that the rate at which
<m>\vr(t)</m> sweeps out area is independent of time. To do so we rewrite the
statement that <m>|\vr(t)\times\vv(t)\big|</m> is constant in polar coordinates.
Writing <m>\vr(t) = r(t)\hat\vr\big(\theta(t)\big)</m> and then applying
Lemma <xref ref="lem_polar"/>.b gives that
<md>
<mrow>
&amp;\text{constant} = \big|\vr\times\vv\big|
   = \Big|r\hat\vr\times\Big(\diff{r}{t}\ \hat\vr
             + r\ \diff{\theta}{t}\ \hat\vth\Big)\Big|
   =r^2\diff{\theta}{t}
</mrow><mrow>
&amp;\text{since}\quad |\hat\vr\times\hat\vr|=0,\
                        |\hat\vr\times\hat\vth|=1
</mrow>
</md>
is constant. It now suffices to observe that <m>r(t)^2\diff{\theta}{t}(t)</m>
is exactly twice the rate at which <m>\vr(t)</m> sweeps out area. To see this,
just look at the figure below. The shaded area is essentially a wedge of
a circular disk of radius <m>r</m>. (If <m>r(t)</m> were independent of <m>t</m>, it would be exactly a wedge of a circular disk.) Its area is the
fraction <m>\frac{\dee{\theta}}{2\pi}</m> of the area of the full disk, which is
</p>

<sidebyside widths="30% 30%" valign="middle">
  <p>
  <me>
  \frac{\dee{\theta}}{2\pi}\ \pi r^2 = \frac{1}{2}r^2\,\dee{\theta}
  </me>
  </p>
  <image source="pfigs/equalArea"/>
</sidebyside>

<p> (b) If <m>f(r)</m> is identically zero, then <m>\vr''(t)=0</m>,
so that <m>\vr'(t)</m> is a constant, say <m>\vv_0</m>, and <m>\vr(t) = \vr_0 + \vv_0 t</m>,
for some constant <m>\vr_0</m>. That's a straight line.
</p>

<p>We'll now show that if the motion of the particle always lies
on a straight line, then <m>f(r)</m> must be identically zero.
Suppose that <m>\vr(t)</m> is a straight line. Then there are
constant vectors <m>\vr_0</m> and <m>\hat\vT</m> such that <m>\vr(t) =\vr_0+ g(t)\hat\vT</m>
for some scalar valued function <m>g(t)</m>. Then
<md>
<mrow>
\vr''(t) &amp;= f\big(r(t)\big)\vr(t)
</mrow>
</md>
becomes
<md>
<mrow>
g''(t)\hat\vT &amp; = f\big(r(t)\big)\,\big[\vr_0+ g(t)\hat\vT\big]
              = f\big(r(t)\big)\,\vr_0
               + f\big(r(t)\big) g(t)\hat\vT
</mrow>
</md>
We may always choose the initial conditions so that, for example,
<m>\vr_0=\hi</m> and <m>\hat\vT=\hj</m>.  So
<md>
<mrow>
g''(t)\hj &amp;   = f\big(r(t)\big)\,\hi
               + f\big(r(t)\big) g(t)\hj
</mrow>
</md>
Taking the dot product of both sides with <m>\hi</m> gives
<m>f\big(r(t)\big)=0</m>, as desired.
</p>

<p> (c) We saw in ยง<xref ref="sec_planet"/>
that the gravitational force <m>-\frac{GMm}{r^3}\vr</m> can produce
elliptical orbits.
So any <m>f(r)</m> which is a positive constant times <m>-\frac{1}{r^3}</m> does
the job.
</p>

</solution>
</exercise>

<exercise><title><fromexam>M317 2000A</fromexam></title>
<statement><p>
An object moves along a curve in the <m>xy</m>-plane having polar
equation <m>r=\frac{1}{\theta+\al}</m> (where <m>\al</m> is a constant) under the influence
of a central force so that the object has no transverse acceleration.
<ol marker="a">
<li>
Verify that <m>r^2\dot\theta=h</m> remains constant as the object
moves.
</li>
<li>
Express the magnitude of the acceleration of the object as
a function of <m>r</m> and <m>h</m>.
</li>
</ol>
</p>

</statement>

<hint><p>
(a) For any central force <m>\big|\vr(t)\times\vv(t)\big|</m> is independent of <m>t</m>.
</p>

<p>(b) Review Lemma <xref ref="lem_polar"/>.
</p></hint>

<answer><p>
(a) See the solution.
</p>

<p>(b) <m>|\va(t)| =\frac{h^2}{r(t)^3}</m>
</p></answer>

<solution><p>
(a)
Our object is subject to a central force. So the acceleration <m>\va(t)</m>
is parallel to <m>\vr(t)</m> and
<me>
\diff{\ }{t}\big(\vr(t)\times\vv(t)\big)
=\vv(t)\times\vv(t) + \vr(t)\times\va(t)
=\vZero +\vZero
=\vZero
</me>
By Lemma <xref ref="lem_polar"/>,
<m>\vv(t) = \diff{r}{t}(t)\ \hat\vr\big(\theta(t)\big)
             + r(t)\ \diff{\theta}{t}(t)\ \hat\vth\big(\theta(t)\big)</m>.
Because <m>\vr(t)=r(t)\hat\vr\big(\theta(t)\big)</m> is parallel to
<m>\hat\vr\big(\theta(t)\big)</m> and is perpendicular to
<m>\hat\vth\big(\theta(t)\big)</m>,
<me>
\vr(t)\times\vv(t)
=r(t)^2\dot\theta(t)\,\hat\vr\big(\theta(t)\big)\times
                       \hat\vth\big(\theta(t)\big)
</me>
and, in particular,
<me>
|\vr(t)\times\vv(t)| = r(t)^2|\dot\theta(t)|
</me>
is a constant. As <m>\dot\theta(t)</m> is continuous, <m>r(t)^2\dot\theta(t)</m>
is also constant.
</p>

<p>(b)
By Lemma <xref ref="lem_polar"/>,
the acceleration
<md>
<mrow>
\va(t) &amp;= \Big(\difftwo{r}{t}(t)-r(t)\Big(\diff{\theta}{t}(t)\Big)^2\Big)
             \hat\vr\big(\theta(t)\big)
</mrow><mrow>
&amp;\hskip1in   +\Big(r(t)\ \difftwo{\theta}{t}(t)
          + 2 \diff{r}{t}(t)\diff{\theta}{t}(t)\Big)
                  \hat\vth\big(\theta(t)\big)
</mrow>
</md>
Because our object is subject to a central force, the acceleration
<m>\va(t)</m> is parallel to <m>\hat\vr\big(\theta(t)\big)</m>. So the
<m>\hat\vth\big(\theta(t)\big)</m> component of the acceleration is zero
and
<me>
\va(t) = \Big(\difftwo{r}{t}(t)-r(t)\Big(\diff{\theta}{t}(t)\Big)^2\Big)
             \hat\vr\big(\theta(t)\big)
</me>
so that
<me>
|\va(t)| = \Big|\difftwo{r}{t}(t)-r(t)\Big(\diff{\theta}{t}(t)\Big)^2\Big|
</me>
Since <m>r(t)=\frac{1}{\theta(t)+\al}</m>
<md>
<mrow>
\dot r(t) = - \frac{1}{[\theta(t)+\al]^2}\dot\theta(t)
          =- r(t)^2 \dot\theta(t) =-h
</mrow>
</md>
So <m>\difftwo{r}{t}(t)=0</m> and
<md>
<mrow>
|\va(t)| = r(t)\dot\theta(t)^2
=\frac{r(t)^4\dot\theta(t)^2}{r(t)^3}
=\frac{h^2}{r(t)^3}
</mrow>
</md>
</p>

</solution>
</exercise></exercisegroup>

</exercises>
