<?xml version="1.0" encoding="UTF-8" ?>
<!-- Copyright 2018-2020 Joel Feldman, Andrew Rechnitzer and Elyse Yeager -->
<!-- This work is licensed under the Creative Commons Attribution-NonCommercial-ShareAlike 4.0 International License-->
<!-- https://creativecommons.org/licenses/by-nc-sa/4.0 -->

<section xml:id="ap_ODE">
  <title>Review of Linear Ordinary Differential Equations</title>

<definition xml:id="def_apODE">
<statement><p>
<ol label="a">
<li>
A <term>differential equation</term> is an equation for an
unknown function that contains the derivatives of that unknown function.
For example <m>y''(t)+y(t)=0</m> is a differential equation for the unknown
function <m>y(t)</m>.
</li>
<li>
A differential equation is called an <term>ordinary differential
equation</term> (often shortened to <q>ODE</q>) if only ordinary derivatives
appear. That is, if the unknown function has only a single independent
variable. A differential equation is called a <term>partial differential
equation</term> (often shortened to <q>PDE</q>) if partial derivatives
appear. That is, if the unknown function has more than one independent
variable. For example <m>y''(t)+y(t)=0</m> is an ODE while
<m>\frac{\partial^2 u}{\partial\, t^2}(x,t)=c^2
\frac{\partial^2 u}{\partial\, x^2}(x,t)</m> is a PDE.
</li>
<li>
The <term>order</term> of a differential equation is the order of the
highest derivative that appears. For example <m>y''(t)+y(t)=0</m>
is a second order ODE.
</li>
<li><p>
An ordinary differential equation that is of the form
<men xml:id="eqn_ODEordern">
a_0(t) y^{(n)}(t) + a_1(t) y^{(n-1)}(t)+\cdots +a_n(t)y(t)
=F(t)
</men>
with given coefficient functions <m>a_0(t)</m>, <m>\cdots</m>, <m>a_n(t)</m> and <m>F(t)</m>
is said to be <term>linear</term>. Otherwise, the ODE is said to be <term>nonlinear</term>.
For example, <m>y'(t)^2+y(t)=0</m>, <m>y'(t)y''(t)+y(t)=0</m> and <m>y'(t)=e^{y(t)}</m>
are all nonlinear.
</p></li>
<li>
The ODE <xref ref="eqn_ODEordern"/> is said to have <term>constant coefficients</term> if
the coefficients  <m>a_0(t)</m>, <m>a_1(t)</m>, <m>\cdots</m>, <m>a_n(t)</m> are all constants. Otherwise,
it is said to have <term>variable coefficients</term>. For example,
the ODE <m>y''(t)+7y(t)=\sin t</m> is constant coefficient, while
<m>y''(t)+ty(t)=\sin t</m> is variable coefficient.
</li>
<li>
The ODE <xref ref="eqn_ODEordern"/> is said to be <term>homogeneous</term> if <m>F(t)</m>
is identically zero. Otherwise, it is said to be <term>inhomogeneous</term> or
<term>nonhomogeneous</term>. For example, the ODE <m>y''(t)+7y(t)=0</m> is homogeneous,
while  <m>y''(t)+7y(t)=\sin t</m> is inhomogeneous. A homogeneous ODE always
has the trivial solution <m>y(t)=0</m>.
</li>
<li>
An <term>initial value problem</term>  is a problem in which one is to find
an unknown function <m>y(t)</m> that satisfies both a given ODE and given
initial conditions, like <m>y(t_0)=1</m>, <m>y'(t_0)=0</m>. Note that all of the 
conditions involve the function <m>y(t)</m> (or its derivatives) evaluated at 
a single time <m>t=t_0</m>.
</li> 
<li>
A <term>boundary value problem</term>  is a problem in which one is to find
an unknown function <m>y(t)</m> that satisfies both a given ODE and given
boundary conditions, like <m>y(t_0)=0</m>, <m>y(t_1)=0</m>. Note that the conditions 
involve the function <m>y(t)</m> (or its derivatives) evaluated at two different 
times. 

</li>
</ol>
</p></statement>
</definition>


<p>The following theorem gives the form of solutions to the ODE <xref ref="eqn_ODEordern"/>.
</p>

<theorem xml:id="thm_odeMain">
<statement><p>
Assume that the coefficients <m>a_0(t)</m>, <m>a_1(t)</m>, <m>\cdots</m>, <m>a_{n-1}(t)</m>,
<m>a_n(t)</m> and <m>F(t)</m> are continuous functions and that
<m>a_0(t)</m> is not zero.
<ol label="a">
<li><p>
The general solution to the ODE <xref ref="eqn_ODEordern"/> is of the form
<men xml:id="eqn_ODEgensln">
y(t)=y_p(t)+ C_1y_1(t)+C_2y_2(t)+\cdots+C_n y_n(t)
</men>
where
<ul>
<li> <m>n</m> is the order of <xref ref="eqn_ODEordern"/>
</li>
<li> <m>y_p(t)</m> is any solution to <xref ref="eqn_ODEordern"/>
</li>
<li> <m>C_1</m>, <m>C_2</m>, <m>\cdots</m>, <m>C_n</m> are arbitrary constants
</li>
<li> <m>y_1</m>, <m>y_2</m>, <m>\cdots</m>, <m>y_n</m> are <m>n</m> independent solutions
to the homogenous equation
<me>
a_0(t) y^{(n)}(t) + a_1(t) y^{(n-1)}(t)+\cdots+a_{n-1}(t) y'(t) +a_n(t)y(t)=0
</me>
associated to <xref ref="eqn_ODEordern"/>.
<q>Independent</q> just means that no <m>y_i</m> can be written as a linear combination
of the other <m>y_j</m>'s. For example, <m>y_1(t)</m> cannot be expressed in the form
<m>b_2y_2(t)+\cdots+b_ny_n(t)</m>.
</li>
</ul>
In <xref ref="eqn_ODEgensln"/>, <m>y_p</m> is called the <q>particular solution</q> and
<m>C_1y_1(t)+C_2y_2(t)+\cdots+C_n y_n(t)</m> is called the
<q>complementary solution</q>.
</p></li>
<li>
Given any constants <m>b_0</m>, <m>\cdots</m>, <m>b_{n-1}</m> there is exactly
one function <m>y(t)</m> that obeys the ODE <xref ref="eqn_ODEordern"/> and the initial
conditions
<me>
y(0)=b_0\qquad y'(0)=b_1\qquad \cdots\qquad y^{(n-1)}(0)=b_{n-1}
</me>
</li>
</ol>
</p></statement>
</theorem>


<example xml:id="eg_RLC"><title>RLC circuit</title>
<p>
As an example of the most commonly used techniques for solving linear,
constant coefficient ODE's, we consider the RLC circuit, which is
the electrical circuit consisting of a resistor of
resistance <m>R</m>, a coil (or solenoid) of inductance <m>L</m>, a capacitor
of capacitance <m>C</m> and a voltage source arranged in series, as shown below.
Here <m>R</m>, <m>L</m> and <m>C</m> are all nonnegative constants.
</p>

<sidebyside width="50%">
<image source="figs/RLC"/>
</sidebyside>

<p>
 We're going to think of the voltage <m>x(t)</m> as an input signal,
and the voltage <m>y(t)</m> as an output signal.
The goal is to determine the output signal produced by a given input signal.
If <m>i(t)</m> is the current flowing at time <m>t</m> in the loop as shown and
<m>q(t)</m> is the charge on the capacitor, then the voltages across <m>R</m>, <m>L</m>
and <m>C</m>, respectively, at time <m>t</m> are
<m>Ri(t)</m>, <m>L\diff{i}{t}(t)</m> and <m>y(t)=\frac{q(t)}{C}</m>. By the Kirchhoff's
law<fn>Gustav Robert Kirchhoff (1824--1887) was a German physicist.</fn>
that says that the voltage between any two points has to be independent
of the path used to travel between the two points, these three voltages
must add up to <m>x(t)</m> so that
<men xml:id="eqn_RLCrlc">
Ri(t) + L\diff{i}{t}(t) + \frac{q(t)}{C} = x(t)
</men>
Assuming that <m>R,\ L,\ C</m> and <m>x(t)</m> are known, this is still one
differential equation in two unknowns, <m>i(t)</m> and <m>q(t)</m>. Fortunately,
there is a relationship between the two. Namely
<men xml:id="eqn_RLCiq">
i(t)=\diff{q}{t}(t) = Cy'(t)
</men>
This just says that the capacitor cannot create or destroy charge on
its own; all charging of the capacitor must come from the current.
Substituting <xref ref="eqn_RLCiq"/> into <xref ref="eqn_RLCrlc"/> gives
<me>
 LCy''(t) + RCy'(t) + y(t) = x(t)
</me>
As a concrete example, we'll take  an ac voltage source and choose the
origin of time so that <m>x(0)=0</m>, <m>x(t)=E_0\sin(\om t)</m>. Then the differential equation becomes
<men xml:id="eqn_ODERy">
LCy''(t)+RCy'(t)+y(t)=E_0\sin(\om t)
</men>
This is a second order, linear, constant coefficient ODE. So we know,
from Theorem <xref ref="thm_odeMain"/>, that the general solution is of the form
<m>y_p(t)+C_1y_1(t)+C_2y_2(t)</m>, where
<ul>
<li>
 <m>y_p(t)</m>, the particular solution, is any one solution
to  <xref ref="eqn_ODERy"/>,
</li>
<li>
<m>C_1,C_2</m> are arbitrary
constants and
</li>
<li>
<m>y_1(t)</m>, <m>y_2(t)</m> are any two independent solutions of the corresponding
homogeneous equation
<men xml:id="eqn_ODERyh">
LCy''(t)+RCy'(t)+y(t)=0
<!-- % \tag{<xref ref="eqn_ODERy"/> $ _{\rm h}$} -->
</men>
</li>
</ul>
So to find the general solution to <xref ref="eqn_ODERy"/>, we need to find
three functions: <m>y_1(t)</m>, <m>y_2(t)</m> and <m>y_p(t)</m>.
</p>


<p><ul>
<li><p>
<em>Finding <m>y_1(t)</m> and <m>y_2(t)</m>:</em>
The best way to find <m>y_1</m> and <m>y_2</m> is to guess them.
Any solution, <m>y_h(t)</m>, of <xref ref="eqn_ODERyh"/> has to have the property that <m>y_h(t)</m>,
<m>RCy_h'(t)</m> and <m>LCy_h''(t)</m> cancel each other out for all <m>t</m>. We choose our guess
so that <m>y_h(t)</m>, <m>y_h'(t)</m> and <m>y_h''(t)</m> are all proportional to a single
function of <m>t</m>. Then it will be easy to see if <m>y_h(t)</m>, <m>RCy_h'(t)</m> and
<m>LCy_h''(t)</m> all cancel. All derivatives of the function <m>e^{rt}</m> are again proportional to <m>e^{rt}</m>. Hence we try <m>y_h(t)=e^{rt}</m>, with the constant
<m>r</m> to the determined. This guess is a solution of <xref ref="eqn_ODERyh"/>
if and only if
<men xml:id="eqn_ODERroots">
\begin{split}
&amp;LCr^2e^{rt}+RCre^{rt}+e^{rt}=0
\iff LCr^2+RCr+1 =0 \\
&amp;\hskip0.5in\iff  r=\frac{-RC\pm\sqrt{R^2C^2-4LC}}{2LC}\equiv r_{1,2}
\end{split}
</men>
How we proceed depends on the sign of <m>R^2C^2-4LC</m>. That is, whether
<m>R \gt  2\sqrt{\frac{L}{C}}</m> or  <m>R \lt  2\sqrt{\frac{L}{C}}</m>
or <m>R = 2\sqrt{\frac{L}{C}}</m>.
</p>
<p>
<ul>
<li>
<em>Finding <m>y_1(t)</m> and <m>y_2(t)</m>, when <m>R \gt  2\sqrt{\frac{L}{C}}</m>:</em>
Then <m>R^2C^2-4LC \gt  0</m>, and <m>r_1</m> and <m>r_2</m> are two different real numbers.
We may take <m>y_1(t)=e^{r_1t}</m> and <m>y_2(t)=e^{r_2t}</m> so that
the complimentary solution is
<m>
C_1y_1(t)+C_2y_2(t)=C_1 e^{r_1t}+C_2e^{r_2 t}
</m>.
</li>
<li><p>
<em>Finding <m>y_1(t)</m> and <m>y_2(t)</m>, when <m>R \lt  2\sqrt{\frac{L}{C}}</m>:</em>
Then <m>R^2C^2-4LC \lt  0</m> and <m>r_1</m> and <m>r_2</m>
are the two different complex numbers <m>-\rho\pm i\nu</m>, where
<me>
\rho=\frac{R}{2L}\qquad\text{and}\qquad
 \nu=\frac{\sqrt{4LC-R^2C^2}}{2LC}
</me>
We may again take
<m>
C_1 e^{r_1t}+C_2e^{r_2 t}
</m>
as the complimentray solution.  However we can also rewrite
<m>C_1 e^{r_1t}+C_2e^{r_2 t}</m> in terms of real valued functions
by using that <m>e^{\pm i\theta}=\cos\theta\pm i\sin\theta</m>:
<md>
<mrow>
&amp;C_1 e^{r_1t}+C_2e^{r_2 t}
  =e^{-\rho t}\big[C_1e^{i\nu t}+C_2e^{-i\nu t}\big]
</mrow><mrow>
  &amp;\hskip0.5in=e^{-\rho t}\big[C_1\big\{\cos(\nu t)+i\sin(\nu t)\big\}+
               C_2\big\{\cos(\nu t)-i\sin(\nu t)\big\}\big]
</mrow><mrow>
  &amp;\hskip0.5in=e^{-\rho t}\big[D_1\cos(\nu t)+D_2\sin(\nu t)\big]
</mrow>
</md>
where<fn>Don't make the mistake of thinking that <m>C_1</m>
and <m>C_2</m> have to be real numbers, forcing <m>D_2</m> to be pure  imaginary.
In most applications, <m>D_1</m> and <m>D_2</m> will be pure real and <m>C_1</m> and
<m>C_2</m> will be complex.</fn>
 <m>D_1=C_1+C_2,\ D_2=i(C_1-C_2)</m>. So we may also take
<m>y_1(t)=e^{-\rho t}\cos(\nu t)</m>, <m>y_2(t)=e^{-\rho t}\sin(\nu t)</m> in
the complementary solution.
</p>

<p>There is yet a third useful way to write
the complementary solution.
Think of <m>(D_1,D_2)</m> as a point in the <m>xy</m>-plane. Call the polar
coordinates of that point <m>A</m> and <m>\theta</m> so that <m>D_1=A\cos\theta</m> and
<m>D_2=A\sin\theta</m>. Then, using the trig identity <m>\cos(\alpha+\beta)
=\cos \alpha\cos\beta-\sin \alpha\sin \beta</m>, with <m>\alpha=\nu t</m> and <m>\beta=-\theta</m>,
<men xml:id="eqn_RLCampPhase">
\begin{split}
&amp;e^{-\rho t}\big[D_1\cos(\nu t)+D_2\sin(\nu t)\big]\\
&amp;\hskip0.5in=e^{-\rho t}\big[A\cos(\nu t)\cos\theta+A\sin(\nu t)\sin\theta\big]\\
&amp;\hskip0.5in=Ae^{-\rho t}\cos(\nu t-\theta)
\end{split}
</men>
We have, in effect, replaced the two arbitrary constants <m>D_1</m> and <m>D_2</m>,
whose values would normally be determined by initial conditions, by two
other arbitrary constants, <m>R</m> and <m>\theta</m>, whose values would also normally
be determined by initial conditions.
</p>
</li>
<li>
<em>Finding <m>y_1(t)</m> and <m>y_2(t)</m>, when <m>R=2\sqrt{\frac{L}{C}}</m>:</em>
Then <m>R^2C^2-4LC=0</m> so that <m>r_1=r_2</m>. We may take
<m>y_1=e^{r_1t}</m>, but <m>e^{r_2t}=e^{r_1t}</m> is certainly not a second independent
solution. So we still need to find <m>y_2</m>.
Here is a trick (called reduction of order<fn>The modern method of reduction of order was created by the French mathematician, physicist
and music theorist Jean le Rond d'Alembert (1717-1783). The interested reader
can easily search out more about his life.</fn>) for finding
the other solutions:
look for solutions of the form  <m>v(t)e^{-r_1 t}</m>. Here <m>e^{-r_1 t}</m>
is the solution we have already found and <m>v(t)</m> is to be determined.
To save writing, set <m>\rho=\frac{R}{2L}</m> so that <m>r_1=r_2=\rho</m>.
To save writing also divide (<xref ref="eqn_ODERy"/><m>_{\rm h}</m>) by <m>LC</m> and
substitute that <m>\frac{R}{L}=2\rho</m> and
<m>\frac{1}{LC}=\frac{R^2}{4L^2}=\rho^2</m>.  (Recall that we are assuming
that <m>R^2=\frac{4L}{C}</m>.) So (<xref ref="eqn_ODERy"/><m>_{\rm h}</m>) is equivalent to
<me>
y_h''(t)+2\rho\,y_h'(t)+\rho^2\,y_h(t)=0
</me>
Substitute in
<md>
<mrow>
y_h(t)&amp;=\ \ \  v(t)e^{-\rho t}
</mrow><mrow>
y_h'(t)&amp;= -\rho v(t)e^{-\rho t}+\phantom{2\rho}v'(t)e^{-\rho t}
</mrow><mrow>
y_h''(t)&amp;= \phantom{-}\rho^2 v(t)e^{-\rho t}-2\rho v'(t)e^{-\rho t}
                  +v''(t)e^{-\rho t}
</mrow>
</md>
So when <m>y_h(t)=v(t)e^{-\rho t}</m>,
<md>
<mrow>
&amp;y_h''(t)+2\rho\,y_h'(t)+\rho^2\,y_h(t)
</mrow><mrow>
&amp;\hskip0.5in=\big[\rho^2\!-\!2\rho^2\!+\!\rho^2\big]v(t)e^{-\rho t}
       +\big[-2\rho\!+\!2\rho\big]v'(t)e^{-\rho t}+v''(t)e^{-\rho t}
</mrow><mrow>
&amp;\hskip0.5in=v''(t)e^{-\rho t}
</mrow>
</md>
Thus <m>v(t)e^{-\rho t}</m> is a solution of (<xref ref="eqn_ODERy"/><m>_{\rm h}</m>) whenever the function
<m>v''(t)=0</m> for all <m>t</m>. But, for any values of the constants <m>C_1</m> and <m>C_2</m>,
<m>v(t)=C_1+C_2t</m> has vanishing second derivative
so <m>\big(C_1+C_2t\big)e^{-\rho t}=\big(C_1+C_2t\big)e^{-r_1 t}</m> solves
(<xref ref="eqn_ODERy"/><m>_{\rm h}</m>). This is of the form  <m>C_1y_1(t)+C_2y_2(t)</m> with
<m>y_1(t)=e^{-r_1t}</m>, the solution that we found first, and <m>y_2(t)=te^{-r_1t}</m>,
a second independent solution. So we may take <m>y_2(t)=te^{r_1t}</m>.
</li>
</ul></p>
</li>
<li><p>
<em>Finding <m>y_p(t)</m>:</em>
The best way to find <m>y_p</m> is to guess it. We guess that the circuit
responds to an oscillating input voltage with an output voltage that oscillates
at the same frequency. So we try
<m>y_p(t)=\mathcal{A}\sin(\om t-\varphi)</m> with the amplitude <m>\mathcal{A}</m>
and phase <m>\varphi</m> to be determined.
</p>

<p>For <m>y_p(t)</m> to be a solution, we need
<md>
<mrow>
LCy_p''(t)+RCy_p'(t)+y_p(t)
   &amp;=E_0 \sin(\om t)
</mrow>
</md>
or
<md>
<mrow>
&amp;-LC\om^2\mathcal{A}\sin(\om t-\varphi)+RC\om \mathcal{A}\cos(\om t-\varphi)
+\mathcal{A}\sin(\om t-\varphi)
</mrow><mrow>&amp;\hskip2in=E_0 \sin(\om t)
</mrow><mrow>
&amp;\hskip2in=E_0 \sin(\om t-\varphi+\varphi)
</mrow>
</md>
and hence, applying <m>\sin(A+B)=\sin A\cos B+\cos A\sin B</m> with <m>A=\om
t-\varphi</m> and <m>B=\varphi</m>,
<md>
<mrow>
&amp;\big(1-LC\om^2\big)\mathcal{A}\sin(\om t-\varphi)+RC\om \mathcal{A}\cos(\om t-\varphi)
</mrow><mrow>&amp;\hskip1in
=E_0 \cos(\varphi)\sin(\om t-\varphi)
+ E_0 \sin(\varphi)\cos(\om t-\varphi)
</mrow>
</md>
Matching coefficients of <m>\sin(\om t-\varphi)</m> and <m>\cos(\om t-\varphi)</m> on
the left and right hand sides gives
<mdn>
<mrow xml:id="eqnODERnum">
\big(1-LC\om^2\big)\mathcal{A}&amp;= E_0 \cos(\varphi)
</mrow>
<mrow xml:id="eqnODERden">
RC\om \mathcal{A}&amp;=E_0 \sin(\varphi)
</mrow>
</mdn>
It is now easy to solve for <m>\mathcal{A}</m> and <m>\varphi</m>
<md alignment="alignat">
<mrow>
\frac{<xref ref="eqnODERden"/>}{<xref ref="eqnODERnum"/>}
&amp;\implies \tan(\varphi) = \frac{RC\om}{1-LC\om^2}
</mrow><mrow>
&amp;\implies \varphi = \arctan\frac{RC\om}{1-LC\om^2}
</mrow><mrow>
\sqrt{<xref ref="eqnODERnum"/>^2\!+<xref ref="eqnODERden"/>^2}
&amp;\implies\sqrt{\big(1\!-\!LC\om^2\big)^2+R^2C^2\om^2}\ \mathcal{A}= E_0
</mrow><mrow>
&amp;\implies \mathcal{A}=\frac{E_0}{\sqrt{(1\!-\!LC\om^2)^2+R^2C^2\om^2}}
</mrow>
</md>
</p>
</li>
</ul>
Naturally, different input frequencies <m>\om</m> give different output
amplitudes <m>\mathcal{A}</m>. Here is a graph of <m>\mathcal{A}</m> against <m>\om</m>,
with all other parameters held fixed.
</p>

<sidebyside width="50%">
<image source="figs/resonance"/>
</sidebyside>

<p>
Note that there is a small range of frequencies that give a large
amplitude response. This is the phenomenon of resonance. It is exploited
in the design of radio and television tuning circuitry. It has also been
dramatically illustrated in, for example, the collapse<fn>There are videos of the collapse on the web.</fn>
 of the Tacoma narrows bridge.
</p></example>

<example xml:id="exBVP"><title>Boundary Value Problems</title>
<p>
By part (b) of Theorem <xref ref="thm_odeMain"/>, an initial value problem consisting
of an <m>n^{\rm th}</m> order linear ODE with reasonable<fn>For example, continuous.</fn>
 coefficients and <m>n</m>
initial conditions always has exactly one solution. We shall now see that
a boundary value problem may have no solutions at all. Or it may have exactly
one solution. Or it may have infinitely many solutions. We shall start
by finding all solutions to the ODE
<men xml:id="eqnbvODE">
y'+y=0
</men>
We shall then impose various boundary conditions and see what happens.
</p>

<p>The function <m>y(t)=e^{rt}</m> is a solution to <xref ref="eqnbvODE"/> if and only if
<me>
r^2e^{rt}+e^{rt}=0\iff r^2+1=0\iff r=\pm i
</me>
where <m>i</m> (which electrical engineers often denote<fn>This is to avoid confusion with the current, which is typically called <m>i</m>.</fn>
  <m>j</m>) is a square root
of <m>-1</m>. Thus the general solution to the second order linear ODE  <xref ref="eqnbvODE"/>
is <m>y(t)=C'_1 e^{it}+C'_2e^{-it}</m>, with <m>C_1'</m> and <m>C_2'</m> arbitrary constants.
We may rewrite this general solution in terms of <m>\sin t</m> and <m>\cos t</m> by
substituting in
<me>
e^{it}=\cos t+i\sin t\qquad
e^{-it}=\cos t-i\sin t
</me>
This gives
<me>
y(t)=C'_1\big(\cos t+i\sin t)+C'_2(\cos t-i\sin t)
=C_1\cos t+C_2\sin t
</me>
where <m>C_1=C'_1+C'_2</m>, and  <m>C_2=i(C'_1-C'_2)</m>.
Note that there is nothing stopping <m>C_1'</m> and <m>C_2'</m> from being complex
numbers. So there is nothing stopping <m>C_1=C'_1+C'_2</m>, and
<m>C_2=i(C'_1-C'_2)</m> from being real numbers.
</p>

<p><ol label="a">
<li>
Now consider the boundary value problem
<men xml:id="eqnbvpA">
y'+y=0\qquad y(0)=0\qquad y(2\pi)=1
</men>
The function <m>y(t)</m> satisfies the ODE if and only if it is of the form
<me>
y(t)=C_1\cos t+C_2\sin t
</me>
for some constants <m>C_1</m> and <m>C_2</m>. A function
of this form satisfies the boundary condition <m>y(0)=0</m> if and only if
<me>
0=y(0)= C_1\cos 0+C_2\sin 0 =C_1
</me>
A function of this form satisfies the boundary condition <m>y(2\pi)=1</m> if and
only if
<me>
1=y(2\pi)= C_1\cos 2\pi+C_2\sin 2\pi =C_1
</me>
The two requirements <m>C_1=0</m> and <m>C_1=1</m> are incompatible. So the boundary
value problem <xref ref="eqnbvpA"/> has no solution at all.
</li>
<li>
Next consider the boundary value problem
<men xml:id="eqnbvpB">
y'+y=0\qquad y(0)=0\qquad y\Big(\frac{\pi}{2}\Big)=0
</men>
The function <m>y(t)</m> satisfies the ODE if and only if it is of the form
<me>
y(t)=C_1\cos t+C_2\sin t
</me>
for some constants <m>C_1</m> and <m>C_2</m>. A function
of this form satisfies the boundary condition <m>y(0)=0</m> if and only if
<me>
0=y(0)= C_1\cos 0+C_2\sin 0 =C_1
</me>
A function of this form satisfies the boundary condition
<m>y\big(\frac{\pi}{2}\big)=0</m> if and  only if
<me>
0=y\Big(\frac{\pi}{2}\Big)
 = C_1\cos \Big(\frac{\pi}{2}\Big)+C_2\sin\Big(\frac{\pi}{2}\Big) =C_2
</me>
So we have a solution if and only if <m>C_1=C_2=0</m> and
the boundary value problem <xref ref="eqnbvpB"/> has exactly one solution, namely <m>y(t)=0</m>, which is a bit dull.
</li>
<li>
Finally consider the boundary value problem
<men xml:id="eqnbvpC">
y'+y=0\qquad y(0)=0\qquad y(2\pi)=0
</men>
The function <m>y(t)</m> satisfies the ODE if and only if it is of the form
<me>
y(t)=C_1\cos t+C_2\sin t
</me>
for some constants <m>C_1</m> and <m>C_2</m>. A function
of this form satisfies the boundary condition <m>y(0)=0</m> if and only if
<me>
0=y(0)= C_1\cos 0+C_2\sin 0 =C_1
</me>
A function of this form satisfies the boundary condition
<m>y(2\pi)=0</m> if and  only if
<me>
0=y(2\pi)= C_1\cos (2\pi)+C_2\sin(2\pi) =C_1
</me>
So we have a solution if and only if <m>C_1=0</m> and
the boundary value problem <xref ref="eqnbvpC"/> has infinitely many solutions, namely
<m>y(t)=C_2\sin t</m> with <m>C_2</m> being an arbitrary constant.
</li>
</ol>
</p></example>


</section>
