<?xml version="1.0" encoding="UTF-8" ?>
<section xmlns:xi="http://www.w3.org/2001/XInclude" xml:id="sec_planet">

<!-- Copyright 2018-2020 Joel Feldman, Andrew Rechnitzer and Elyse Yeager -->
<!-- This work is licensed under the Creative Commons Attribution-NonCommercial-ShareAlike 4.0 International License-->
<!-- https://creativecommons.org/licenses/by-nc-sa/4.0 -->

<title>Optional <mdash/> Planetary Motion</title>

<p>
We now return to the claim, made in ยง<xref ref="sec_central_forces"/> on central
forces, that if <m>\vr(t)</m> obeys Newton's inverse square law
<me>
\difftwo{\vr}{t} = -\frac{GM}{r^3}\vr = -\frac{GM}{r^2}\hat\vr
</me>
then the curve obeys Kepler's laws
<ol>
<li>
<m>\vr(t)</m> runs over an ellipse having one focus at the origin and
</li>
<li>
<m>\vr(t)</m> sweeps out equal areas in equal times and
</li>
<li>
the square of the period is proportional to the cube of the major axis of the
ellipse.
</li>
</ol>
We just showed, in ยง<xref ref="sec_central_forces"/>, that the fact that
<m>-\frac{GM}{r^3}\vr</m> is parallel to <m>\vr</m> implies that <m>\vr(t)</m>
lies in a plane through the origin and sweeps out equal area in equal times.
We now verify the remaining Kepler laws.
</p>

<p>We start by just rewriting Newton's laws above in polar coordinates.
We saw in Lemma <xref ref="lem_polar"/>.c, that if we write <m>\vr(t) = r(t)\,\hat\vr(t)</m>,
then
<md>
<mrow>
\difftwo{\vr}{t} &amp;=
  \left(\difftwo{r}{t}-r\ \left(\diff{\theta}{t}\right)^2\right) \hat\vr
   +\left(r\ \difftwo{\theta}{t} + 2 \diff{r}{t}\ \diff{\theta}{t}\right)\hat\vth
</mrow><mrow>
&amp;= -\frac{GM}{r^3}\vr
= -\frac{GM}{r^2}\hat\vr
</mrow>
</md>
The <m>\hat\vr</m> and <m>\hat\vth</m> components of this equation are
<md>
<mrow>
\difftwo{r}{t}-r\ \left(\diff{\theta}{t}\right)^2 &amp;= -\frac{GM}{r^2}
</mrow><mrow>
r\ \difftwo{\theta}{t} + 2 \diff{r}{t}\ \diff{\theta}{t} &amp;= 0
</mrow>
</md>
The second of these two equations only tells us that
<me>
\diff{\ }{t}\left\{r^2\,\diff{\theta}{t}\right\}
= r\left\{
     r\ \difftwo{\theta}{t} + 2 \diff{r}{t}\ \diff{\theta}{t}\right\} = 0
\implies
r^2\,\diff{\theta}{t} = h,\quad\text{a constant}
</me>
which we already knew. Substituting <m>\diff{\theta}{t} =\frac{h}{r^2}</m>
into the first equation gives
</p>

<fact xml:id="eqn_planetRadialR">
<statement><p>
<me>
  \difftwo{r}{t}-\frac{h^2}{r^3} = -\frac{GM}{r^2}
</me></p>
</statement></fact>

<p>
This equations contains a lot of <m>\frac{1}{r}</m>'s. So let's set <m>u=\frac{1}{r}</m>.
Furthermore, for the first of Kepler's laws, we really want <m>r</m> as a function of
<m>\theta</m> rather than <m>t</m>. So let's make <m>u</m> a function of <m>\theta</m> and write
<me>
r(t) = \frac{1}{u(\theta(t))}
</me>
Then
<md>
<mrow>
\diff{r}{t}(t) &amp;= -\frac{1}{u^2}
        \diff{u}{\theta}\big(\theta(t)\big)\diff{\theta}{t}(t)
   = - h\diff{u}{\theta}\big(\theta(t)\big)\qquad
\text{since } \diff{\theta}{t} = \frac{h}{r^2}=hu^2
</mrow><mrow>
\difftwo{r}{t}(t)
   &amp;= -h\difftwo{u}{\theta}\big(\theta(t)\big)\diff{\theta}{t}(t)
     = -h^2 u\big(\theta(t)\big)^2 \difftwo{u}{\theta}\big(\theta(t)\big)
</mrow>
</md>
and our equation becomes
</p>


<fact xml:id="eqn_planetRadialU">
<statement><p>
<me>
-h^2u^2\difftwo{u}{\theta} -h^2u^3= -GM u^2\qquad\text{or}\qquad
\difftwo{u}{\theta} + u = \frac{GM}{h^2}
</me>
</p></statement>
</fact>

<p>
This is a second order, linear, ordinary differential equation
with constant coefficients.  Recall<fn>See Appendix <xref ref="ap_ODE"/>.</fn> that the general solution of such an
equation is the sum of a <q>particular solution</q> (i.e. any one solution,
which in this case we can take to be the constant function <m>\frac{GM}{h^2}</m>)
plus the general solution of the homogeneous equation
<m>u'+u=0</m>, which one often writes as
<me>
A\cos\theta +B\sin\theta
</me>
with <m>A</m> and <m>B</m>  arbitrary constants. In this particular application it is
more convenient to write the solution in a different, standard but less
commonly used, form. Namely, we can use the triangle
</p>

<sidebyside width="20%">
<image source="figs/trianglePl"/>
</sidebyside>

<p>to write <m>A= C\cos\alpha</m> and <m>B=C\sin\alpha</m> so that
the general solution of the homogeneous equation <m>u'+u=0</m> becomes
<me>
C\cos\alpha\cos\theta +C\sin\alpha\sin\theta
=C\cos(\theta-\alpha)
</me>
with <m>C</m> and <m>\alpha</m> being arbitrary constants. So the general solution
to <xref ref="eqn_planetRadialU"/> is
<me>
u(\theta) = \frac{GM}{h^2} + C\cos(\theta-\alpha)
</me>
and the general solution to <xref ref="eqn_planetRadialR"/> is
<me>
r(t) = \frac{1}{\frac{GM}{h^2} + C\cos(\theta(t)-\alpha)}
</me>
The angle <m>\alpha</m> just shifts the zero point of our coordinate <m>\theta</m>.
By rotating our coordinate system by <m>\alpha</m>, we can arrange that <m>\alpha=0</m>
and then
<me>
r(t) = \frac{1}{\frac{GM}{h^2} + C\cos(\theta(t))}
     = \frac{\ell}{1+\veps\cos\theta}
\qquad\text{with}\quad
\ell=\frac{h^2}{GM},\
\veps=\frac{Ch^2}{GM}
</me>
As we saw in Example <xref ref="eg_conicA"/>, this is exactly the equation
of a conic section with eccentricity <m>\veps</m>.
</p>

<p>That leaves only the last of Kepler's laws, relating the period
to the semi-major axis. As we are talking about planets, whose orbits
remain bounded, our conic section must be a circle or ellipse, rather
than a parabola or hyperbola.
Looking back at Example <xref ref="conicB"/>, we see that the semi-major
and semi-minor axes of our ellipse are
<md>
<mrow>
a=\frac{\ell}{1-\veps^2}
\qquad
b=\frac{\ell}{\sqrt{1-\veps^2}}
</mrow>
</md>
The period <m>T</m> of our orbit is just the length of time it takes
the radius vector <m>\vr(t)</m> to sweep out the area of the ellipse<fn>You
probably computed the area of an ellipse in first year calculus. If not,
you should be able to do it now in a few lines.</fn>,
which is <m>\pi ab</m>.  As the rate at which the radius vector is sweeping out
area is <m>\frac{1}{2} r^2\diff{\theta}{t} = \frac{h}{2}</m>, we have
<md>
<mrow>
T^2 = \Big(\frac{\pi a b}{h/2}\Big)^2
    =\frac{4\pi^2 a^2 b^2}{h^2}
    =\frac{4\pi^2 a^2 b^2}{GM\ell}
    =\frac{4\pi^2}{GM}\ a^3\qquad
\text{since }\ell=\frac{b^2}{a}
</mrow>
</md>
</p>


<!-- <xi:include href="../problems/prob_s1.10.ptx" /> -->

</section>
