<?xml version="1.0" encoding="UTF-8" ?>
<section xmlns:xi="http://www.w3.org/2001/XInclude" xml:id="sec_curvature">

<!-- Copyright 2018-2020 Joel Feldman, Andrew Rechnitzer and Elyse Yeager -->
<!-- This work is licensed under the Creative Commons Attribution-NonCommercial-ShareAlike 4.0 International License-->
<!-- https://creativecommons.org/licenses/by-nc-sa/4.0 -->

<title>Curvature</title>


<p>
So far, when we have wanted to approximate a complicated curve by
a simple curve near some point, we drew the tangent line
to the curve at the point. That's pretty crude. In particular tangent
lines are straight <mdash/> they don't curve. We will get a much better idea
of what the complicated curve looks like if we approximate it, locally,
by a very simple <q>curvy curve</q> rather than by a straight line.
Probably the simplest <q>curvy curve</q> is a circle
<fn>Circles are good
for studying <q>curvature</q>, because, unlike parabolas for example, the rate
at which a circle curves is uniform over the entire circle.</fn>
and that's what we'll use.
</p>

<definition xml:id="def_curvature">
<statement><p>
<ol label="a">
<li>
The circle which best approximates a given curve near a given
point is called the <term>circle of curvature</term> or the
<term>osculating circle</term>
<fn><q>Osculare</q> is the Latin verb <q>to kiss</q>.
The German mathematician Gottfried Wilhelm (von) Leibniz (1646--1716)
named the circle the <q>circulus osculans</q>.</fn> at the point.
</li>
<li>
The radius of the circle of curvature is called the <term>radius of curvature</term>
at the point and is normally denoted <m>\rho</m>.
</li>
<li>
The <term>curvature</term> at the point is <m>\ka=\frac{1}{\rho}</m>.
</li>
<li>
The centre of the circle of curvature is called <term>centre of curvature</term>
at the point.
</li>
</ol>
</p></statement>
</definition>

<p>
These definitions are illustrated in the figure below. It shows (part of)
the osculating circle at the point <m>P</m>. The point <m>C</m> is the centre of
curvature.
</p>

<sidebyside>
<image source="figs/curvatureDef"/>
</sidebyside>

<p>Note that when the curvature <m>\ka</m> is large, the radius of curvature <m>\rho</m>
is small and we have a very curvy curve. On the other hand when the
curvature <m>\ka</m> is small, the radius of curvature <m>\rho</m> is large and
our curve  is almost straight. In particular, straight lines have
curvature exactly zero.
</p>

<p>We are now going to determine how to find the circle of curvature,
starting by figuring out what its radius should be. We'll first look
at curves
<fn>We'll also assume that the curves of interest are smooth,
with no cusps for example, and not straight, so that the radius of
curvature <m>0 \lt \rho \lt \infty</m>.</fn>
</p>

<p>that lie in the <m>xy</m>-plane and then move on to curves in 3d.
Consider the black curve in the figure below.
</p>

<sidebyside>
<image source="figs/curvature"/>
</sidebyside>
<p>
That figure also contains a (portion of a) red circle that fits the
curve really well between the two radial lines that are (a very small) angle
<m>\dee{\theta}</m> apart. So the arclength <m>\dee{s}</m> of the part of the black
curve between the two radial lines, should be (essentially) the same
as the arc length of the circle between the two radial lines, which is
<m>\rho\,|\dee{\theta}|</m>, where <m>\rho</m> is the radius of the circle.
(We put in absolute values to take into account the
possibility that <m>\dee{\theta}</m> could be negative.)
Thus <m>\dee{s} = \rho\,|\dee{\theta}|</m>. When <m>\dee{\theta}</m> is a macroscopic
angle, this is of course an approximation. But in the limit as
<m>\dee{\theta}\rightarrow 0</m>, we should end up with
<me>
\rho = \Big|\diff{s}{\theta}\Big|
</me>
We now have a formula for the radius of curvature, but not in a very
convenient form, because to evaluate it we would need to know the arc length
along the curve as a function of the angle <m>\theta</m> in the rightmost
figure below.
We'll now spend some time developing more convenient formulae for <m>\rho</m>.
First consider the three figures below. They all show the same curve
as in the last figure. The leftmost figure just shows
<ul>
<li>
the curve of interest, which is the black curve, and
</li>
<li>
the (blue) point of interest on the black curve. We want to find the curvature
at that point.
</li>
</ul>
The middle figure shows the same curve and point of interest and also
shows
<ul>
<li>
the red circle of curvature (i.e. best fitting circle) for the black curve
at the blue dot.
</li>
<li>
The red dot is the centre of curvature.
</li>
</ul>
The rightmost figure shows the same black curve, blue point of interest
and red circle of curvature (at least part of it) somewhat enlarged.
<ul>
<li>
The angle <m>\theta</m> is the angle between <m>\hi</m> and the radius
vector from the red dot (the centre of curvature) to the blue dot
(the point of interest).
</li>
<li>
<m>\hat\vT</m> is the tangent vector to the black curve at the blue
dot.
</li>
<li>
The angle <m>\phi</m> is the angle between <m>\hi</m> and <m>\hat\vT</m>.
The vector <m>\hat\vT</m> is also tangent to the red circle. As
the tangent and radius vectors for circles are perpendicular to
each other
<fn>We saw that in Example <xref ref="eg_paramCircleTan"/>.</fn>
,
we have that <m>\phi=\theta+\frac{\pi}{2}</m> and hence
<m>\rho = \Big|\diff{s}{\phi}\Big|</m> too.
</li>
</ul>
</p>

<sidebyside width="32%">
<image source="figs/curvatureB1"/>
<image source="figs/curvatureB2"/>
<image source="figs/curvatureB"/>
</sidebyside>

<p>
We are now in a position to develop a bunch of formulae for the radius
of curvature <m>\rho</m> and the curvature <m>\ka=\frac{1}{\rho}</m>, that are more
convenient than <m>\ka = \Big|\diff{s}{\phi}\Big|^{-1}</m>. These formulae
will use the
</p>

<definition xml:id="notn_curveNotation">
<statement><p>
If <m>\vr(t)</m> is a parametrized curve, then
<ul>
<li>
<m>\vv(t) = \diff{\vr}{t}(t)</m> is the velocity vector at <m>\vr(t)</m>
</li>
<li>
<m>\va(t) = \difftwo{\vr}{t}(t) </m> is the acceleration vector at <m>\vr(t)</m>
</li>
<li>
<m>\hat\vT(t)</m> is the unit tangent vector to the curve at <m>\vr(t)</m> that
points in the direction of increasing <m>t</m>.
</li>
<li>
<m>\hat\vN(t)</m> is the unit normal vector to the curve at <m>\vr(t)</m>
that points toward the centre of curvature.
</li>
<li>
<m>\ka(t)</m> is the curvature at <m>\vr(t)</m>
</li>
<li>
<m>\rho(t)</m> is the radius of curvature at <m>\vr(t)</m>
</li>
</ul>
</p></statement>
</definition>


<theorem xml:id="thm_curvatureFormulae">
<statement>
<p><ol label="a">
<li>
Given
<fn>The equation <m>s=s(\phi)</m> is called the <q>intrinsic
equation of the curve</q>.</fn>
 <m>s(\phi)</m>,
i.e. if we know the arc length along the curve as a function of
the angle
<fn>The notation <m>\measuredangle(\hi,\hat\vT)</m>
means <q>the angle between <m>\hi</m> and <m>\hat\vT</m></q>.</fn>
<m>\phi=\measuredangle(\hi,\hat\vT)</m>, then
<me>
\rho = \Big|\diff{s}{\phi}\Big|\qquad
\ka = \Big|\diff{s}{\phi}\Big|^{-1}\qquad
\ka = \Big|\diff{\phi}{s}\Big|
</me>
</li>
<li xml:id="thm_curvatureFormulae_part_b">
Given <m>\vr(s)</m>,
i.e. if we have a parametrization of the curve in terms of arc length, then
<me>
\diff{\hat\vT}{s}(s) = \ka(s)\,\hat\vN(s)
</me>
where <m>\hat\vN(s)</m> is the unit normal vector to the curve at <m>\vr(s)</m>
that points toward the centre of curvature.
</li>
<li xml:id="thm_curvatureFormulae_part_c">
Given <m>\vr(t)</m>, i.e. if we have a general parametrized curve,
then
<md>
<mrow>
\diff{\hat\vT}{t} = \ka \diff{s}{t} \hat\vN\quad
\vv(t) =  \diff{s}{t}(t)\,\hat\vT(t) \quad
\va(t)
       =  \difftwo{s}{t}\hat\vT
                           + \ka\Big(\diff{s}{t}\Big)^2\hat\vN
</mrow>
</md>
</li>
<li>
Given <m>\big(x(t)\,,\,y(t)\big)</m>, (for curves in the <m>xy</m>-plane)
<me>
\ka = \left|\frac{\vv(t)\times\va(t)}{\big(\diff{s}{t}\big)^3}\right|
=\frac{\big|\diff{x}{t}\difftwo{y}{t}-\diff{y}{t}\difftwo{x}{t}\big|}
{ {\big[\big(\diff{x}{t}\big)^2+\big(\diff{y}{t}\big)^2\big]}^{3/2} }
</me>
</li>
<li xml:id="thm_curvatureFormulae_part_e">
Given <m>y(x)</m>, (again for curves in the <m>xy</m>-plane)
<me>
\ka
=\frac{\big|\difftwo{y}{x}\big|}
{ {\big[1+\big(\diff{y}{x}\big)^2\big]}^{3/2} }
</me>
</li>
</ol>
</p></statement>
</theorem>

<proof>
<p>
(a)
Given <m>s(\phi)</m>, then
<me>
\rho = \Big|\diff{s}{\phi}\Big|\qquad
\ka = \Big|\diff{s}{\phi}\Big|^{-1}
</me>
As we are assuming that <m>0 \lt \rho=\Big|\diff{s}{\phi}\Big| \lt \infty</m>,
the inverse function theorem says that we can
invert the function <m>s(\phi)</m> (at least locally) to get <m>\phi</m> as a
function of <m>s</m>, and that
<me>
\ka = \Big|\diff{\phi}{s}\Big|
</me>
</p>

<p> (b)
Given <m>\vr(s)</m>,
then, by Lemma <xref ref="lem_CVtanArclen"/>.c, <m>\hat\vT(s) = \vr'(s)</m>
is a unit tangent to the curve at <m>\vr(s)</m> and
<me>
\diff{\hat\vT}{s} = \diff{\hat\vT}{\phi} \diff{\phi}{s}
\tag{$*$}
</me>
Now up to a sign <m>\diff{\phi}{s}</m> is <m>\ka</m>, and just because
<m>\phi=\measuredangle(\hi,\hat\vT)</m>, with <m>\hat\vT</m> a unit vector,
<me>
\begin{split}
\hat\vT&amp;=\cos\phi\,\hi + \sin\phi\,\hj \\
\implies \diff{\hat\vT}{\phi}&amp;= -\sin\phi\,\hi + \cos\phi\,\hj
\end{split}
\tag{$**$}
</me>
So <m>\diff{\hat\vT}{\phi}</m> is a unit vector that is
perpendicular
<fn>Think about why this should be the case. In particular,
sketch <m>\hat\vT</m> and <m>\phi</m> and think about what the sketch says about
<m>\diff{\hat\vT}{\phi}</m>.</fn>
to <m>\hat\vT</m>, and hence to the curve at <m>\vr(s)</m>, and
<me>
\diff{\hat\vT}{s}(s) = \ka(s)\,\hat\vN(s)
\tag{$\dagger$}
</me>
with <m>\hat\vN(s)</m> a unit normal vector to the curve at <m>\vr(s)</m>.
In fact, <m>\hat\vN(s)</m> is the unit normal vector to the curve at <m>\vr(s)</m>
that points toward the centre of curvature.
</p>

<p>To see that,
look at the figures below
<fn>In each of the four figures, the arrow on the curve specifies the direction of increasing arc length <m>s</m> and the red dot is the centre of curvature for the curve at the blue dot.</fn>,
and note that substituting the sign information
from each figure into (<m>*</m>) gives (<m>\dagger</m>).
For example,
</p>

<sbsgroup width="45%">
<sidebyside>
<image source="figs/curvatureSignA"/>
<image source="figs/curvatureSignC"/>
</sidebyside>
<sidebyside>
<image source="figs/curvatureSignB"/>
<image source="figs/curvatureSignD"/>
</sidebyside>
</sbsgroup>

<p>
consider the figure on the lower left. In that figure,
<ul>
<li><p>
the <m>x</m> component of <m>\hat\vT</m> is negative (<m>\hat\vT</m> is leftward pointing in the figure),
<ul>
<li>
which makes <m>\cos\phi</m> negative (see (<m>**</m>)),
</li>
<li>
which makes the <m>y</m> component of <m>\diff{\hat\vT}{\phi}</m> negative
            (see (<m>**</m>) again),
</li>
<li>
so <m>\diff{\hat\vT}{\phi}</m> is downward pointing,
</li>
</ul>
so <m>\diff{\hat\vT}{\phi}=-\hat\vN</m> (the centre of curvature is the red dot
above the curve) and
</p></li>
<li> as <m>s</m> increases (i.e. as you move in the direction of the
arrow on the curve), <m>\phi</m> decreases (on the far right hand part of the curve <m>\phi\approx\frac{\pi}{2}</m>, while on the far left hand part of the curve <m>\phi\approx 0</m>), so <m>\diff{\phi}{s} \lt 0</m> and
<m>\ka = \big|\diff{\phi}{s}\big| = - \diff{\phi}{s}</m>.
</li>
<li> So by (<m>*</m>),
<m>\diff{\hat\vT}{s} = \diff{\hat\vT}{\phi} \diff{\phi}{s}
=\big(-\hat\vN)(-\ka) = \ka\hat\vN</m>.
</li>
</ul>
In each of the three other figures we also end up with
<m>\diff{\hat\vT}{s} = \ka(s)\hat\vN(s)</m>.
</p>


<p>
Note that if <m>\ka(s)=0</m>, then <m>\hat\vN(s)</m> is not defined. This makes sense:
if the curve is (locally) a straight line, there is no <q>best fitting circle</q>.
</p>

<p> (c)
Given <m>\vr(t)</m>,
i.e. if we have a general parametrized curve, we can determine a unit
tangent vector by using Lemma <xref ref="lem_CVtanArclen"/>:
<me>
\vv(t) = \diff{\vr}{t}(t) = \diff{s}{t}(t)\,\hat\vT(t)
\quad\implies\quad
\hat\vT(t) = \frac{\vr'(t)}{|\vr'(t)|}
</me>
Then we can determine <m>\ka</m> and <m>\hat\vN</m>  by differentiating
<m>\hat\vT(t)</m> and using the chain rule:
<me>
\diff{\hat\vT}{t} = \diff{\hat\vT}{s}\diff{s}{t}
 = \ka \diff{s}{t} \hat\vN
\quad\implies\quad
\ka(t) = \frac{|\hat\vT'(t)|}{|\vr'(t)|}
</me>
Also, if we differentiate <m>\vv(t) = \diff{s}{t}\hat\vT(t)</m>, we get
that the acceleration
<me>
\va(t) = \difftwo{\vr}{t}
       =  \difftwo{s}{t}\hat\vT + \diff{s}{t}\,\diff{\hat\vT}{t}
       =  \difftwo{s}{t}\hat\vT
                           + \ka\Big(\diff{s}{t}\Big)^2\hat\vN
</me>
</p>

<p xml:id="clpcurvesthm_curvatureFormulae_partd">
(d)
Given <m>\big(x(t)\,,\,y(t)\big)</m>, (for curves in the <m>xy</m>-plane),
we can read off the curvature from
<md>
<mrow>
\vv(t)\times\va(t)
&amp;=\Big(\diff{s}{t}(t)\,\hat\vT(t)\Big)\times
    \Big(\difftwo{s}{t}\hat\vT
                           + \ka\Big(\diff{s}{t}\Big)^2\hat\vN\Big)

</mrow><mrow>
&amp;= \ka\Big(\diff{s}{t}\Big)^3\hat\vT\times\hat\vN
\qquad\text{(since }  \hat\vT\times\hat\vT=\vZero
</mrow>
</md>
Think of <m>\hat\vT</m> and <m>\hat\vN</m> as 3d vectors that whose <m>z</m>-components happen to be zero. As <m>\hat\vT</m> and <m>\hat\vN</m> are mutually perpendicular
unit vectors in the <m>xy</m>-plane, the cross-product <m>\hat\vT\times\hat\vN</m>
will be either <m>+\hk</m> or <m>-\hk</m>. In both cases,
<m>|\vv(t)\times\va(t)\big| = \ka\big|\diff{s}{t}\big|^3</m>. So
<md>
<mrow>
\ka &amp;= \left|\frac{\vv(t)\times\va(t)}{\big(\diff{s}{t}\big)^3}\right|
=\left|\frac{\big[\diff{x}{t}\hi+\diff{y}{t}\hj\big]\times
        \big[\difftwo{x}{t}\hi+\difftwo{y}{t}\hj\big]}
           {\big(\diff{s}{t}\big)^3}\right|
=\left|\frac{\big[\diff{x}{t}\difftwo{y}{t}-\diff{y}{t}\difftwo{x}{t}\big]\hk}
           {\big(\diff{s}{t}\big)^3}\right|

</mrow><mrow>
&amp;=\frac{\big|\diff{x}{t}\difftwo{y}{t}-\diff{y}{t}\difftwo{x}{t}\big|}
{ {\big[\big(\diff{x}{t}\big)^2+\big(\diff{y}{t}\big)^2\big]}^{3/2} }
</mrow>
</md>
</p>

<p> (e)
Given <m>y(x)</m>, again for curves in the <m>xy</m>-plane,
we can parametrize the curve using <m>x</m> as the parameter:
<me>
\vr(t) = \big(X(t)\,,\,Y(t)\big) \qquad\text{with $X(t)=t$ and $Y(t) =y(t)$}
</me>
Then
<me>
\diff{X}{t} = 1 \qquad
\difftwo{X}{t} = 0 \qquad
\diff{Y}{t} = \diff{y}{x} \qquad
\difftwo{Y}{t} = \difftwo{y}{x}
</me>
and
<me>
\ka
=\frac{\big|\diff{X}{t}\difftwo{Y}{t}-\diff{Y}{t}\difftwo{X}{t}\big|}
{ {\big[\big(\diff{X}{t}\big)^2+\big(\diff{Y}{t}\big)^2\big]}^{3/2} }
=\frac{\big|\difftwo{y}{x}\big|}
{ {\big[1+\big(\diff{y}{x}\big)^2\big]}^{3/2} }
</me>
</p></proof>

<p>
Take another look at Theorem <xref ref="thm_curvatureFormulae"/>
and note that
<ul>
<li>
the tangential component of acceleration, i.e. <m>\difftwo{s}{t}</m>,
arises purely from change in speed while
</li>
<li>
the normal component of acceleration, i.e. <m>\ka\big(\diff{s}{t}\big)^2</m>,
arises from curvature and is proportional to the square of the speed
<m>\diff{s}{t}</m>. Think about what you feel when you are driving.
That's why velodromes and (car) race tracks often have banked corners.
</li>
</ul>
</p>

<example xml:id="eg_curveCircle">
<p>
As a warm up example, and also a check that our formulae make sense,
we'll find the curvature <m>\ka</m>, radius of curvature, <m>\rho</m>, unit tangent
vector, <m>\hat\vT</m>, unit normal vector, <m>\hat\vN</m>, and centre of curvature
of the parametrized curve
<me>
\vr(t) = a\cos t\,\hi + a\sin t\,\hj
</me>
with the constant <m>a \gt 0</m>.
This is, of course, the circle of radius <m>a</m> centred on the origin.
As
<me>
\vv(t)=\diff{\vr}{t}(t)= -a\sin t\,\hi + a\cos t\,\hj
\implies \diff{s}{t}(t) = |\vv(t)| = a
</me>
we have that the unit tangent vector
<me>
\vT(t) = \frac{\vv(t)}{|\vv(t)|} = -\sin t\,\hi + \cos t\,\hj
</me>
Note, as a check, that this is indeed a vector of length one and
is perpendicular to the radius vector (as expected <mdash/> the curve is a circle).
As
<me>
\diff{\hat\vT}{t}(t)= -\cos t\,\hi  -\sin t\,\hj
</me>
we have that
<me>
\hat\vN(t) = \frac{\diff{\hat\vT}{t}(t)}{\big|\diff{\hat\vT}{t}(t)\big|}
           = -\cos t\,\hi  -\sin t\,\hj
\quad
\ka(t)
= \frac{\big|\diff{\hat\vT}{t}(t)\big|}{\diff{s}{t}(t)}
=\frac{1}{a}
\quad
\rho(t)=\frac{1}{\ka(t)} =a
</me>
Now look at the figure.
</p>

<sidebyside>
<image source="figs/circleCentreB"/>
</sidebyside>

<p>
To get to the centre of curvature we should start from
<m>\vr(t)</m> and walk a distance <m>\rho(t)</m>, which after all is the radius
of curvature, in the direction <m>\hat\vN(T)</m>, which is pointing towards the centre of curvature. So the centre of curvature is
<me>
\vr(t)+\rho(t)\hat\vN(t)
=\big[a\cos t\,\hi  +a\sin t\,\hj\big]
+a\big[-\cos t\,\hi  -\sin t\,\hj\big]
= \vZero
</me>
This makes perfectly good sense <mdash/> the radius of curvature is
the radius of the original circle and the centre of curvature is the
centre of the original circle.
</p>

<p>One alternative calculation of the curvature, using <m>x(t) = a\cos t </m>,
<m>y(t)=a\sin t</m>, is
<md>
<mrow>
\ka(t)
&amp;=\frac{\big|
  \diff{x}{t}(t)\difftwo{y}{t}(t)-\diff{y}{t}(t)\difftwo{x}{t}(t)
  \big|}{\Big[\big(\diff{x}{t}(t)\big)^2
                +\big(\diff{y}{t}(t)\big)^2\Big]^{3/2}}
</mrow><mrow>
&amp;=\frac{\big|
  -a\sin t\big(-a\sin t\big)-a\cos t\big(-a\cos t\big)
  \big|}{\big[\big(-a\sin t\big)^2
                +\big(a\cos t\big)^2\big]^{3/2}}
</mrow><mrow>
&amp;=\frac{1}{a}
</mrow>
</md>
Another alternative calculation of the curvature, using <m>y(x)
=\sqrt{a^2-x^2}</m> (for the part of the circle with <m>y \gt 0</m>),
<me>
y'(x) = -\frac{x}{\sqrt{a^2-x^2}}=-\frac{x}{y(x)} \qquad
y'(x) = -\frac{y(x) - xy'(x)}{y(x)^2}
       =  -\frac{y(x)^2 + x^2}{y(x)^3}
       =  -\frac{a^2}{y(x)^3}
</me>
is
<md>
<mrow>
\ka(x)
&amp;=\frac{\big|\difftwo{y}{x}(x)\big|}
  {\Big[1+\big(\diff{y}{x}(x)\big)^2\Big]^{3/2}}
=\frac{\frac{a^2}{y(x)^3}}
  {\Big[1+\frac{x^2}{y(x)^2}\Big]^{3/2}}
=\frac{a^2}{\big[y(x)^2+x^2\big]^{3/2}}
=\frac{1}{a}
</mrow>
</md>
</p></example>


<example xml:id="eg_curvatureEtc">
<p>
As a more computationally involved example, we'll analyze
<md>
<mrow>
\vr(t) &amp;= \big(\cos t + t\sin t\big)\hi +\big(\sin t-t\cos t\big)\hj
\qquad t \gt 0
</mrow><mrow>
\vv(t) &amp;= t\cos t\,\hi + t\sin t\,\hj
</mrow><mrow>
\va(t) &amp;= \big(\cos t - t\sin t\big)\hi +\big(\sin t+t\cos t\big)\hj
</mrow>
</md>
We can read off from <m>\vv(t)</m>, that
<md>
<mrow>
\diff{s}{t}(t) &amp;= |\vv(t)| =t
</mrow><mrow>
\difftwo{s}{t}(t) &amp;= 1
</mrow><mrow>
\vT(t)&amp;=\frac{\vv(t)}{|\vv(t)|} = \cos t\,\hi + \sin t\,\hj
</mrow>
</md>
Next, from <m>\va(t)</m>, we read off that
<md>
<mrow>
\va(t) &amp;=\big(\cos t - t\sin t\big)\hi +\big(\sin t+t\cos t\big)\hj\qquad
\text{and}
</mrow><mrow>
\va(t)&amp;=\difftwo{s}{t}(t)\,\hat\vT(t)
                             +\ka(t)\big(\diff{s}{t}(t)\big)^2\hat\vN(t)
</mrow>
<intertext>(by Theorem <xref ref="thm_curvatureFormulae"/> .c)</intertext>
<mrow>
&amp;=\cos t\,\hi + \sin t\,\hj +t^2\ka(t) \hat\vN(t)
</mrow><mrow>
\implies
t^2\ka(t) \hat\vN(t)&amp;= - t\sin t\,\hi + t\cos t\,\hj
</mrow>
</md>
so that
<md>
<mrow>
\ka(t) = \frac{1}{t} \quad\text{and}\quad
\hat\vN(t)= -\sin t\,\hi + \cos t\,\hj
</mrow>
</md>
As an alternative calculation of the curvature, we have
<md>
<mrow>
\ka(t)
&amp;=\frac{|\vv(t)\times\va(t)|}{(\diff{s}{t}(t))^3}
</mrow><mrow>
&amp;=\frac{\big|\big[t\cos t\,\hi + t\sin t\,\hj\big]\times
      \big[\big(\cos t - t\sin t\big)\hi +\big(\sin t+t\cos t\big)\hj\big]\big|}
{(\diff{s}{t}(t))^3}
</mrow><mrow>
&amp;=\frac{\big|\big[t\cos t\big(\sin t+t\cos t\big)
                 -t\sin t\big(\cos t - t\sin t\big)\big]\hk\big|}
{(\diff{s}{t}(t))^3}
</mrow><mrow>
&amp;=\frac{|t^2\hk|}{t^3}
=\frac{1}{t}
</mrow>
</md>
It pays to think before you calculate!
</p></example>


<!-- <xi:include href="../problems/prob_s1.3.ptx" /> -->

</section>
