<?xml version="1.0" encoding="UTF-8" ?>
<section xmlns:xi="http://www.w3.org/2001/XInclude" xml:id="sec_polar">

<!-- Copyright 2018-2020 Joel Feldman, Andrew Rechnitzer and Elyse Yeager -->
<!-- This work is licensed under the Creative Commons Attribution-NonCommercial-ShareAlike 4.0 International License-->
<!-- https://creativecommons.org/licenses/by-nc-sa/4.0 -->

<title>Optional <mdash/> Polar Coordinates</title>

<p>So far we have always written vectors in two dimensions in terms of the basis vectors
<m>\hi</m> and <m>\hj</m>. This is not always convenient. For example, when working in
polar coordinates it is often convenient to use basis vectors
<m>\hat\vr(\theta)</m>, <m>\hat\vth(\theta)</m> which depend on the value of the
current polar coordinate <m>\theta</m> <mdash/> though one usually just writes
<m>\hat\vr</m>, <m>\hat\vth</m>, suppressing the dependence on <m>\theta</m> from
the notation. When one is at the point with polar coordinates
<m>(r,\theta)</m>, these basis vectors are defined by
</p>

<fact xml:id="eqn_polarBasis">
<statement>
<sidebyside widths="45% 30%" valign="middle">
<p>
<md>
<mrow>
\hat\vr(\theta) &amp;= \cos\theta\,\hi + \sin\theta\,\hj
</mrow><mrow>
\hat\vth(\theta) &amp;= -\sin\theta\,\hi + \cos\theta\,\hj
</mrow>
</md>
</p>
<image source="figs/polar"/>
</sidebyside>
</statement>
</fact>

<p>
Note that this basis has two very nice properties.
<ol>
<li>
<m>|\hat\vr(\theta)| = |\hat\vth(\theta)| = 1</m>,
   <m>\hat\vr(\theta) \perp \hat\vth(\theta)</m>  (orthonormality)
</li>
<li>
<m>\diff{\hat\vr}{\theta}(\theta)= \hat\vth(\theta)</m>,
<m>\diff{\hat\vth}{\theta}(\theta) = -\hat\vr(\theta)</m>
</li>
</ol>
That <m>\diff{\hat\vr}{\theta}(\theta)</m> is some scalar multiple of
<m>\hat\vth(\theta)</m> follows just from the fact that <m>|\hat\vr(\theta)| = 1</m>.
<md>
<mrow>
|\hat\vr(\theta)| = 1 &amp;\implies \hat\vr(\theta)\cdot\hat\vr(\theta)=1
</mrow><mrow>
             &amp;\implies \hat\vr(\theta)\cdot \diff{\hat\vr}{\theta}(\theta)
                                =\frac{1}{2}\diff{}{t}\big(
                                   \hat\vr(\theta)\cdot\hat\vr(\theta)\big)
                                =0
</mrow><mrow>
         &amp;\implies  \diff{\hat\vr}{\theta}(\theta)\perp \hat\vr(\theta)
         \implies \diff{\hat\vr}{\theta}(\theta)\parallel \hat\vth(\theta)
</mrow>
</md>
Similarly, that <m>\diff{\hat\vth}{\theta}(\theta)</m> is some scalar
multiple of <m>\hat\vr(\theta)</m> follows just from the fact
that <m>|\hat\vth(\theta)| = 1</m>.
</p>

<lemma xml:id="lem_polar">
<statement><p>
If we parametrize a curve by giving its polar coordinates<fn>As usual <m>r</m> is the distance from the origin to the point and <m>\theta</m> is angle between the <m>x</m>-axis and the vector from the origin to the point.</fn>
 <m>\big(r(t)\,,\,\theta(t)\big)</m>, then
<ol label="a">
<li> the position vector of the point at time <m>t</m> is
<md>
<mrow>
\vr(t) = r(t)\ \hat\vr\big(\theta(t)\big)
</mrow>
</md>
</li>
<li> and the velocity vector of the point at time <m>t</m> is
<md>
<mrow>
\vv(t) = \diff{r}{t}(t)\ \hat\vr\big(\theta(t)\big)
             + r(t)\ \diff{\theta}{t}(t)\ \hat\vth\big(\theta(t)\big)
</mrow>
</md>
</li>
<li> and the acceleration vector of the point at time <m>t</m> is
<md>
<mrow>
\va(t) &amp;=
\left[\difftwo{r}{t}(t)\!-\!r(t)\Big(\diff{\theta}{t}(t)\Big)^2\right]
             \hat\vr\big(\theta(t)\big)
</mrow><mrow>
&amp;\hskip1in
   +\left[r(t)\ \difftwo{\theta}{t}(t)
          \!+\! 2 \diff{r}{t}(t)\diff{\theta}{t}(t)\right]
                  \hat\vth\big(\theta(t)\big)
</mrow>
</md>
</li>
</ol>
</p></statement>
</lemma>

<p>It is standard to suppress the arguments <m>t</m> and <m>\theta(t)</m>
and write, for example,
<me>
\vv= \diff{r}{t}\ \hat\vr
             + r\ \diff{\theta}{t}\ \hat\vth
</me>
But it is important to remember that the arguments really are there.
</p>

<proof>
<p>The vector from the origin to the point whose
polar coordinates are
<m>(r,\theta)</m> is <m>\vr = r\,\hat\vr(\theta)</m>. So if we parametrize a curve by
giving the polar coordinates at time <m>t</m>,
<md>
<mrow>
\vr(t) &amp;= r(t)\ \hat\vr\big(\theta(t)\big)
</mrow><mrow>
\vv(t) &amp;= \diff{r}{t}(t)\ \hat\vr\big(\theta(t)\big) +
              r(t)\ \diff{\hat\vr}{\theta}\big(\theta(t)\big)\
              \diff{\theta}{t}(t) \notag
</mrow><mrow>
        &amp;= \diff{r}{t}(t)\ \hat\vr\big(\theta(t)\big)
             + r(t)\ \diff{\theta}{t}(t)\ \hat\vth\big(\theta(t)\big)

</mrow><mrow>

\va(t) &amp; = \difftwo{r}{t}\ \hat\vr
                + \diff{r}{t}\ \diff{\hat\vr}{\theta}\ \diff{\theta}{t}
             + \diff{r}{t}\ \diff{\theta}{t}\ \hat\vth
             + r\ \difftwo{\theta}{t}\ \hat\vth
             + r\ \Big(\diff{\theta}{t}\Big)^2\ \diff{\hat\vth}{\theta}

</mrow><mrow>
       &amp;=\Big[\difftwo{r}{t}-r\ \Big(\diff{\theta}{t}\Big)^2\Big] \hat\vr
   +\Big[r\ \difftwo{\theta}{t} + 2 \diff{r}{t}\ \diff{\theta}{t}\Big]\hat\vth
</mrow>
</md>
</p></proof>

<example xml:id="eg_beadToss">
<p>
As an example, consider a bead that is sliding on a frictionless rod
that has one end fixed at the origin and that is rotating about the
origin at a constant <m>\Omega\,</m>rad/sec.
</p>

<sidebyside width="35%">
<image source="figs/beadRod"/>
</sidebyside>

<p>
Because the rod is frictionless,
it is incapable of applying to the bead any force parallel to the rod. So
under Newton's law, <m>m\va=\vF</m>, the radial<fn>The <m>\hat\vth</m> component
of the acceleration just tells us how much normal force the rod is applying
to the bead to keep it on the rod.</fn>
 component of the acceleration
of the particle is exactly zero. So, if the polar coordinates of the bead
at time <m>t</m> are <m>\big(r(t),\theta(t)\big)</m>, then,
by Lemma <xref ref="lem_polar"/>.c,
<me>
\difftwo{r}{t}-r\ \Big(\diff{\theta}{t}\Big)^2 = 0
</me>
As the rod is rotating at <m>\Omega\,</m>rad/sec,
<m>\diff{\theta}{t}=\Omega</m> and
<me>
\difftwo{r}{t}-\Omega^2\ r = 0
</me>
The general solution to this constant coefficient second order
ordinary differential equation is<fn>A review of the technique used to find this solution is given in Appendix <xref ref="ap_ODE"/>. In any event, it is easy to check that <m>r(t)=A e^{\Omega\,t} + B e^{-\Omega\,t}</m> really does obey
<m>\difftwo{r}{t}-\Omega^2\ r = 0</m>.</fn>
<me>
r(t)  = A e^{\Omega\,t} + B e^{-\Omega\,t}
</me>
where <m>A</m> and <m>B</m> are arbitrary constants that are determined by initial
conditions.
Just as an example, if <m>r(0)= 1</m> and <m>r'(0)= 0</m>,
then <m>A+B=1</m> and <m>A\Omega-B\Omega=0</m>, so that <m>A=B=\frac{1}{2}</m> and
<me>
r(t)  = \frac{1}{2}\big(e^{\Omega\,t}+e^{-\Omega\,t}\big)\qquad
</me>
If, again for example, <m>\theta(0) = 0</m>, then <m>\theta(t) = \Omega t</m>
and the bead follows the polar coordinate curve
<me>
r(\theta) = \frac{1}{2}\big(e^{\theta}+e^{-\theta}\big)
</me>
Observe that <m>r(\theta)</m> is <m>1</m> when <m>\theta=0</m>, increases as <m>\theta</m> increases, and tends to <m>\infty</m> as <m>\theta\rightarrow+\infty</m>. The curve is a spiral.
</p>

<sidebyside width="40%">
<image source="figs/beadCurve"/>
</sidebyside>
</example>

<example xml:id="eg_conicA"><title>Conic sections in polar coordinates</title>
<p>
In this example, we derive the equation of a general conic section in
polar coordinates. A conic section is the intersection of a plane with a cone.
This is illustrated in the figures below.
</p>

<sidebyside widths="20% 20% 20% 20%" valign="middle">
<image source="figs/conePlaneCircle"/>
<image source="figs/conePlaneEllipse"/>
<image source="figs/conePlaneParabola"/>
<image source="figs/conePlaneHyperbola"/>
</sidebyside>

<p>
For our current purposes, it is convenient to use the equivalent<fn>It is outside our scope to prove this equivalence.</fn> (and often used) definition that a conic section is the set of points <m>P</m>
in the <m>xy</m>-plane
<ul>
<li>
whose distance from a fixed point <m>F</m> (called the <em>focus</em> of the conic)
</li>
<li>
is a constant multiple <m>\veps\ge 0</m> (called the <em>eccentricity</em>
of the conic)
</li>
<li>
of the distance from <m>P</m> to a fixed line <m>L</m> (called the <em>directrix</em>
of the conic).
</li>
</ul>
Choose a coordinate system with the focus <m>F</m> of the conic being the origin
and with the directrix <m>L</m> being <m>x=p</m> for some <m>p \gt 0</m>.
</p>

<sidebyside width="33%">
<image source="figs/conic"/>
</sidebyside>

<p>
If <m>P</m> has polar coordinates <m>(r,\theta)</m>, then <m>P</m> has <m>x</m>-coordinate
<m>r\cos\theta</m>. The point <m>Q</m> on the line <m>L</m> in the figure above
has <m>x</m>-coordinate <m>p</m>.
So the distance from <m>P</m> to <m>L</m>, which is also the distance from <m>P</m> to
<m>Q</m>, is <m>p-r\cos\theta</m>.  The distance from <m>P</m> to <m>F</m> is <m>r</m>. We require that
the distance from <m>P</m> to <m>F</m> is <m>\veps</m> times the distance from <m>P</m> to <m>L</m>.
So
<me>
r=\veps\big(p-r\cos\theta\big)
\iff
r=\frac{\veps p}{1+\veps\cos\theta}
</me>
The numerator <m>\veps p</m> is usually renamed to <m>\ell</m> giving the equation
<me>
r=\frac{\ell}{1+\veps\cos\theta}
</me>
</p></example>

<example xml:id="conicB"><title>Conic sections in polar coordinates, again</title>
<p>
We'll now take the equation <m>r=\frac{\ell}{1+\veps\cos\theta}</m>
for a conic section in polar coordinates, from the last example,
and convert it to the more familiar Cartesian coordinates. Just by the
definition of polar coordinates
<md>
<mrow>
r\big(1+\veps\cos\theta\big)=\ell
&amp;\iff r = \ell -\veps x
</mrow><mrow>
&amp;\iff x^2+y^2 = \ell^2-2\veps\ell x+\veps^2 x^2
</mrow><mrow>
&amp;\iff (1-\veps^2) x^2  + 2\veps\ell x + y^2 = \ell^2
\tag{C}
</mrow>
</md>
Now consider separately four different cases, depending on the value of
<m>\veps \ge 0</m>.
<ul>
<li><p>
If <m>\veps=0</m>, (C) reduces to
</p>

<sidebyside widths="45% 30%" valign="middle">
<p><me>
x^2+y^2 = \ell^2
</me></p>
<image source="figs/conicCircle"/>
</sidebyside>
<p>
which is of course a circle of radius <m>\ell</m>.
</p>
</li>
<li>
<p>
If <m>0 \lt \veps \lt 1</m>, completing the square in (C)
gives
<me>
(1-\veps^2)\Big(x+\frac{\veps\ell}{1-\veps^2}\Big)^2 + y^2
   = \ell^2 + \frac{\veps^2\ell^2}{1-\veps^2}
   =  \frac{\ell^2}{1-\veps^2}
</me>
which is equivalent to
</p>

<sidebyside  widths="45% 40%" valign="middle">
<p>
  <me>
  \frac{\big(x+\frac{\veps\ell}{1-\veps^2}\big)^2}
                { \frac{\ell^2}{{(1-\veps^2)}^2}}
  +\frac{y^2}{\frac{\ell^2}{1-\veps^2}}
  =1
</me></p>
 <image source="figs/conicEllipse"/>
</sidebyside>

<p>
and is of course an ellipse with semi-major axis <m>r_M=\frac{\ell}{1-\veps^2}</m>
and semi-minor axis <m>r_m=\frac{\ell}{\sqrt{1-\veps^2}}</m>.
</p>
</li>
<li><p>
If <m>\veps=1</m>, (C) reduces to
</p>
<sidebyside widths="45% 33%" valign="middle">
<p><me>
y^2 = \ell^2-2\ell x
</me></p>
<image source="figs/conicParabola"/>
</sidebyside>
<p>
which is of course a parabola.
</p>
</li>
<li><p>
If <m>\veps \gt 1</m>, the same computation as in the <m>0 \lt \veps \lt 1</m> case
gives
</p>
<sidebyside widths="45% 33%" valign="middle">
  <p><me>
  \frac{\big(x-\frac{\veps\ell}{\veps^2-1}\big)^2}
                { \frac{\ell^2}{{(\veps^2-1)}^2}}
  -\frac{y^2}{\frac{\ell^2}{\veps^2-1}}
  =1
  </me></p>
  <image source="figs/conicHyperbola"/>
</sidebyside>
<p>
and is of course a hyperbola.
</p>
</li>
</ul>
</p>
</example>


<xi:include href="../problems/prob_s1.8.ptx" />

</section>
