<?xml version="1.0" encoding="UTF-8" ?>
<section xmlns:xi="http://www.w3.org/2001/XInclude" xml:id="sec_paramCircles">

<!-- Copyright 2018-2020 Joel Feldman, Andrew Rechnitzer and Elyse Yeager -->
<!-- This work is licensed under the Creative Commons Attribution-NonCommercial-ShareAlike 4.0 International License-->
<!-- https://creativecommons.org/licenses/by-nc-sa/4.0 -->

<title>Optional <mdash/> Parametrizing Circles</title>


<p>
We now discuss a simple strategy for parametrizing circles in three
dimensions, starting with the circle in the <m>xy</m>-plane that has radius <m>\rho</m>
and is centred on the origin. This is easy to parametrize:
</p>

<sidebyside widths="40% 50%" valign="middle">
  <image source="figs/circle1"/>
<p>
<md>
<mrow>
&amp;\vr(t)=\rho\cos t\,\hi+ \rho\sin t\,\hj
</mrow><mrow>
&amp;0\le t\lt 2\pi
</mrow>
</md>
</p>
</sidebyside>

<p>
Now let's move the circle so that its centre is at some general point
<m>\vc</m>. To parametrize this new circle, which still has radius <m>\rho</m> and which
is still parallel to the <m>xy</m>-plane, we just translate by <m>\vc</m>:
</p>

<sidebyside widths="36% 50%" valign="middle">
<image source="figs/circle2"/>
<p>
<md>
<mrow>
&amp;\vr(t)=\vc+\rho\cos t\,\hi+ \rho\sin t\,\hj
</mrow><mrow>
&amp; 0\le t\lt 2\pi
</mrow>
</md>
</p>
</sidebyside>

<p>
Finally, let's consider a circle in general position. The secret to
parametrizing a general circle is to replace <m>\hi</m> and <m>\hj</m> by two new vectors
<m>\hi'</m> and <m>\hj'</m> which
<ol label="a">
<li> are unit vectors,
</li>
<li> are parallel to the plane of the desired circle and
</li>
<li> are mutually perpendicular.
</li>
</ol>
</p>

<sidebyside widths="40% 50%" valign="middle">
  <image source="figs/circle3"/>
<p>
<md>
<mrow>
&amp;
\vr(t)=\vc+\rho\cos t\,\hi'+ \rho\sin t\,\hj'
</mrow><mrow>
&amp; 0\le t\lt 2\pi
</mrow>
</md></p>
</sidebyside>
<p>
To check that this is correct, observe that
<ul>
<li>
<m>\vr(t)-\vc</m> is parallel to the plane of the desired circle because
both <m>\hi'</m> and <m>\hj'</m> are parallel to the plane of the desired circle
and <m>\vr(t)-\vc=\rho\cos t\,\hi'+ \rho\sin t\,\hj'</m>
</li>
<li>
<m>\vr(t)-\vc</m> is of length <m>\rho</m> for all <m>t</m> because
<md>
<mrow>
|\vr(t)-\vc\,|^2
   &amp;=(\vr(t)-\vc\,)\cdot(\vr(t)-\vc\,)
</mrow><mrow>
   &amp;=(\rho\cos t\,\hi'+ \rho\sin t\,\hj')\cdot
          (\rho\cos t\,\hi'+ \rho\sin t\,\hj')
</mrow><mrow>
&amp;=\rho^2\cos^2 t\ \hi'\cdot\hi'
  + \rho^2\sin^2 t\ \hj'\cdot\hj'
  +2\rho\cos t\sin t\ \hi'\cdot\hj'
</mrow><mrow>
&amp;=\rho^2(\cos^2t+\sin^2t)=\rho^2
</mrow>
</md>
since <m>\hi'\cdot\hi'=\hj'\cdot\hj'=1</m> (<m>\hi'</m> and <m>\hj'</m> are both unit
vectors) and <m>\hi'\cdot\hj'=0</m> (<m>\hi'</m> and <m>\hj'</m> are perpendicular).
</li>
</ul>
To find such a parametrization in practice, we need to find the centre
<m>\vc</m> of the circle, the radius <m>\rho</m> of the circle and two mutually
perpendicular unit vectors, <m>\hi'</m> and <m>\hj'</m>, in the plane of the circle.
It is often easy to find at least one point <m>\vp</m> on the circle. Then
we can take <m>\hi'=\frac{\vp-\vc}{|\vp-\vc|}</m>. It is also often easy
to find a unit vector, <m>\hk'</m>, that is normal to the plane of the circle.
Then we can choose <m>\hj'=\hk'\times\hi'</m>. We'll illustrate this now.
</p>

<example xml:id="eg_paramCircleA">
<p>
Let <m>C</m> be the intersection of the sphere <m>x^2+y^2+z^2=4</m>
and the plane <m>z=y</m>.
<ul>
<li>
The intersection of any plane with any sphere is a
circle. The plane in question passes through the centre of the sphere,
so <m>C</m> has the same centre and same radius as the sphere.
So <m>C</m> has radius <m>2</m> and centre <m>(0,0,0)</m>.
</li>
<li>
Notice that the point <m>(2,0,0)</m> satisfies both <m>x^2+y^2+z^2=4</m> and <m>z=y</m> and so
is on <m>C</m>. We may choose <m>\hi'</m> to be the unit vector in the direction
from the centre <m>(0,0,0)</m> of the circle towards <m>(2,0,0)</m>. Namely <m>\hi'=(1,0,0)</m>.
</li>
<li>
Since the plane of the circle is <m>z-y=0</m>, the vector <m>\vnabla(z-y)=(0,-1,1)</m>
is perpendicular to the  plane of <m>C</m>. So we may take <m>\hk'=\frac{1}{\sqrt{2}}(0,-1,1)</m>.
</li>
<li>
Then <m>\hj'=\hk'\times\hi'
=\frac{1}{\sqrt{2}}(0,-1,1)\times(1,0,0)=\frac{1}{\sqrt{2}}(0,1,1)</m>.
</li>
</ul>
Substituting in <m>\vc=(0,0,0)</m>, <m>\rho=2</m>, <m>\hi'=(1,0,0)</m> and
<m>\hj'=\frac{1}{\sqrt{2}}(0,1,1)</m> gives
</p>

<sidebyside  widths="40% 50%" valign="middle">
<image source="figs/circle4"/>
<p><md>
<mrow>
\vr(t)&amp;=2\cos t\,(1,0,0)+ 2\sin t\,\frac{1}{\sqrt{2}}(0,1,1)
</mrow><mrow>
&amp;=2\big(\cos t, \frac{\sin t}{\sqrt{2}},\frac{\sin t}{\sqrt{2}}\big)
</mrow><mrow>
&amp; 0\le t\lt 2\pi
</mrow>
</md></p>
</sidebyside>

<p>
To check this, note that <m>x=2\cos t</m>, <m>y=\sqrt{2}\sin t</m>,
<m>z=\sqrt{2}\sin t</m> satisfies both <m>x^2+y^2+z^2=4</m> and <m>z=y</m>.
</p>

</example>

<example xml:id="eg_paramCircleBB">
<p>
Let <m>C</m> be the circle that passes through the three points
<m>(3,0,0)</m>, <m>(0,3,0)</m> and <m>(0,0,3)</m>.
<ul>
<li>
All three points obey <m>x+y+z=3</m>.
So the circle lies in the plane <m>x+y+z=3</m>. We guess, by symmetry,
or by looking at the figure below, that the centre of the circle is
at the centre of mass of the three points, which is <m>\frac{1}{3}[(3,0,0)+(0,3,0)+(0,0,3)]=(1,1,1)</m>.
We must check this and can do so by checking that <m>(1,1,1)</m> is
equidistant from the three points:
<md alignment="alignat">
<mrow>
\big|(3,0,0)-(1,1,1)\big|&amp;=\big|(2,-1,-1)\big|&amp;&amp;=\sqrt{6}
</mrow><mrow>
\big|(0,3,0)-(1,1,1)\big|&amp;=\big|(-1,2,-1)\big|&amp;&amp;=\sqrt{6}
</mrow><mrow>
\big|(0,0,3)-(1,1,1)\big|&amp;=\big|(-1,-1,2)\big|&amp;&amp;=\sqrt{6}
</mrow>
</md>
This tells us both that <m>(1,1,1)</m> is indeed the centre (as only the centre is equidistant from any three distinct points on a circle) and that
the radius of <m>C</m> is <m>\sqrt{6}</m>.
</li>
<li>
We may choose <m>\hi'</m> to be the unit vector in the direction from
the centre <m>(1,1,1)</m> of the circle towards <m>(3,0,0)</m>. Namely <m>\hi'=\frac{1}{\sqrt{6}}(2,-1,-1)</m>.
</li>
<li>
Since the plane of the circle is <m>x+y+z=3</m>, the vector
<m>\vnabla(x+y+z)=(1,1,1)</m> is perpendicular to the plane of <m>C</m>.
So we may take <m>\hk'=\frac{1}{\sqrt{3}}(1,1,1)</m>.
</li>
<li>
Then 
<md>
<mrow>
\hj'&amp;=\hk'\times\hi'
=\frac{1}{\sqrt{18}}(1,1,1)\times(2,-1,-1)=\frac{1}{\sqrt{18}}(0,3,-3)
</mrow><mrow>
&amp;
=\frac{1}{\sqrt{2}}(0,1,-1)
</mrow>
</md>
</li>
</ul>
Substituting in <m>\vc=(1,1,1)</m>, <m>\rho=\sqrt{6}</m>, <m>\hi'=\frac{1}{\sqrt{6}}(2,-1,-1)</m>
and  <m>\hj'=\frac{1}{\sqrt{2}}(0,1,-1)</m> gives
<md>
<mrow>
\vr(t)&amp;=(1,1,1)+\sqrt{6}\cos t\,\frac{1}{\sqrt{6}}(2,-1,-1)
        + \sqrt{6}\sin t\,\frac{1}{\sqrt{2}}(0,1,-1)\cr
&amp;=\big(1+2\cos t, 1-\cos t+\sqrt{3}\sin t,1-\cos t-\sqrt{3}\sin t\big)
</mrow>
</md>
</p>

<sidebyside width="40%">
  <image source="figs/circle5"/>
</sidebyside>

<p>
To check this, note that <m>\vr(0)=(3,0,0)</m>,
<m>\vr\big(\frac{2\pi}{3}\big)=(0,3,0)</m>
and <m>\vr\big(\frac{4\pi}{3}\big)=(0,0,3)</m> since
<m>\cos\frac{2\pi}{3}=\cos\frac{4\pi}{3}=-\frac{1}{2}</m>,
<m>\sin\frac{2\pi}{3}=\frac{\sqrt{3}}{2}</m> and
<m>\sin\frac{4\pi}{3}=-\frac{\sqrt{3}}{2}</m>.
</p>

</example>

<!-- <xi:include href="../problems/prob_s1.12.ptx" /> -->

</section>
