<?xml version="1.0" encoding="UTF-8" ?>
<section xmlns:xi="http://www.w3.org/2001/XInclude" xml:id="sec_curve_derivs">

<!-- Copyright 2018-2020 Joel Feldman, Andrew Rechnitzer and Elyse Yeager -->
<!-- This work is licensed under the Creative Commons Attribution-NonCommercial-ShareAlike 4.0 International License-->
<!-- https://creativecommons.org/licenses/by-nc-sa/4.0 -->

<title>Derivatives, Velocity, Etc.</title>



<p>This being a Calculus text, one of our main operations is differentiation.
We are now interested in parametrizations <m>\vr(t)</m>.
It is very easy and natural to extend our definition of derivative to <m>\vr(t)</m>
as follows.
</p>

<definition xml:id="def__curve_deriv">
<statement><p>
The derivative of the vector valued function <m>\vr(t)</m> is defined to be
</p>

<sidebyside widths="50% 35%" valign="middle">
<p>
<me>
\vr'(t) =  \diff{\vr}{t}(t)=\lim_{h\rightarrow 0}\frac{\vr(t+h)-\vr(t)}{h}
</me>
</p>
<image source="figs/parCurveDerivA"/>
</sidebyside>

<p>
when the limit exists. In particular, if
<m>\vr(t)=\big(x(t)\,,\,y(t)\,,\,z(t)\big)</m>, then
<me>
\vr'(t)=\big(x'(t)\,,\,y'(t)\,,\,z'(t)\big)
</me>
That is, to differentiate a vector valued function of <m>t</m>, just differentiate
each of its components.
</p></statement>
</definition>


<p>And of course differentiation interacts with arithmetic operations,
like addition, in the obvious way. Only a little more thought is required to
see that differentiation interacts quite nicely with dot and cross
products too.
</p>

<theorem xml:id="thm_DIFFalgebra"><title>Arithmetic of differentiation</title>
<statement><p>
Let
<ul>
<li>
<m>\va(t),\vb(t)</m> be vector valued differentiable functions of <m>t\in\bbbr</m>
that take values in <m>\bbbr^n</m> and
</li>
<li>
 <m>\alpha,\beta \in \mathbb{R}</m> be constants and
</li>
<li>
 <m>\ga(t)</m> and <m>s(t)</m> be real valued differentiable functions of <m>t\in\bbbr</m>
</li>
</ul>
Then
<md alignment="alignat">
<mrow>
&amp;\text{(a)}\quad &amp;&amp;\diff{}{t}\big[\alpha\,\va(t)+\beta\,\vb(t)\big]
         =\alpha\,\va'(t)+\beta\,\vb'(t)
           &amp;&amp;\text{(linear combination)}
</mrow><mrow>
&amp;\text{(b)} &amp;&amp;\diff{}{t}\big[\ga(t)\vb(t)\big]
         =\ga'(t)\vb(t)+\ga(t)\vb'(t)
           &amp;&amp;\text{(multiplication by scalar function)}

</mrow><mrow>
&amp;\text{(c)} &amp;&amp;\diff{}{t}\big[\va(t)\cdot\vb(t)\big]
         =\va'(t)\cdot\vb(t)+\va(t)\cdot\vb'(t)
           &amp;&amp;\text{(dot product)}

</mrow><mrow>
&amp;\text{(d)} &amp;&amp;\diff{}{t}\big[\va(t)\times\vb(t)\big]
         =\va'(t)\times\vb(t)+\va(t)\times\vb'(t)
           \ \ &amp;&amp;\text{(cross product)}
</mrow><mrow>
&amp;\text{(e)} &amp;&amp;\diff{}{t}\big[\va\big(s(t)\big)\big]
         =\va'\big(s(t)\big)\,s'(t)
           &amp;&amp;\text{(composition)}
</mrow>
</md>
</p>

</statement>
</theorem>


<p>Let's think about the geometric significance of <m>\vr'(t)</m>.
In particular, let's think about the relationship between <m>\vr'(t)</m>
and distances along the curve.
The derivative <m>\vr'(t)</m> is the limit of   <m>\frac{\vr(t+h)-\vr(t)}{h}</m> as <m>h\rightarrow 0</m>.
The numerator, <m>\vr(t+h)-\vr(t)</m>, is the vector with head at <m>\vr(t+h)</m>
and tail at <m>\vr(t)</m>.
</p>

<sidebyside width="50%">
<image source="figs/parCurveDeriv"/>
</sidebyside>

<p>
  When <m>h</m> is very small this vector
<ul>
<li>
has the essentially the same direction as the tangent vector to the curve at <m>\vr(t)</m> and
</li>
<li>
has length being essentially the length of the part of the curve between
<m>\vr(t)</m> and <m>\vr(t+h)</m>.
</li>
</ul>
Taking the limit as <m>h\rightarrow 0</m> yields that
<ul>
<li>
<m>\vr'(t)</m> is a tangent vector to the curve at <m>\vr(t)</m> that points in
the direction of increasing <m>t</m> and
</li>
<li>
if <m>s(t)</m> is the length of the part of the curve between
<m>\vr(0)</m> and <m>\vr(t)</m>, then  <m>\diff{s}{t}(t)=\big|\diff{\vr}{t}(t)\big|</m>.
</li>
</ul>
This is worth stating formally.
</p>

<lemma xml:id="lem_CVtanArclen">
<statement><p>
Let <m>\vr(t)</m> be a parametrized curve.
<ol label="a">
<li>
Denote by <m>\hat\vT(t)</m> the unit tangent vector to the curve
at <m>\vr(t)</m> pointing in the direction of increasing <m>t</m>. If
<m>\vr'(t)\ne 0</m>
then
<me>
\hat\vT(t) = \frac{\vr'(t)}{|\vr'(t)|}
</me>
</li>
<li><p>
Denote by <m>s(t)</m> the length of the part of the curve between
<m>\vr(0)</m> and <m>\vr(t)</m>.Then
</p>

<sidebyside widths="50% 45%" valign="middle">
<p><md>
<mrow>
\diff{s}{t}(t)&amp;=\Big|\diff{\vr}{t}(t)\Big|
</mrow><mrow>
s(T)-s(T_0)&amp;= \int_{T_0}^T \left|\diff{\vr}{t}(t)\right|\,\dee{t}
</mrow>
</md></p>
  <image source="figs/parCurveDerivB"/>
</sidebyside>
</li>
<li>
In particular, if the parameter happens to be arc length, i.e. if <m>t=s</m>,
so that <m>\diff{s}{s}=1</m>, then
<me>
\left|\diff{\vr}{s}(s)\right|=1\qquad
\hat\vT(s) = \vr'(s)
</me>
</li>
</ol>
</p></statement>
</lemma>

<p>As an application, we have the
</p>

<lemma xml:id="lem_CVvelocityEtc">
<statement><p>
If <m>\vr(t)=\big(x(t)\,,\,y(t)\,,\,z(t)\big)</m> is the position of a
particle at time <m>t</m>, then
<md>
<mrow>
\text{position at time } t
       &amp;=\vr(t)=\big(x(t)\,,\,y(t)\,,\,z(t)\big)
</mrow><mrow>
\text{velocity at time } t
       &amp;=\vv(t)=\vr'(t)=\big(x'(t)\,,\,y'(t)\,,\,z'(t)\big)
        = \diff{s}{t}(t)\,\hat\vT(t)
</mrow><mrow>
\text{speed at time } t
       &amp;= \diff{s}{t}(t)=|\vv(t)|=|\vr'(t)|=\sqrt{(x'(t)^2+y'(t)^2+z'(t)^2}
</mrow><mrow>
\text{acceleration at time } t
       &amp;=\va(t)=\vr'(t)=\vv'(t)=\big(x''(t)\,,\,y''(t)\,,\,z''(t)\big)
</mrow><mrow>
</mrow>
<intertext>and the distance travelled between times <m>T_0</m> and <m>T</m> is</intertext><mrow>
  s(T)-s(T_0)&amp;= \int_{T_0}^T \Big|\diff{\vr}{t}(t)\Big|\,\dee{t}
       = \int_{T_0}^T \sqrt{(x'(t)^2+y'(t)^2+z'(t)^2}\,\dee{t}
</mrow>
</md>
</p></statement>
</lemma>

<p>
Note that the velocity <m>\vv(t) = \vr'(t)</m> is a vector quantity while the
speed <m>\diff{s}{t}(t)=|\vr'(t)|</m> is a scalar quantity.
</p>

<example xml:id="eg_paramCircleTan">
<p>
In general it can be quite difficult to compute arc lengths.
So, as an easy warmup example, we will compute the circumference of the circle
<m>x^2+y^2=a^2</m>. We'll also find a unit tangent to the circle at any point on
the circle. We'll use the parametrization
<me>
\vr(\theta) = \big(a\cos\theta\,,\,a\sin\theta\big)\qquad
0\le \theta\le 2\pi
</me>
of Example <xref ref="eg_paramCircle"/>. Using Lemma <xref ref="lem_CVtanArclen"/>,
but with the parameter <m>t</m> renamed to <m>\theta</m>
<md>
<mrow>
\vr'(\theta) &amp;= a\big(-\sin\theta\,,\cos\theta\big)
</mrow><mrow>
\hat\vT(\theta) &amp;= \frac{\vr'(\theta)}{|\vr'(\theta)|}
               =  \big(-\sin\theta\,,\cos\theta\big)
</mrow><mrow>
\diff{s}{\theta}(\theta)&amp;=\big|\vr'(\theta)\big| = a
</mrow><mrow>
s(\Theta)-s(0)&amp;= \int_{0}^\Theta \big|\vr'(\theta)\big|\,\dee{\theta}
          =a\Theta
</mrow>
</md>
As<fn>You might guess that <m>\Theta</m> is a capital Greek theta. You'd be right.</fn>
 <m>s(\Theta)</m> is the arc length of the part of the circle with
<m>0\le\theta\le\Theta</m>, the circumference of the whole circle is
<me>
s(2\pi) = 2\pi a
</me>
which is reassuring, since this formula has been known<fn>The earliest known written approximations of <m>\pi</m>, in Egypt and Babylon, date
from 1900--1600BC. The first recorded algorithm for rigorously evaluating <m>\pi</m>
was developed by Archimedes around 250 BC. The first use of the symbol <m>\pi</m>,
for the ratio between the circumference of a circle and its diameter,
in print was in 1706 by William Jones.</fn>
for thousands of years.
</p>

<sidebyside width="66%">
<image source="figs/parCircleT"/>
</sidebyside>

<p>
The formula <m>s(\Theta)-s(0)=a\Theta</m> also makes sense <mdash/> the part of the
circle with <m>0\le\theta\le\Theta</m> is the fraction <m>\frac{\Theta}{2\pi}</m>
of the whole circle, and so should have length <m>\frac{\Theta}{2\pi}\times
2\pi a</m>. Also note that
<me>
\vr(\theta)\cdot\hat\vT(\theta) = \big(a\cos\theta\,,\,a\sin\theta\big)
\cdot \big(-\sin\theta\,,\cos\theta\big)
=0
</me>
so that the tangent to the circle at any point is perpendicular
to the radius vector of the circle at that point. This is another geometric fact
that has been known<fn>It is Proposition 18 in Book 3 of Euclid's Elements. It was published around 300BC.</fn>
 for thousands of years.
</p></example>

<example xml:id="eg_paramHelix">
<p>
Consider the curve
<me>
\vr(t) = 6\sin(2t)\hi + 6\cos(2t)\hj +5t\hk
</me>
where the standard basis vectors <m>\hi = (1,0,0)</m>, <m>\hj=(0,1,0)</m>
and <m>\hk =(0,0,1)</m>.
We'll first sketch it, by observing that
<ul>
<li> <m>x(t)=6\sin(2t)</m> and <m>y(t) =6\cos(2t)</m> obey
<m>x(t)^2+y(t)^2 = 36 \sin^2(2t) + 36\cos^2(2t) = 36</m>. So all points of the
curve lie on the cylinder <m>x^2+y^2=36</m> and
</li>
<li> as <m>t</m> increases, <m>\big(x(t),y(t)\big)</m> runs clockwise
around the circle <m>x^2+y^2=36</m> and at the same time <m>z(t) = 5t</m>
just increases linearly.
</li>
</ul>
Our curve is the helix
</p>

<sidebyside width="45%">
<image source="figs/helix4"/>
</sidebyside>

<p>
We have marked three points of the curve on the above sketch. The first has
<m>t=0</m> and is <m>0\hi+6\hj+0\hk</m>. The second has <m>t=\frac{\pi}{2}</m> and is <m>0\hi-6\hj+\frac{5\pi}{2}\hk</m>, and the third has <m>t=\pi</m> and is
<m>0\hi+6\hj+5\pi\hk</m>.
We'll now use Lemma <xref ref="lem_CVtanArclen"/> to find a unit tangent
<m>\hat\vT(t)</m> to the curve at <m>\vr(t)</m> and also the arclength of the part of curve between <m>t=0</m> and <m>t=\pi</m>.
<md>
<mrow>
\vr(t) &amp;= 6\sin(2t)\hi + 6\cos(2t)\hj +5t\hk
</mrow><mrow>
\vr'(t) &amp;= 12\cos(2t)\hi -12\sin(2t)\hj +5\hk
</mrow><mrow>
\diff{s}{t}(t)&amp;=\big|\vr'(t)\big|
=\sqrt{12^2\cos^2(2t) +12^2\sin^2(2t)+5^2}
= \sqrt{12^2+5^2}
</mrow><mrow>
&amp;= 13
</mrow><mrow>
\hat\vT(t) &amp;= \frac{\vr'(t)}{|\vr'(t))|}
               =  \frac{12}{13}\cos(2t)\hi -\frac{12}{13}\sin(2t)\hj +\frac{5}{13}\hk
</mrow><mrow>
s(\pi)-s(0)&amp;= \int_{0}^\pi \big|\vr'(t)\big|\,\dee{t}
          =13\pi
</mrow>
</md>
</p></example>

<example xml:id="eg_astroid">
<p>
In this example, we find the perimeter of the astroid<fn>
Astroid should not be confused with asteroid, though both words derive
from the Greek word for star.</fn>
<me>
x^{2/3}+y^{2/3} = a^{2/3}
</me>
A geometric construction of this curve, as well as a derivation of its equation is given in the optional section <xref ref="sec_astroid"/> later.  We'll start by finding a convenient
parametrization.
<ul>
<li>
To do so, notice that <m>x^{2/3}+y^{2/3} = a^{2/3}</m> looks somewhat like the
equation of the circle <m>x^2+y^2=a^2</m>.
</li>
<li>
The standard parametrization of the circle, namely
<m>x=a\cos t</m>, <m>y=a \sin t</m> works because of the elementary trig identity <m>\cos^2t+\sin^2t=1</m>.
</li>
<li>
If we can arrange that <m>x(t)^{2/3} = a^{2/3}\cos^2 t</m> and <m>y(t)^{2/3}=a^{2/3}\sin^2 t</m>, then the same elementary trig identity will give <m>x(t)^{2/3}+y(t)^{2/3} = a^{2/3}</m>, as desired.
</li>
<li>
But
of course its easy to arrange that: just solve  <m>x(t)^{2/3} = a^{2/3}\cos^2 t</m> for <m>x(t)</m>,
namely <m>x(t) = a\cos^3t</m>, and solve <m>y(t)^{2/3}=a^{2/3}\sin^2 t</m> for <m>y(t)</m>,
namely <m>y(t)=a\sin^3 t</m>.
</li>
</ul>
Our parametrization is
<me>
\vr(t) = a\cos^3t\hi + a\sin^3 t\hj
</me>
By Lemma <xref ref="lem_CVtanArclen"/>
<md>
<mrow>
\vr(t) &amp;= a\cos^3t\hi + a\sin^3 t\hj
</mrow><mrow>
\vr'(t) &amp;= -3a\sin t\cos^2t\hi + 3a\sin^2 t\cos t\hj
</mrow><mrow>
\diff{s}{t}(t)&amp;=\big|\vr'(t)\big|
= \sqrt{9a^2\sin^2t\cos^4t + 9a^2\sin^4t\cos^2t}
</mrow><mrow>
&amp; = 3a \sqrt{\sin^2t\cos^2t(\cos^2t+\sin^2t)}
</mrow><mrow>
 &amp;=3a\big|\sin t\cos t\big|
</mrow><mrow>
\hat\vT(t) &amp;= \frac{\vr'(t)}{|\vr'(t))|}
=  \frac{\sin t\cos t}{|\sin t\cos t|}\ \big(-\cos t\hi+\sin t\hj\big)

</mrow><mrow>
 &amp;=  \sgn\!\big(\!\sin t\cos t\big)\ \big(-\cos t\hi+\sin t\hj\big)
</mrow>
</md>
Here <m>\sgn\!\big(\!\sin t\cos t\big)</m> means <q>the sign of <m>\sin t\cos t</m></q>, i.e <m>+1</m> when <m>\sin t\cos t \gt 0</m> and <m>-1</m> when <m>\sin t\cos t \lt 0</m>. So
<md>
<mrow>
&amp;\hat\vT(t)
</mrow><mrow>
 &amp;=\left.\begin{cases}1&amp;\text{if } \sin t \gt 0,\ \cos t \gt 0
                              \text{ or } \sin t \lt 0,\ \cos t \lt 0
</mrow><mrow>
                           -1&amp;\text{if } \sin t \gt 0,\ \cos t \lt 0
                              \text{ or } \sin t \lt 0,\ \cos t \gt 0
                \end{cases}\right\}\big(-\cos t\hi+\sin t\hj\big)
</mrow><mrow>
 &amp;=\left.\begin{cases}1&amp;\text{if } 0 \lt  t \lt \frac{\pi}{2}
                                            \text{ or }  \pi \lt  t \lt \frac{3\pi}{2}
</mrow><mrow>
                           -1&amp;\text{if }  \frac{\pi}{2} \lt t \lt \pi
                                          \text{ or }  \frac{3\pi}{2} \lt t \lt 2\pi
                \end{cases}\right\}\big(-\cos t\hi+\sin t\hj\big)
</mrow>
</md>
</p>

<p>Before we go on to sketch the astroid and compute its perimeter, we can
make a few observations that will simplify our lives.
<ul>
<li><p>
The signs of both components
of <m>\vr(t)</m> are the same as the signs of the components of
<m>\cos t\,\hi +\sin t\,\hj</m>; and the signs of both components
of <m>\vr'(t)</m> are the same as the signs of the components of
<m>-\sin t\,\hi +\cos t\,\hj</m>.
Consequently the astroid looks somewhat like a circle in that
<ul>
<li>
when <m>0\le t\le \frac{\pi}{2}</m>, <m>\vr(t)</m> lies in the first quadrant
and moves upward and to the left as <m>t</m> increases and
</li>
<li>
when <m>\frac{\pi}{2}\le t\le \pi</m>, <m>\vr(t)</m> lies in the second
quadrant and moves downward and to the left as <m>t</m> increases and
</li>
<li>
when <m>\pi\le t\le \frac{3\pi}{2}</m>, <m>\vr(t)</m> lies in the third quadrant
and moves downward and to the right as <m>t</m> increases and
</li>
<li>
when <m>\frac{3\pi}{2}\le t\le 2\pi</m>, <m>\vr(t)</m> lies in the fourth
quadrant and moves upward and to the right as <m>t</m> increases and
</li>
<li>
<m>\vr(2\pi)=\vr(0)</m> so that the astroid is a closed curve that
circumnavigates the origin exactly once as <m>t</m> runs from <m>0</m> to <m>2\pi</m>.
</li>
</ul></p>
</li>
<li>
  <p>
Something weird happens at those values of <m>t</m> where <m>\sin t\cos t</m> changes sign<fn>Like a cross-walk sign.</fn>,
i.e. at <m>t=0</m>, <m>\frac{\pi}{2}</m>, <m>\pi</m>, <m>\frac{3\pi}{2}</m>, etc. Namely <m>\hat T(t)</m>
flips. To be precise
<md>
<mrow>
\lim_{t\rightarrow 0-}\hat T(t) &amp;= \hi &amp;
\lim_{t\rightarrow 0+}\hat T(t) &amp;= -\hi
</mrow><mrow>
\lim_{t\rightarrow \pi/2-}\hat T(t) &amp;= \hj &amp;
\lim_{t\rightarrow \pi/2+}\hat T(t) &amp;= -\hj
</mrow>
</md>
and so on. This signals cusps in the curve at <m>t=0</m>, i.e. at <m>\vr(0) = a\hi</m>,
and at <m>t=\frac{\pi}{2}</m>, i.e. at <m>\vr(\frac{\pi}{2}) = a\hj</m>, and so on. So
while the astroid looks somewhat like a circle, it has cusps at <m>\pm a\hi</m> and <m>\pm a\hj</m>. Here is the sketch.
</p>

<sidebyside width="60%">
<image source="figs/astroid4"/>
</sidebyside>
</li>
<li> The astroid is invariant under reflections in the <m>x</m>-axis and in the
<m>y</m>-axis. That is, <m>x^{2/3}+y^{2/3} = a^{2/3}</m> is invariant under <m>x\rightarrow -x</m>
and also under <m>y\rightarrow -y</m>. So to find the whole perimeter, it suffices to find the
arc length of the part of the astroid in the first quadrant, and then multiply by <m>4</m>.
<md>
<mrow>
\text{perimeter}
&amp;=4\int_0^{\pi/2}\diff{s}{t}\ \dee{t}
 = 4\int_0^{\pi/2}3a\sin t\cos t\ \dee{t}
</mrow><mrow>
 &amp; = 6a\int_0^{\pi/2}\sin(2t)\ \dee{t}
=6a\Big[-\frac{\cos(2t)}{2}\Big]_0^{\pi/2}
</mrow><mrow>
 &amp;=6a
</mrow>
</md>
</li>
</ul>
</p>

</example>


<example xml:id="eg_zeroSpeed">
<p>
In the last example, we found that the astroid  had
cusps at those points <m>\vr(t)</m> where the velocity <m>\vr'(t)</m> vanished.
In this example, we will explore a little further what can happen when
<m>\vr'(t)=\vZero</m>.
</p>

<p>Suppose that you are out for a walk and that your position
at time <m>t</m> is <m>\vr(t)</m>. If at some time you have nonzero velocity,
it is very hard for you to  change your direction of motion
discontinuously<fn>For your velocity to jump
discontinuously, your acceleration has to be infinite, which requires an
infinite force. You might not look so healthy afterwards</fn>. On the other hand, when
<m>\vr'(t)=0</m>, you are not moving at all and it is easy for you to turn and
leave in any direction you choose. You could reverse direction completely,
or make a sharp left turn, or not change direction at all. Here are examples
of all of these. They all have <m>\vr'(t)=0</m>. They are sketched below.
<md alignment="alignat">
<mrow>
\vr_1(t) &amp;= (t^5, t^2) &amp;
\vr_1'(t)&amp;= (5t^4, 2t)
</mrow><mrow>
\vr_2(t) &amp;= \left.\begin{cases} (t^2, 0) &amp; \text{if }  t\le 0 \\
                        (0 , t^2) &amp; \text{if } t\ge 0
          \end{cases}\right\}\qquad &amp;
\vr_2'(t)&amp;= \left.\begin{cases} (2t, 0) &amp; \text{if }  t\le 0 \\
                        (0 , 2t) &amp; \text{if } t\ge 0
          \end{cases} \right\}
</mrow><mrow>
\vr_3(t) &amp;= (t^3, 0) &amp;
\vr_3'(t) &amp;= (3t^2, 0)
</mrow>
</md>
</p>

<sidebyside widths="30% 18% 23%" valign="middle">
<image source="figs/cuspA"/>
<image source="figs/cuspB"/>
<image source="figs/nocusp"/>
</sidebyside>

</example>

<example xml:id="eg_corkscrew">
<p>
We'll find the arc length of
<me>
\vr(t) = t\cos t\,\hi + t\sin t\,\hj +t\,\hk\qquad
0\le t\le\sqrt{2}
</me>
We'll first sketch it, by observing that
<ul>
<li> <m>x(t)=t\cos t </m>, <m>y(t) =t\sin t </m> and <m>z(t)=t</m> obey
<m>x(t)^2+y(t)^2 = t^2 = z(t)^2</m>. So all points of the
curve lie on the cone <m>x^2+y^2=z^2</m> and
</li>
<li> as <m>t</m> increases, <m>\big(x(t),y(t)\big)</m> runs
counterclockwise around a <q>circle</q> whose radius increases linearly with <m>t</m>
and at the same time <m>z(t)</m>  also increases linearly.
</li>
</ul>
Our curve is the <q>corkscrew</q>
</p>

<sidebyside width="60%">
<image source="figs/corkscrew"/>
</sidebyside>

<p>
By Lemma <xref ref="lem_CVtanArclen"/>
<md>
<mrow>
\vr(t) &amp;= t\cos t\,\hi + t\sin t\,\hj +t\,\hk
</mrow><mrow>
\vr'(t) &amp;= [\cos t -t\sin t ]\hi +[\sin t+t\cos t]\hj + \hk
</mrow>
</md>
so that
<md>
<mrow>
&amp;\diff{s}{t}(t)=\big|\vr'(t)\big|
</mrow><mrow>
&amp;= \sqrt{\big(\cos^2t\!-\!2 t\sin t\cos t\!+\!t^2\sin^2 t\big)
             \!+\!\big(\sin^2t\!+\!2 t\sin t\cos t \!+\!t^2\cos^2 t\big)\!+\!1}
</mrow><mrow>
&amp;=\sqrt{2+t^2}
</mrow>
</md>
Our goal, stated at the beginning of this example, was to compute
<me>
s(\sqrt{2})-s(0)= \int_{0}^{\sqrt{2}} \big|\vr'(t)\big|\,\dee{t}
          = \int_{0}^{\sqrt{2}} \sqrt{2+t^2}\,\dee{t}
</me>
To evaluate the integral, we'll use three techniques that you learned
in your first integral calculus course. First,  motivated by the
<m>\sqrt{2+t^2}</m>,  we'll use the trigonometric substitution
<me>
t=\sqrt{2}\tan u\qquad
\dee{t} =\sqrt{2}\sec^2 u\,\dee{u}\qquad
2+t^2=2\big[1+\tan^2u\big]=2\sec^2 u
</me>
When <m>t=0</m>, <m>u=0</m> and when <m>t=\sqrt{2}</m>, <m>\tan u=1</m> so that <m>u=\frac{\pi}{4}</m>
and
<md>
<mrow>
s(\sqrt{2})-s(0)&amp;= \int_{0}^{\pi/4} \sqrt{2\sec^2u}\,\sqrt{2}\sec^2 u\,\dee{u}
= 2\int_{0}^{\pi/4} \sec^3 u\,\dee{u}
</mrow>
</md>
You may have evaluated this integral in first year. There are several ways of doing so. Perhaps the most straight forward, but also most tedious,
method is to rewrite the integral as
<me>
s(\sqrt{2})-s(0)= 2\int_{0}^{\pi/4} \frac{\cos u}{\cos^4 u}\,\dee{u}
</me>
We recognize that this is a trigonometric integral that contains an odd power
of <m>\cos u</m>, so we substitute <m>w=\sin u</m>, <m>\dee{w}=\cos u\,\dee{u}</m>,
<m>\cos^2 u= 1-w^2</m>. When <m>u=0</m>, <m>w=0</m> and when <m>u=\frac{\pi}{4}</m>,
<m>w=\frac{1}{\sqrt{2}}</m> so that
<me>
s(\sqrt{2})-s(0)= 2\int_{0}^{1/\sqrt{2}}  \frac{\dee{w}}{{(1-w^2)}^2}
</me>
The integrand is now a rational function, i.e. a ratio of polynomials.
So we apply partial fractions.
<md>
<mrow>
s(\sqrt{2})-s(0)
&amp;= 2\int_{0}^{1/\sqrt{2}}  \frac{\dee{w}}{{[(1-w)(1+w)]}^2}
</mrow><mrow>
&amp;= \frac{1}{2}\int_{0}^{1/\sqrt{2}}
        \Big[\frac{1}{1-w}+\frac{1}{1+w}\Big]^2 \dee{w}
</mrow><mrow>
&amp;= \frac{1}{2}\int_{0}^{1/\sqrt{2}}
        \Big[\frac{1}{(1-w)^2}+\frac{2}{(1-w)(1+w)}+\frac{1}{(1+w)^2}\Big]
          \dee{w}
</mrow><mrow>
&amp;= \frac{1}{2}\int_{0}^{1/\sqrt{2}}
        \Big[\frac{1}{(1-w)^2}+\frac{1}{1-w}+\frac{1}{1+w}
             +\frac{1}{(1+w)^2}\Big]  \dee{w}
</mrow><mrow>
&amp;= \frac{1}{2}
        \Big[\frac{1}{1-w}-\ln|1-w|+\ln|1+w|
             -\frac{1}{1+w}\Big]_{0}^{1/\sqrt{2}}
</mrow><mrow>
&amp;= \frac{1}{2}
        \Big[\frac{2w}{1-w^2}+\ln\frac{1+w}{1-w}\Big]_{0}^{1/\sqrt{2}}
= \frac{1}{2}
        \Big[2\sqrt{2}+\ln\frac{\sqrt{2}+1}{\sqrt{2}-1}\Big]
</mrow><mrow>
&amp;\approx 2.2956
</mrow>
</md>
Ooof!
</p></example>


<!-- <xi:include href="../problems/prob_s1.1.ptx" /> -->

</section>
