<?xml version="1.0" encoding="UTF-8" ?>
<section xmlns:xi="http://www.w3.org/2001/XInclude" xml:id="sec_unified">

<!-- Copyright 2018-2020 Joel Feldman, Andrew Rechnitzer and Elyse Yeager -->
<!-- This work is licensed under the Creative Commons Attribution-NonCommercial-ShareAlike 4.0 International License-->
<!-- https://creativecommons.org/licenses/by-nc-sa/4.0 -->

<title>Optional <mdash/> A Generalized Stokes' Theorem</title>


<p>As we have seen, the fundamental theorem of calculus,
the divergence theorem, Greens' theorem and Stokes' theorem
share a number of common features. There is in fact a single framework
which encompasses and generalizes all of them, and there is a
single theorem of which they are all special cases. We now give a
bare bones introduction to this framework and theorem. A proper
treatment typically takes up a good part of a full course.
Here is an outline of what we shall do:
<ul>
<li>
First, we will define <term>differential forms</term>. To try and keep
things as simple and concrete as possible, we'll only define<fn>In  general, a differential form is defined on a <term>manifold</term>, which is
an abstract generalization of a multi-dimensional surface, like a sphere or a torus.</fn>
differential forms on <m>\bbbr^3</m> <mdash/> all of our functions will be defined on
<m>\bbbr^3</m>. Very roughly
speaking, a <m>k</m>-form is what you write after the integral sign of
an integral over a <m>k</m> dimensional object. Here <m>k</m> is one of <m>0</m>, <m>1</m>,
<m>2</m>, <m>3</m>.  As a example, a <m>1</m>-form is an expression of the
form <m>F_1(x,y,z)\,\dee{x}
 + F_2(x,y,z)\,\dee{y}
 + F_3(x,y,z)\,\dee{z}</m>. For <m>k=0</m>, think of a point as a zero
dimensional object and think of evaluating a function at a point
as <q>integrating the function over the point</q>.
</li>
<li>
<p>
Then we will define some operations on differential forms, so that
we can add them, multiply them, differentiate them and, eventually,
integrate them.  The derivative of
a <m>k</m>-form <m>\om</m> is a <m>(k+1)</m>-form that is denoted <m>\dee{\om}</m>.
It will turn out that
<ul>
<li>
differentiating a <m>0</m>-form amounts to taking a gradient,
</li>
<li>
differentiating a <m>1</m>-form amounts to taking a curl, and
</li>
<li>
differentiating a <m>2</m>-form amounts to taking a divergence.
</li>
</ul>
</p>
</li>
<li><p>
Finally we will get to the generalized Stokes' theorem which says that,
if <m>\om</m> is a <m>k</m>-form (with <m>k=0,1,2</m>) and <m>D</m> is a <m>(k+1)</m>-dimensional
domain of integration, then
<me>
\int_D d\om=\int_{\partial D}\om
</me>
It will turn out that
<ul>
<li>
when <m>k=0</m>, this is just the fundamental theorem of calculus and
</li>
<li>
when <m>k=1</m>, this is both Green's theorem and our Stokes' theorem, and
</li>
<li>
when <m>k=2</m>, this is the divergence theorem.
</li>
</ul></p>
</li>
</ul>
</p>

<p>Now let's get to work. For simplicity, we will assume throughout this
section that all derivatives of all functions exist and are continuous.
Our first task to define differential forms.
</p>

<p>As we said above we will define a 1-form as an expression of the form
<m>F_1(x,y,z)\,\dee{x}
 + F_2(x,y,z)\,\dee{y}
 + F_3(x,y,z)\,\dee{z}</m>. When you learned the definition of the
integral the symbol <q><m>\dee{x}</m></q> was not given any mathematical
meaning by itself. A meaning was given only to collections of symbols like the indefinite integral <q><m>\int f(x)\ \dee{x}</m></q> and the definite integral
<q><m>\int_a^b f(x)\ \dee{x}</m></q>.
Later in this section, we will give a meaning
to <m>\dee{x}</m>. We will, in Definition <xref ref="def_differentialFormDiff"/>,
define a differentiation operator that we will call <m>\dee{}</m>. Then <m>\dee{x}</m>
will be that differentiation operator applied to the function <m>f(x)=x</m>.
However, until then we will have to treat <m>\dee{x}</m> and <m>\dee{y}</m> and
<m>\dee{z}</m> just as symbols. Their sole role in
<m>F_1(x,y,z)\,\dee{x}
 + F_2(x,y,z)\,\dee{y}
 + F_3(x,y,z)\,\dee{z}</m>
is to allow us to distinguish<fn>We could also define,
for example, a <m>1</m>-form as an ordered list
   <m>\big( F_1(x,y,z)\,,\,
          F_2(x,y,z)\,,\,
          F_3(x,y,z)\big)</m> of three functions and just view
<m> F_1(x,y,z)\,\dee{x}
+ F_2(x,y,z)\,\dee{y}
 + F_3(x,y,z)\,\dee{z}</m>
as another notation for
    <m>\big( F_1(x,y,z)\,,\,
          F_2(x,y,z)\,,\,
          F_3(x,y,z)\big)</m>.</fn>
<m>F_1(x,y,z)</m>, <m>F_2(x,y,z)</m> and <m>F_3(x,y,z)</m>.
</p>

<p>Similarly, we will define a 2-form as an expression of the form
<m>F_1(x,y,z)\,\dee{y}\wedge\dee{z}
 + F_2(x,y,z)\,\dee{z}\wedge\dee{x}
 + F_3(x,y,z)\,\dee{x}\wedge\dee{y}</m>.
Once again there is a symbol, namely <q><m>\wedge</m></q>, that we have not yet given a meaning to. We will, in Definition <xref ref="def_differentialFormMult"/>,
define a product, called the wedge product, with <m>\wedge</m> as
the multiplication symbol.
Then <m>\dee{x}\wedge\dee{y}</m> will be the wedge product of <m>\dee{x}</m> and
<m>\dee{y}</m>. Until then we will have to treat <m>\dee{y}\wedge\dee{z}</m>,
<m>\dee{z}\wedge\dee{x}</m> and <m>\dee{x}\wedge\dee{y}</m> just as three more
meaningless symbols.
</p>

<p>Finally here is the definition.
</p>

<definition xml:id="def_differentialForm">
<statement><p>
<ol label="a">
<li>
A <m>0</m>-form is a function <m>f(x,y,z)</m>.
</li>
<li>
A <m>1</m>-form is an expression of the form
<me>
  F_1(x,y,z)\,\dee{x}
 + F_2(x,y,z)\,\dee{y}
 + F_3(x,y,z)\,\dee{z}
</me>
with <m>F_1(x,y,z)</m>, <m>F_2(x,y,z)</m> and <m>F_3(x,y,z)</m> being functions
of three variables.
</li>
<li>
A <m>2</m>-form is an expression of the form
<me>
 F_1(x,y,z)\,\dee{y}\wedge\dee{z}
 + F_2(x,y,z)\,\dee{z}\wedge\dee{x}
 + F_3(x,y,z)\,\dee{x}\wedge\dee{y}
</me>
with <m>F_1(x,y,z)</m>, <m>F_2(x,y,z)</m> and <m>F_3(x,y,z)</m> being functions
of three variables.
</li>
<li>
A <m>3</m>-form is an expression of the form
 <m> f(x,y,z)\,\dee{x}\wedge\dee{y}\wedge\dee{z}</m>,
with <m>f(x,y,z)</m> being a function of three variables.
</li>
</ol>
At this stage (there'll more later), just think of <q><m>\dee{x}</m></q>,
<q><m>\dee{y}</m></q>, <q><m>\dee{z}</m></q>, <q><m>\dee{x}\wedge\dee{y}</m></q>, and so on,
as symbols.  Do not yet attempt to attach any significance to them.
</p></statement>
</definition>

<p>There are four operations involving differential forms <mdash/> addition,
multiplication (<m>\wedge</m>), differentiation (<m>\dee{}</m>) and integration.
Here are their
definitions. First, addition is defined, and works, just the way that
you would expect it to.
</p>

<definition xml:id="def_differentialFormAdd"><title>Addition of differential forms</title>
<statement><p>
<ol label="a">
<li>
The sum of the <m>0</m>-forms  <m>f</m> and <m>g</m> is the <m>0</m>-form <m>f+g</m>.
</li>
<li>
The sum of two <m>1</m>-forms is the <m>1</m>-form
<md>
<mrow>
  &amp;\big[F_1\,\dee{x}
          + F_2\,\dee{y}
          + F_3\,\dee{z}\big]
</mrow><mrow>
  +&amp;\big[G_1\,\dee{x}
          + G_2\,\dee{y}
          + G_3\,\dee{z}\big]
</mrow><mrow>
 =&amp; (F_1+G_1)\,\dee{x}
          + (F_2+G_2)\,\dee{y}
          + (F_3+G_3)\,\dee{z}
</mrow>
</md>
</li>
<li>
The sum of two <m>2</m>-forms is the <m>2</m>-form
<md>
<mrow>
  &amp;\big[F_1\,\dee{y}\wedge\dee{z}
          + F_2\,\dee{z}\wedge\dee{x}
          + F_3\,\dee{x}\wedge\dee{y}\big]
</mrow><mrow>
  +&amp;\big[G_1\,\dee{y}\wedge\dee{z}
          + G_2\,\dee{z}\wedge\dee{x}
          + G_3\,\dee{x}\wedge\dee{y}\big]
</mrow><mrow>
  =&amp;(F_1+G_1)\,\dee{y}\wedge\dee{z}
          + (F_2+G_2)\,\dee{z}\wedge\dee{x}
          + (F_3+G_3)\,\dee{x}\wedge\dee{y}
</mrow>
</md>
</li>
<li>
The sum of two <m>3</m>-forms is the <m>3</m>-form
<md>
<mrow>
   f\,\dee{x}\wedge\dee{y}\wedge\dee{z}
 \ +\  g\,\dee{x}\wedge\dee{y}\wedge\dee{z}
 \ =\  \big(f+g\big)\,\dee{x}\wedge\dee{y}\wedge\dee{z}
</mrow>
</md>
</li>
</ol>
</p></statement>
</definition>

<p>There is one wrinkle in multiplication. It is not commutative,
meaning that <m>\alpha\wedge\be</m> need not be the same as <m>\be\wedge\alpha</m>.
You have already seen some noncommutative products. If <m>\va</m> and <m>\vb</m>
are two vectors in <m>\bbbr^3</m>, then <m>\va\times\vb = -\vb\times \va</m>.
Also, if <m>A</m> and <m>B</m> are two <m>n\times n</m> matrices, the matrix product
<m>AB</m> need not be the same  as <m>BA</m>.
</p>

<definition xml:id="def_differentialFormMult"><title>Multiplication of differential forms</title>
<statement><p>

We now define a multiplication rule for differential forms.
If <m>\om</m> is a <m>k</m>-form and <m>\om'</m> is a
<m>k'</m>-form then the product will be a <m>(k+k')</m>-form and will be denoted
<m>\om\wedge\om'</m> (read <q>omega wedge omega prime</q>). It is
determined by the following properties.
<ol label="a">
<li>
If <m>f</m> is a function (i.e. a <m>0</m>-form), then
<md>
<mrow>
 f\big[F_1\,\dee{x} + F_2\,\dee{y} + F_3\,\dee{z}\big]
   &amp;= (fF_1)\,\dee{x} \!+\! (fF_2)\,\dee{y} \!+\! (fF_3)\,\dee{z}
</mrow><mrow>
 f\big[F_1\,\dee{y}\wedge\dee{z}
       \!+\! F_2\,\dee{z}\wedge\dee{x}
       \!+\! F_3\,\dee{x}\wedge\dee{y}\big]
  &amp;=(fF_1)\,\dee{y}\wedge\dee{z}
       + (fF_2)\,\dee{z}\wedge\dee{x}
</mrow><mrow>&amp;\hskip1.25in
       + (fF_3)\,\dee{x}\wedge\dee{y}
</mrow><mrow>
 f\big[g\,\dee{x}\wedge\dee{y}\wedge\dee{z}\big]
   &amp;= (fg)\,\dee{x}\wedge\dee{y}\wedge\dee{z}
</mrow>
</md>
Traditionally, the <m>\wedge</m> is not written when multiplying
a differential form by a function (i.e. a <m>0</m>-form).
</li>
<li>
<m>\om\wedge\om'</m> is linear in <m>\om</m> and in <m>\om'</m>. This means that
if <m>\om = f_1\om_1+f_2\om_2</m>, where <m>f_1</m>,<m>f_2</m> are
functions and <m>\om_1,\om_2</m> are forms, then
<me>
\big(f_1\om_1+f_2\om_2\big)\wedge \om'= f_1 (\om_1\wedge\om')
+f_2 (\om_1\wedge\om')
</me>
Similarly,
<me>
\om\wedge\big(f_1\om'_1+f_2\om'_2\big)= f_1 (\om\wedge\om'_1)
+f_2 (\om\wedge\om'_1)
</me>
</li>
<li>
<p>If <m>\om</m> is a <m>k</m>-form and <m>\om'</m> is a  <m>k'</m>-form then <me>
   \om\wedge\om'=(-1)^{kk'}\om'\wedge\om
</me>
That is, if at least one of <m>k</m> and <m>k'</m> is even, then
<me>
\om\wedge\om'=\om'\wedge\om
</me>
(so that the wedge product is commutative)
and if <m>k</m> and <m>k'</m> are <em>both odd</em> then
<me>
\om\wedge\om'=-\om'\wedge\om
</me>
(so that the wedge product is anticommutative).
In particular, if <m>\om</m> is a <m>d</m>-form with <m>d</m> <em>odd</em>
<me>
\om\wedge\om = 0
</me></p>
</li>
<li>
The wedge product is associative. This means that
<me>
(\om\wedge\om')\wedge\om''=\om\wedge\big(\om'\wedge\om''\big)
</me>
</li>
</ol>
</p></statement>
</definition>

<p>
So the wedge product obeys most of the usual multiplication rules, with
the one big exception that if <m>\om</m> is <m>k</m>-form and <m>\om'</m> is a
<m>k'</m>-form with <m>k</m> and <m>k'</m>  <em>both odd</em> then <m>\om\wedge\om'=-\om'\wedge\om</m>.
</p>

<p>The best way to get a handle on
the wedge product is to work through some examples, like these.
</p>

<example xml:id="eg_diffFormAddMultA">
<p>
Let
    <m>\om = F_1\,\dee{x}
     + F_2\,\dee{y}
     + F_3\,\dee{z}
    </m>
and
    <m>\om' = G_1\,\dee{x}
     + G_2\,\dee{y}
     + G_3\,\dee{z}
    </m>
be any two <m>1</m>-forms. Their product is
<md>
<mrow>
   \om\wedge\om'
&amp;=\big[F_1\,\dee{x}
     + F_2\,\dee{y}
     + F_3\,\dee{z}\big]
   \wedge
   \big[G_1\,\dee{x}
     + G_2\,\dee{y}
     + G_3\,\dee{z}\big]
</mrow><mrow>
   &amp;= \ \big(F_1\,\dee{x}\big)\wedge\big(G_1\,\dee{x}\big)
     +\big(F_1\,\dee{x}\big)\wedge\big(G_2\,\dee{y}\big)
     +\big(F_1\,\dee{x}\big)\wedge\big(G_3\,\dee{y}\big)
</mrow><mrow>
   &amp;\hskip0.1in +\big(F_2\,\dee{x}\big)\wedge\big(G_1\,\dee{x}\big)
     +\big(F_2\,\dee{x}\big)\wedge\big(G_2\,\dee{y}\big)
     +\big(F_2\,\dee{x}\big)\wedge\big(G_3\,\dee{y}\big)
</mrow><mrow>
   &amp;\hskip0.1in+ \big(F_3\,\dee{x}\big)\wedge\big(G_1\,\dee{x}\big)
     +\big(F_3\,\dee{x}\big)\wedge\big(G_2\,\dee{y}\big)
     +\big(F_3\,\dee{x}\big)\wedge\big(G_3\,\dee{y}\big)
</mrow><mrow>
 &amp;\hskip0.5in\text{(by linearity, i.e. by part (b) of the last Definition)}
</mrow><mrow>
   &amp;= \ F_1G_1\,\dee{x}\wedge\,\dee{x}
     + F_1G_2\,\dee{x}\wedge\,\dee{y}
     + F_1G_3\,\dee{x}\wedge\,\dee{z}
</mrow><mrow>
   &amp;\hskip0.1in +F_2G_1\,\dee{y}\wedge\,\dee{x}
     + F_2G_2\,\dee{y}\wedge\,\dee{y}
     + F_2G_3\,\dee{y}\wedge\,\dee{z}
</mrow><mrow>
   &amp;\hskip0.1in+ F_3G_1\,\dee{z}\wedge\,\dee{x}
     + F_3G_2\,\dee{z}\wedge\,\dee{y}
     + F_3G_3\,\dee{z}\wedge\,\dee{z}
</mrow><mrow>
   &amp;= \big(F_1G_2-F_2G_1)\,\dee{x}\wedge\dee{y}
                  +\big(F_3G_1-F_1G_3)\,\dee{z}\wedge\dee{x}
</mrow><mrow>
   &amp;\hskip0.1in
                  +\big(F_2G_3-F_3G_2)\,\dee{y}\wedge\dee{z}
</mrow>
</md>
because
<me>
\dee{x}\wedge\,\dee{x}=\dee{y}\wedge\,\dee{y}=\dee{z}\wedge\,\dee{z}=0
</me>
and
<me>
\dee{x}\wedge\,\dee{y}=-\dee{y}\wedge\,\dee{x}\qquad
\dee{x}\wedge\,\dee{z}=-\dee{z}\wedge\,\dee{x}\qquad
\dee{z}\wedge\,\dee{y}=-\dee{y}\wedge\,\dee{z}
</me>
</p>
</example>

<p>
Note that, looking at the last example,
if we view <m>\vF=(F_1,F_2,F_3)</m> and <m>\vG=(G_1,G_2,G_3)</m>
as vectors, we can write the product simply as
</p>

<fact xml:id="eqn_prodCross">
  <statement>
    <p>
<md>
<mrow>
&amp;\big[F_1\,\dee{x}
     + F_2\,\dee{y}
     + F_3\,\dee{z}\big]
   \wedge
   \big[G_1\,\dee{x}
     + G_2\,\dee{y}
     + G_3\,\dee{z}\big]
</mrow><mrow>
&amp;\hskip1in=(\vF\times\vG)_1\, \dee{y}\wedge\dee{z}
 +(\vF\times\vG)_2\, \dee{z}\wedge\dee{x}
 +(\vF\times\vG)_3\, \dee{x}\wedge\dee{y}
</mrow>
</md>
</p>
</statement>
</fact>

<p>
where we are using <m>(\vF\times\vG)_\ell</m> to denote the <m>\ell^{\rm th}</m>
component of the cross product <m>\vF\times\vG</m>.
In the special case that <m>F_3=G_3=0</m>, we have
</p>

<fact xml:id="eqnprodDet">
  <statement>
    <p><md>
<mrow>
\big[F_1\,\dee{x}
     + F_2\,\dee{y}\big]
   \wedge
   \big[G_1\,\dee{x}
     + G_2\,\dee{y}\big]
&amp;=\big(F_1G_2-F_2G_1)\,\dee{x}\wedge\dee{y}
</mrow><mrow>
&amp;=\det\left[\begin{matrix} F_1 &amp; F_2 \\
G_1 &amp; G_2\end{matrix}\right]
         \dee{x}\wedge\dee{y}
</mrow>
</md>
</p>
</statement>
</fact>

<p>We can now see why in the Definition <xref ref="def_differentialForm"/>.c
of <m>2</m>-forms
<ul>
<li>
there were no <m>\dee{x}\wedge\dee{x}</m> or
              <m>\dee{y}\wedge\dee{y}</m> or
              <m>\dee{z}\wedge\dee{z}</m>
terms <mdash/> they are all zero and
</li>
<li>
there were no <m>\dee{y}\wedge\dee{x}</m> or
              <m>\dee{z}\wedge\dee{y}</m> or
              <m>\dee{x}\wedge\dee{z}</m>
terms <mdash/> they can all be rewritten using
<m>\dee{x}\wedge\dee{y}</m>,
              <m>\dee{y}\wedge\dee{z}</m> and
              <m>\dee{z}\wedge\dee{x}</m>
terms (or vice versa).
</li>
</ul>
The reason that we chose to write the Definition <xref ref="def_differentialForm"/>.c
as<me>
 F_1\,\dee{y}\wedge\dee{z}
 + F_2\,\dee{z}\wedge\dee{x}
 + F_3\,\dee{x}\wedge\dee{y}
</me>
as opposed to in the form, for example,
<me>
 f_1\,\dee{x}\wedge\dee{y}
 + f_2\,\dee{x}\wedge\dee{z}
 + f_3\,\dee{y}\wedge\dee{z}
</me>
was to make formulae like <xref ref="eqn_prodCross"/> work.
The easy way to remember
<me>
 F_1\,\dee{y}\wedge\dee{z}
 + F_2\,\dee{z}\wedge\dee{x}
 + F_3\,\dee{x}\wedge\dee{y}
</me>
is to rename (in your head) <m>x,y,z</m> to <m>x_1,x_2,x_3</m>. Then the subscripts
in the three terms of
<me>
 F_1\,\dee{x_2}\wedge\dee{x_3}
 + F_2\,\dee{x_3}\wedge\dee{x_1}
 + F_3\,\dee{x_1}\wedge\dee{x_2}
</me>
are just <m>1,2,3</m> and <m>2,3,1</m> and <m>3,1,2</m> <mdash/> the three cyclic permutations
of <m>1,2,3</m>.
</p>

<example xml:id="eg_diffFormAddMultB">
<p>
The product of the (general) <m>1</m>-form
    <m>\om = F_1\,\dee{x}
     + F_2\,\dee{y}
     + F_3\,\dee{z}
    </m>
and the (general) <m>2</m>-form
    <m>\om'=\big[G_1\,\dee{y}\wedge\dee{z}
          + G_2\,\dee{z}\wedge\dee{x}
          + G_3\,\dee{x}\wedge\dee{y}\big]
    </m>
(again note the numbering of the coefficients in the <m>2</m>-form) is
<md>
<mrow>
  \om\wedge\om'
 &amp;=\big[F_1\,\dee{x}
     + F_2\,\dee{y}
     + F_3\,\dee{z}\big]
   \wedge
   \big[G_1\,\dee{y}\wedge\dee{z}
          + G_2\,\dee{z}\wedge\dee{x}
          + G_3\,\dee{x}\wedge\dee{y}\big]
</mrow><mrow>
  &amp;= \ F_1G_1\,\dee{x}\wedge\dee{y}\wedge\dee{z}
     + F_2G_2\,\dee{y}\wedge\dee{z}\wedge\dee{x}
     + F_3G_3\,\dee{z}\wedge\dee{x}\wedge\dee{y}
</mrow><mrow>
  &amp; = \big(F_1G_1+F_2G_2+F_3G_3)\,\dee{x}\wedge\dee{y}\wedge\dee{z}
</mrow>
</md>
Here we have used that, for <m>1</m>-forms, <m>\alpha\wedge\beta=-\beta\wedge\alpha</m>,
so that
<md>
<mrow>
\dee{y}\wedge\dee{z}\wedge\dee{x}
&amp;=-\dee{y}\wedge\dee{x}\wedge\dee{z}=\dee{x}\wedge\dee{y}\wedge\dee{z}

</mrow><mrow>
\dee{z}\wedge\dee{x}\wedge\dee{y}
&amp;=-\dee{x}\wedge\dee{z}\wedge\dee{y} =\dee{x}\wedge\dee{y}\wedge\dee{z}
</mrow>
</md>
We have also used that any wedge product of three
<m>\dee{\{x\text{ or }y\text{ or }z\}}</m>'s
with at least two of the coordinates being the same is zero. For example
<me>
\dee{x}\wedge\dee{z}\wedge\dee{x} = - \dee{x}\wedge\dee{x}\wedge\dee{z}
   =0
</me>
So
<md>
<mrow>
   &amp;\big[F_1\,\dee{x}
     + F_2\,\dee{y}
     + F_3\,\dee{z}\big]
   \wedge
   \big[G_1\,\dee{y}\wedge\dee{z}
          + G_2\,\dee{z}\wedge\dee{x}
          + G_3\,\dee{x}\wedge\dee{y}\big]
</mrow><mrow>
  &amp;\hskip4in = \vF\cdot\vG\,\dee{x}\wedge\dee{y}\wedge\dee{z}
</mrow>
</md>
</p>
</example>

<example xml:id="eg_diffFormAddMultC">
<p>
Combining Examples <xref ref="eg_diffFormAddMultA"/> and <xref ref="eg_diffFormAddMultB"/>,
we have the wedge product of any three (general)
<m>1</m>-forms
    <m>F_1\,\dee{x}
     + F_2\,\dee{y}
     + F_3\,\dee{z}</m>
and
    <m>G_1\,\dee{x}
     + G_2\,\dee{y}
     + G_3\,\dee{z}</m>
and
    <m>H_1\,\dee{x}
     + H_2\,\dee{y}
     + H_3\,\dee{z}</m>
is
<md>
<mrow>
&amp;\big[F_1\,\dee{x}
     \!+\! F_2\,\dee{y}
     \!+\! F_3\,\dee{z}\big]
   \wedge
   \big[G_1\,\dee{x}
     \!+\! G_2\,\dee{y}
     \!+\! G_3\,\dee{z}\big]
   \wedge
   \big[H_1\,\dee{x}
     + H_2\,\dee{y}
     + H_3\,\dee{z}\big]
</mrow><mrow>
&amp;\hskip0.1in=\big[F_1\,\dee{x}
     + F_2\,\dee{y}
     + F_3\,\dee{z}\big]
   \wedge
</mrow><mrow>&amp;\hskip1in
   \big[(\vG\times\vH)_1\, \dee{y}\wedge\dee{z}
 +(\vG\times\vH)_2\, \dee{z}\wedge\dee{x}
 +(\vG\times\vH)_3\, \dee{x}\wedge\dee{y}\big]
</mrow><mrow>
&amp;\hskip0.1in
  =\big\{F_1(\vG\times\vH)_1 + F_2(\vG\times\vH)_2 + F_3(\vG\times\vH)_3\big\}
     \dee{x}\wedge\dee{y}\wedge\dee{z}
</mrow><mrow>
&amp;\hskip0.1in
  =\big\{F_1(G_2H_3\!-\!G_3H_2) \!+\!
         F_2(G_3H_1\!-\!G_1H_3) \!+\!
         F_3(G_1H_2\!-\!G_2H_1\big\}
     \dee{x}\wedge\dee{y}\wedge\dee{z}

</mrow>
</md>
This can be expressed cleanly in terms of determinants.
Recalling the rule for expanding a determinant along its top row
<md>
<mrow>
&amp;\big[F_1\,\dee{x}
     \!+\! F_2\,\dee{y}
     \!+\! F_3\,\dee{z}\big]
   \wedge
   \big[G_1\,\dee{x}
     \!+\! G_2\,\dee{y}
     \!+\! G_3\,\dee{z}\big]
   \wedge
   \big[H_1\,\dee{x}
     \!+\! H_2\,\dee{y}
     \!+\! H_3\,\dee{z}\big]

</mrow><mrow>
&amp;\hskip3in
  =\det\left[\begin{matrix} F_1 &amp; F_2 &amp; F_3 \\
                            G_1 &amp; G_2 &amp; G_3 \\
                            H_1 &amp; H_2 &amp; H_3 \end{matrix}\right]
     \dee{x}\wedge\dee{y}\wedge\dee{z}
</mrow>
</md>
</p>
</example>


<p>Our next operation is a differential operator which unifies and generalizes
gradient, curl and divergence.
</p>

<definition xml:id="def_differentialFormDiff">
  <title>Differentiation of differential forms</title>
<statement><p>
If <m>\om</m> is a <m>k</m>-form, then <m>\dee{\om}</m> is a <m>k+1</m>-form, with
<m>\dee{}</m> being the unique<fn>That <m>\dee{}</m> is unique just means that
the action of <m>\dee{}</m> on <em>any</em> differential form is completely
determined by the four rules (a), (b), (c), (d). We will see in
Example <xref ref="eg_diffFormDiff"/>.b,c,d, that this is indeed the case.</fn>
such operator that obeys
<ol label="a">
<li>
<m>\dee{}</m> is linear. That is, if <m>\om_1,\om_2</m> are <m>k</m>-forms and
<m>a_1,a_2\in\bbbr</m>, then
<me>
\dee{\big(a_1\om_1+a_2\om_2\big)}
=a_1\dee{\om_1}+a_2\dee{\om_2}
</me>
</li>
<li>
<m>\dee{}</m> obeys a <q>graded product rule</q>. Precisely, if <m>\om^{(k)}</m> is a
<m>k</m>-form and <m>\om^{(\ell)}</m> is an <m>\ell</m>-form, then
<me>
\dee{\big(\om^{(k)}\wedge\om^{(\ell)}\big)}
=\big(d\om^{(k)}\big)\wedge\om^{(\ell)}
+(-1)^k\om^{(k)} \wedge \big(\dee{\om^{(\ell)}}\big)
</me>
</li>
<li>
If <m>f(x,y,z)</m> is a <m>0</m>-form, then
<md>
<mrow>
\dee{f}
&amp;=\frac{\partial f}{\partial x}(x,y,z)\ \dee{x}
+\frac{\partial f}{\partial y}(x,y,z)\ \dee{y}
+\frac{\partial f}{\partial z}(x,y,z)\ \dee{z}
</mrow><mrow>
&amp;=\vnabla f(x,y,z)\cdot\dee{\vr}
\qquad\text{where }
\dee{\vr} = \dee{x}\,\hi + \dee{y}\,\hj + \dee{z}\,\hk
</mrow>
</md>
</li>
<li>
For any differential form <m>\om</m>,
<me>
\dee{\big(\dee{\om}\big)}=0
</me>
</li>
</ol>
</p></statement>
</definition>


<example xml:id="eg_diffFormDiff">
<p>
<ol label="a">
<li>
If <m>f(x,y,z) = x</m>, then
<me>
\dee{f}
=\frac{\partial x}{\partial x}(x,y,z)\ \dee{x}
+\frac{\partial x}{\partial y}(x,y,z)\ \dee{y}
+\frac{\partial x}{\partial z}(x,y,z)\ \dee{z}
=\dee{x}
</me>
That is, <m>\dee{x}</m> really is the operator <m>\dee{}</m> applied to the
function <m>x</m>. Similarly, <m>\dee{y}</m> really is the operator <m>\dee{}</m>
applied to the function <m>y</m> and <m>\dee{z}</m> really is the operator
<m>\dee{}</m> applied to the function <m>z</m>.
</li>
<li>
For any <m>k</m>-form <m>\om</m>
<md>
<mrow>
\dee{\big[\om\wedge\dee{x}\big]}
&amp;=\dee{\om}\wedge\dee{x} + (-1)^k\om\wedge\dee{\big(\dee{x}\big)}
</mrow><mrow>
&amp;=\dee{\om}\wedge\dee{x}
</mrow>
</md>
Similarly
<me>
\dee{\big[\om\wedge\dee{y}\big]}=\dee{\om}\wedge\dee{y}\qquad
\dee{\big[\om\wedge\dee{z}\big]}=\dee{\om}\wedge\dee{z}
</me>
</li>
<li>
For any <m>1</m>-form
<md>
<mrow>
&amp;\dee{}\big[F_1\dee{x} + F_2\dee{y} + F_3\dee{z}\big]
=\dee{F_1}\wedge\dee{x} + \dee{F_2}\wedge\dee{y}  + \dee{F_3}\wedge\dee{z}

</mrow><mrow>
&amp;\hskip0.5in=\Big(\frac{\partial F_1}{\partial x}\ \dee{x}
      +\frac{\partial F_1}{\partial y}\ \dee{y}
      +\frac{\partial F_1}{\partial z}\ \dee{z}\Big)\wedge\dee{x}
</mrow><mrow>&amp;\hskip2in
+\Big(\frac{\partial F_2}{\partial x}\ \dee{x}
      +\frac{\partial F_2}{\partial y}\ \dee{y}
      +\frac{\partial F_2}{\partial z}\ \dee{z}\Big)\wedge\dee{y}
</mrow><mrow>&amp;\hskip2in
+\Big(\frac{\partial F_3}{\partial x}\ \dee{x}
      +\frac{\partial F_3}{\partial y}\ \dee{y}
      +\frac{\partial F_3}{\partial z}\ \dee{z}\Big)\wedge\dee{z}
</mrow><mrow>
&amp;\hskip0.5in=
  \Big(\frac{\partial F_3}{\partial y}-\frac{\partial F_2}{\partial z}\Big)
          \ \dee{y}\wedge\dee{z}
   +\Big(\frac{\partial F_1}{\partial z}-\frac{\partial F_3}{\partial x}\Big)
          \ \dee{z}\wedge\dee{x}
</mrow><mrow>&amp;\hskip2in
   +\Big(\frac{\partial F_2}{\partial x}-\frac{\partial F_1}{\partial y}\Big)
          \ \dee{x}\wedge\dee{y}
</mrow><mrow>
&amp;\hskip0.5in=
   (\vnabla\times\vF)_1\,\dee{y}\wedge\dee{z}
   +(\vnabla\times\vF)_2\,\dee{z}\wedge\dee{x}
   +(\vnabla\times\vF)_3\,\dee{x}\wedge\dee{y}
</mrow>
</md>
</li>
<li>
For any <m>2</m>-form
<md>
<mrow>
&amp;\dee{}\big[F_1\,\dee{y}\wedge\dee{z}
 + F_2\,\dee{z}\wedge\dee{x}
 + F_3\,\dee{x}\wedge\dee{y}\big]

</mrow><mrow>
&amp;\hskip0.5in=\dee{F_1}\wedge\dee{y}\wedge\dee{z}
+ \dee{F_2}\wedge\dee{z}\wedge\dee{x}
+ \dee{F_3}\wedge\dee{x}\wedge\dee{y}\big]

</mrow><mrow>
&amp;\hskip0.5in=\Big(\frac{\partial F_1}{\partial x}\ \dee{x}
      +\frac{\partial F_1}{\partial y}\ \dee{y}
      +\frac{\partial F_1}{\partial z}\ \dee{z}\Big)\wedge\dee{y}\wedge\dee{z}

</mrow><mrow>&amp;\hskip2in
+\Big(\frac{\partial F_2}{\partial x}\ \dee{x}
      +\frac{\partial F_2}{\partial y}\ \dee{y}
      +\frac{\partial F_2}{\partial z}\ \dee{z}\Big)\wedge\dee{z}\wedge\dee{x}

</mrow><mrow>&amp;\hskip2in
+\Big(\frac{\partial F_3}{\partial x}\ \dee{x}
      +\frac{\partial F_3}{\partial y}\ \dee{y}
      +\frac{\partial F_3}{\partial z}\ \dee{z}\Big)\wedge\dee{x}\wedge\dee{y}

</mrow><mrow>
&amp;\hskip0.5in=
  \Big(\frac{\partial F_1}{\partial x}
       +\frac{\partial F_2}{\partial y}
       +\frac{\partial F_3}{\partial z}\Big)
          \ \dee{x}\wedge\dee{y}\wedge\dee{z}

</mrow><mrow>
&amp;\hskip0.5in=
   \vnabla\cdot\vF\ \dee{x}\wedge\dee{y}\wedge\dee{z}
</mrow>
</md>
</li>
<li>
For any <m>3</m>-form
<md>
<mrow>
\dee{}\big[f\,\dee{x}\wedge\dee{y}\wedge\dee{z}\big]
&amp;=\Big(\frac{\partial f}{\partial x}\ \dee{x}
      +\frac{\partial f}{\partial y}\ \dee{y}
      +\frac{\partial f}{\partial z}\ \dee{z}\Big)
    \wedge\dee{x}\wedge\dee{y}\wedge\dee{z}
</mrow><mrow>
&amp;=0
</mrow>
</md>
</li>
</ol>
</p></example>


<example xml:id="eg_diffFormDiffB">
<p>
In Definition <xref ref="def_differentialFormDiff"/>.c, we defined,
for any function <m>f(x,y,z)</m> of three variables
<md>
<mrow>
\dee{f}
&amp;=\frac{\partial f}{\partial x}(x,y,z)\ \dee{x}
+\frac{\partial f}{\partial y}(x,y,z)\ \dee{y}
+\frac{\partial f}{\partial z}(x,y,z)\ \dee{z}
</mrow>
</md>
The analogous formulae<fn>Indeed, you can view <m>f(t)</m> as a function
of three variables that happens to be independent of two of the three
variables. Similarly you can view <m>f(u,v)</m>  as a function of three
variables that happens to be independent of one of the three variables.</fn>
 for functions of one or two variables also apply.
<md>
<mrow>
\dee{f(t)} &amp; = \diff{f}{t}(t)\,\dee{t}
</mrow><mrow>
\dee{f(uv)}
&amp;=\frac{\partial f}{\partial u}(u,v)\ \dee{u}
+\frac{\partial f}{\partial v}(u,v)\ \dee{v}
</mrow>
</md>
<ol label="a">
<li>
Let <m>F_1(x,y,z)\,\dee{x} + F_2(x,y,z)\,\dee{y} + F_3(x,y,z)\,\dee{z}</m>
be a <m>1</m>-form. Suppose that we substitute <m>x=x(t)</m>, <m>y=y(t)</m> and <m>z=z(t)</m>,
so that we are restricting our <m>1</m>-form to a parametrized curve.
Then, writing <m>\vr(t) = \big(x(t),y(t),z(t)\big)</m>,
<md>
<mrow>
&amp;F_1\big(x(t),y(t),z(t)\big)\,\dee{x(t)}
  + F_2\big(x(t),y(t),z(t)\big)\,\dee{y(t)}
</mrow><mrow>&amp;\hskip2in
  + F_3\big(x(t),y(t),z(t)\big)\,\dee{z(t)}
</mrow><mrow>
&amp;\hskip0.5in=F_1\big(\vr(t)\big)\diff{x}{t}(t)\,\dee{t}
  + F_2\big(\vr(t)\big)\diff{y}{t}(t)\,\dee{t}
  + F_3\big(\vr(t)\big)\diff{z}{t}(t)\,\dee{t}
</mrow><mrow>
&amp;\hskip0.5in= \vF\big(\vr(t)\big)\cdot\diff{\vr}{t}(t)\,\dee{t}
</mrow>
</md>
</li>
<li>
Let <m>F_1(x,y,z)\,\dee{y}\wedge\dee{z}
 + F_2(x,y,z)\,\dee{z}\wedge\dee{x}
 + F_3(x,y,z)\,\dee{x}\wedge\dee{y}</m>
be a <m>2</m>-form. Suppose that we substitute <m>x=x(u,v)</m>, <m>y=y(u,v)</m> and
<m>z=z(u,v)</m>, so that we are restricting our <m>2</m>-form to a parametrized surface.
Then, writing <m>\vr(u,v) = \big(x(u,v),y(u,v),z(u,v)\big)</m>,
<md>
<mrow>
&amp;F_1\big(x(u,v),y(u,v),z(u,v)\big)\,\dee{y(u,v)}\wedge\dee{z(u,v)}

</mrow><mrow>&amp;\hskip1in
  + F_2\big(x(u,v),y(u,v),z(u,v)\big)\,\dee{z(u,v)}\wedge\dee{x(u,v)}

</mrow><mrow>&amp;\hskip1in
  + F_3\big(x(u,v),y(u,v),z(u,v)\big)\,\dee{x(u,v)}\wedge\dee{y(u,v)}
</mrow><mrow>
&amp;=F_1\big(\vr(u,v)\big)\,
    \Big(\frac{\partial y}{\partial u}\dee{u}
        +\frac{\partial y}{\partial v}\dee{v}\Big)\wedge
    \Big(\frac{\partial z}{\partial u}\dee{u}
        +\frac{\partial z}{\partial v}\dee{v}\Big)

</mrow><mrow>&amp;\hskip1in
  + F_2\big(\vr(u,v)\big)\,
    \Big(\frac{\partial z}{\partial u}\dee{u}
        +\frac{\partial z}{\partial v}\dee{v}\Big)\wedge
    \Big(\frac{\partial x}{\partial u}\dee{u}
        +\frac{\partial x}{\partial v}\dee{v}\Big)

</mrow><mrow>&amp;\hskip1in
  + F_3\big(\vr(u,v)\big)\,
    \Big(\frac{\partial x}{\partial u}\dee{u}
        +\frac{\partial x}{\partial v}\dee{v}\Big)\wedge
    \Big(\frac{\partial y}{\partial u}\dee{u}
        +\frac{\partial y}{\partial v}\dee{v}\Big)
</mrow><mrow>
&amp;=\Big[F_1\big(\vr(u,v)\big)\,
    \Big(\frac{\partial y}{\partial u}\frac{\partial z}{\partial v}
        -\frac{\partial y}{\partial v}\frac{\partial z}{\partial u}\Big)
      +F_2\big(\vr(u,v)\big)\,
    \Big(\frac{\partial z}{\partial u}\frac{\partial x}{\partial v}
        -\frac{\partial z}{\partial v}\frac{\partial x}{\partial u}\Big)

</mrow><mrow>&amp;\hskip1in
      +F_3\big(\vr(u,v)\big)\,
    \Big(\frac{\partial x}{\partial u}\frac{\partial y}{\partial v}
        -\frac{\partial x}{\partial v}\frac{\partial y}{\partial u}\Big)
        \Big] \dee{u}\wedge\dee{v}
</mrow><mrow>
&amp;=\Big[\vF\big(\vr(u,v)\big)\cdot \frac{\partial\vr}{\partial u}(u,v)
                 \times \frac{\partial\vr}{\partial v}(u,v)\Big]
         \dee{u}\wedge\dee{v}
</mrow>
</md>
</li>
</ol>
</p></example>


<p>Let us summarize what we have seen in the Example <xref ref="eg_diffFormDiff"/>.</p>

<lemma xml:id="lemma_dGradCurlDiv">
<statement><p>
<ol label="a">
<li>
For any <m>0</m>-form
<me>
\dee{f}
=\vnabla f(x,y,z)\cdot\dee{\vr}
</me>
</li>
<li>
For any <m>1</m>-form
<md>
<mrow>
&amp;\dee{}\big[F_1\dee{x} + F_2\dee{y} + F_3\dee{z}\big]

</mrow><mrow>&amp;\hskip1in
=   (\vnabla\times\vF)_1\,\dee{y}\wedge\dee{z}
   +(\vnabla\times\vF)_2\,\dee{z}\wedge\dee{x}
   +(\vnabla\times\vF)_3\,\dee{x}\wedge\dee{y}
</mrow>
</md>
</li>
<li>
For any <m>2</m>-form
<me>
\dee{}\big[F_1\,\dee{y}\wedge\dee{z}
 + F_2\,\dee{z}\wedge\dee{x}
 + F_3\,\dee{x}\wedge\dee{y}\big]
=   \vnabla\cdot\vF\ \dee{x}\wedge\dee{y}\wedge\dee{z}
</me>
</li>
<li>
For any <m>3</m>-form
<me>
\dee{}\big[f\,\dee{x}\wedge\dee{y}\wedge\dee{z}\big]=0
</me>
</li>
</ol>
</p></statement>
</lemma>


<p>Our final operation is integration of differential forms. </p>

<definition xml:id="def_differentialFormInt">
  <title>Integration of differential forms</title>
<statement><p>
<ol label="a">
<li>
Let <m>f(x,y,z)</m> be a  <m>0</m>-form and <m>P=(x_0,y_0,z_0)\in\bbbr^3</m> be a point.
Then
<me>
\int_{P} f = f\big(x_0,y_0,z_0\big)
</me>
More generally if, for each <m>1\le i\le \ell</m>, <m>P_i=(x_i,y_i,z_i)\in\bbbr^3</m>
is a point and <m>n_i</m> is an integer, then
<me>
\int_{\Sigma_{i=1}^\ell n_iP_i} f = \sum_{i=1}^\ell n_i f\big(x_i,y_i,z_i\big)
</me>
</li>
<li>
Let  <m>\om = \vF(\vr)\cdot\dee{\vr}
 = F_1(x,y,z)\,\dee{x} + F_2(x,y,z)\,\dee{y} + F_3(x,y,z)\,\dee{z} </m>
be a  <m>1</m>-form. Let <m>\cC</m> be a curve that is parametrized
by <m>\vr(t) = \big(x(t)\,,\,y(t)\,,\,z(t)\big)</m>, <m>a\le t\le b</m>. Then,
motivated by Example <xref ref="eg_diffFormDiffB"/>.a above,
<me>
\int_{\cC}\om = \int_a^b \vF\big(\vr(t)\big)\cdot \diff{\vr}{t}(t)\ \dee{t}
              =\int_{\cC} \vF\cdot\dee{\vr}
</me>
</li>
<li>
Let  <m>\om = F_1(x,y,z)\,\dee{y}\wedge\dee{z}
 + F_2(x,y,z)\,\dee{z}\wedge\dee{x}
 + F_3(x,y,z)\,\dee{x}\wedge\dee{y}</m>
be a  <m>2</m>-form. Let <m>S</m> be an oriented surface that is parametrized
by <m>\vr(u,v) = \big(x(u,v)\,,\,y(u,v)\,,\,z(u,v)\big)</m>,
with <m>(u,v)</m> running over a region <m>R</m> in the <m>uv</m>-plane.
Assume that <m>\vr(u,v)</m> is orientation preserving in the sense that
<m>\hn\,\dee{S} = +\frac{\partial \vr}{\partial u}
\times \frac{\partial \vr}{\partial v}\,\dee{u}\,\dee{v}</m>.Then,
motivated by Example <xref ref="eg_diffFormDiffB"/>.b above,
<md>
<mrow>
\int_{S}\om &amp;= \dblInt_R \Big[\vF\big(\vr(u,v)\big)\cdot
           \frac{\partial\vr}{\partial u}(u,v)
                 \times \frac{\partial\vr}{\partial v}(u,v)\Big]
         \dee{u}\wedge\dee{v}
           = \dblInt_S \vF\cdot \hn\,\dee{S}
</mrow>
</md>
</li>
<li>
Let  <m>\om = f(x,y,z)\,\dee{x}\wedge\dee{y}\wedge\dee{z}</m>
be a  <m>3</m>-form. Let <m>V</m> be a solid in <m>\bbbr^3</m>. Then
<md>
<mrow>
\int_{V}\om &amp;= \tripInt_V f(x,y,z)\,\dee{x}\dee{y}\dee{z}
</mrow>
</md>
</li>
</ol>
</p></statement>
</definition>

<p>Finally, after all of these definitions, we have a very compact
theorem that simultaneously covers the fundamental theorem of calculus,
Green's theorem. Stokes' theorem and the divergence theorem. Had we given
all of our definitions in <m>n</m> dimensions, rather than just three dimensions,
it would cover a lot more. This general theorem is also called Stokes'
theorem.
</p>


<theorem xml:id="thm_GenStokes"><title>Stokes' Theorem</title>
<statement><p>
If <m>\om</m> is a <m>k</m>-form (with <m>k=0,1,2</m>) and <m>D</m> is a <m>(k+1)</m>-dimensional
domain of integration, then
<me>
\int_D d\om=\int_{\partial D}\om
</me>
Here <m>\partial D</m> is the boundary of <m>D</m> (suitably oriented).
</p></statement>
</theorem>


<p>To see the connection between the general Stokes' Theorem <xref ref="thm_GenStokes"/>
and the Stokes' and divergence theorems of the earlier part of this chapter,
here are the <m>k=1</m> and <m>k=2</m> cases of Theorem <xref ref="thm_GenStokes"/> again.
<ul>
<li>
  Let <m>\om = F_1 \dee{x} + F_2 \dee{y} + F_3 \dee{z}</m> be a <m>1</m>-form
and let <m>S</m> be a piecewise smooth oriented surface as in (our original)
Stokes' theorem <xref ref="thm_Stokes"/>. Then, by Lemma <xref ref="lemma_dGradCurlDiv"/>.b,
<me>
d\om = (\vnabla\times\vF)_1\,\dee{y}\wedge\dee{z}
   +(\vnabla\times\vF)_2\,\dee{z}\wedge\dee{x}
   +(\vnabla\times\vF)_3\,\dee{x}\wedge\dee{y}
</me>
So, by parts (c) (but with <m>\vF</m> replaced by <m>\vnabla\times\vF</m>) and (b)
of Definition <xref ref="def_differentialFormInt"/>,
the conclusion <m>\int_D d\om=\int_{\partial D}\om</m> of
(the general) Stokes' Theorem <xref ref="thm_GenStokes"/> is
<md>
<mrow>
\dblInt_S \vnabla\times\vF\cdot\hn\,\dee{S}
=\int_S d\om=\int_{\partial S}\om
=\int_{\partial S}\vF\cdot\dee{\vr}
</mrow>
</md>
which is the conclusion of (our original) Stokes' theorem <xref ref="thm_Stokes"/>.
</li>
<li>
  <m>\om = F_1(x,y,z)\,\dee{y}\wedge\dee{z}
 + F_2(x,y,z)\,\dee{z}\wedge\dee{x}
 + F_3(x,y,z)\,\dee{x}\wedge\dee{y}</m>
be a  <m>2</m>-form
and let <m>V</m> be a solid as in the divergence theorem <xref ref="thm_divThm"/>.
Then, by Lemma <xref ref="lemma_dGradCurlDiv"/>.c,
<me>
d\om = \vnabla\cdot\vF\,\dee{x}\wedge\dee{y}\wedge\dee{z}
</me>
So, by parts (d) (with <m>f =\vnabla\cdot\vF</m>) and (c)
of Definition <xref ref="def_differentialFormInt"/>,
the conclusion <m>\int_D d\om=\int_{\partial D}\om</m> of
(the general) Stokes' Theorem <xref ref="thm_GenStokes"/> is
<md>
<mrow>
\tripInt_V \vnabla\cdot\vF\,\dee{x}\dee{y}\dee{z}
=\int_V d\om=\int_{\partial V}\om
=\dblInt_{\partial V}\vF\cdot\hn\,\dee{S}
</mrow>
</md>
which is the conclusion of the divergence theorem <xref ref="thm_divThm"/>.
</li>
</ul>
</p>

<!-- <xi:include href="../problems/prob_s4.7.ptx" /> -->

</section>
