<?xml version="1.0" encoding="UTF-8" ?>
<section xmlns:xi="http://www.w3.org/2001/XInclude" xml:id="sec_GreenThm">

<!-- Copyright 2018-2020 Joel Feldman, Andrew Rechnitzer and Elyse Yeager -->
<!-- This work is licensed under the Creative Commons Attribution-NonCommercial-ShareAlike 4.0 International License-->
<!-- https://creativecommons.org/licenses/by-nc-sa/4.0 -->

<title>Green's Theorem</title>


<p>Our next variant of the fundamental theorem of calculus is
Green's<fn>George Green (1793<ndash/>1841) was a British
mathematical physicist. He spent much of the early part of his life
working in his father's bakery and grain mill. He was finally admitted
as an undergraduate to Cambridge in 1832, aged nearly forty.</fn>
 theorem, which
relates an integral, of a derivative of a (vector-valued) function,
over a region  in the <m>xy</m>-plane, with an integral of the function
over the curve bounding the region.
First we need to define some properties of curves.
</p>

<definition xml:id="def_Green">
<statement>
<p>
<ol label="a">
<li>
A curve <m>C</m> with parametrization <m>\vr(t)</m>, <m>a\le t\le b</m>, is said to be
<term>closed</term> if <m>\vr(a)=\vr(b)</m>.
</li>
<li>
A curve <m>C</m> is said to be <term>simple</term> if it does not cross itself.
More precisely, if <m>\vr(t)</m>, <m>a\le t\le b</m>, is a parametrization of the
curve and if <m>a\le t_1,t_2\le b</m> obey <m>t_1\ne t_2</m> and <m>\{t_1,t_2\}
\ne\{a,b\}</m>, then <m>\vr(t_1)\ne \vr(t_2)</m>. That is, if <m>\vr(t_1)=\vr(t_2)</m>,
then either <m>t_1=t_2</m> or <m>t_1=a</m>, <m>t_2=b</m>, or <m>t_1=b</m>, <m>t_2=a</m>.
</li>
<li><p>
A curve <m>C</m> is <term>piecewise smooth</term> if it has a parametrization
<m>\vr(t)</m> which
<ul>
<li>
is continuous and which
</li>
<li>
is differentiable except possibly at finitely many points with
</li>
<li>
the derivative being continuous and nonzero except possibly at finitely
many points.
</li>
</ul>
</p></li>
</ol>
</p></statement>
</definition>

<p>
Here are sketches of some examples.
</p>

<sidebyside widths="20% 26% 20% 23%" valign="middle">
<image source="figs/curve1"/>
    <image source="figs/curve2"/>
    <image source="figs/curve3"/>
    <image source="figs/astroid5"/>
</sidebyside>

<p>
And here is Green's theorem.
</p>

<theorem xml:id="thm_Green"><title>Green's Theorem</title>
<statement><p>
Let
<ul>
<li>
<m>R</m> be a finite region in the <m>xy</m>-plane,
</li>
<li><p>
the boundary, <m>C</m>, of <m>R</m> consist of a finite number of piecewise smooth, simple closed curves
<ul>
<li>
     that are oriented (i.e. arrows are put on <m>C</m>) consistently
     with <m>R</m> in the sense that if you walk along
     <m>C</m> in the direction of the arrows, then <m>R</m> is on your left
</li>
</ul>
</p>

<sidebyside widths="25%  27%" valign="middle">
<image source="figs/greens1"/>
<image source="figs/dcircleE"/>
</sidebyside>
</li>
<li>
<m>F_1(x,y)</m> and <m>F_2(x,y)</m> have continuous first partial derivatives
at <em>every</em> point of <m>R</m>.
</li>
</ul>
Then
<me>
\oint_{C} \big[F_1(x,y)\,\dee{x} +F_2(x,y)\,\dee{y}\big]
 =\dblInt_{R}\left(\frac{\partial F_2}{\partial x}
                - \frac{\partial F_1}{\partial y}\right)\ \dee{x}\dee{y}
</me>
</p></statement>
</theorem>


<warning xml:id="warn_Green">
<p>
Note that in Theorem <xref ref="thm_Green"/> we are assuming that
<m>F_1</m> and <m>F_2</m> have continuous first partial derivatives
at <em>every</em> point of <m>R</m>.
If that is not the case, for example
because <m>F_1</m> or <m>F_2</m> is not defined on all of <m>R</m>, then
the conclusion of Green's theorem can fail. An example is
<m>F_1=-\frac{y}{x^2+y^2}</m>, <m>F_2=\frac{x}{x^2+y^2}</m>, <m>R=\Set{(x,y)}{x^2+y^2\le 1}</m>.
See Examples<nbsp/><xref ref="eg_greenC"/> and <xref ref="eg_greenCC"/>.
</p>
</warning>

<p>
Here are three notational remarks before we start the proof.
<ul>
<li>
One way to remember the integrand on the right hand side is to write it
as <m>(\vnabla\times\vF)\cdot\hk</m>.
</li>
<li>
Many people use <m>M</m> instead of <m>F_1</m> and <m>N</m> instead of <m>F_2</m>.
Then Green's theorem becomes
<m>\oint_{C} \big[M(x,y)\,\dee{x} +N(x,y)\,\dee{y}\big]
 =\dblInt_{R}\Big(\frac{\partial N}{\partial x}
                - \frac{\partial M}{\partial y}\Big)\ \dee{x}\dee{y}</m>
</li>
<li>  The symbol <m>\oint_C</m> is just an alternate notation for <m>\int_C</m>
that is sometimes used when <m>C</m> is a closed curve.
See Notation <xref ref="not_workIntegral"/>.
</li>
</ul>
</p>

<proof>
<p>
We prove the result by reformulating it as a divergence theorem statement.
To that end, we define
<md>
<mrow>
V&amp;=\Set{(x,y,z)}{ (x,y)\in R,\ \ 0\le z\le 1}
</mrow><mrow>
\vG(x,y,z) &amp;= F_2(x,y)\,\hi -F_1(x,y)\,\hj
</mrow>
</md>
Notice that <m>V</m> is exactly the volume obtained by expanding <m>R</m> vertically
upward by one unit.
</p>

<sidebyside width="45%">
<image source="figs/greens2"/>
</sidebyside>

<p>
The definition of <m>\vG</m> does <em>not</em> contain a typo <mdash/> the <m>x</m>-component
of <m>\vG</m> really is <m>F_2</m> and the <m>y</m>-component of <m>\vG</m> really is <m>-F_1</m>.
(More or less the reverse of what you would normally write down.)
</p>

<p>These definitions have been rigged so that the divergence theorem
applied to <m>\vG</m> and <m>V</m>, namely
<md>
<mrow>
\dblInt_{\partial V} \vG\cdot\hn\,\dee{S}
&amp;=\tripInt_V\vnabla\cdot\vG\ \dee{V}
</mrow>
</md>
gives us exactly Green's theorem, as we shall now see.
</p>

<p>Since <m>\vnabla\cdot\vG = \frac{\partial F_2}{\partial x}
                - \frac{\partial F_1}{\partial y}</m>,  the right hand side is just
<md>
<mrow>
\tripInt_V\vnabla\cdot\vG\ \dee{V}
&amp;= \dblInt_{R}\dee{x}\dee{y}\int_0^1\dee{z} \ \vnabla\cdot\vG
</mrow><mrow>
&amp;= \dblInt_{R}\dee{x}\dee{y}\int_0^1\dee{z} \
        \left(\frac{\partial F_2}{\partial x}(x,y)
                - \frac{\partial F_1}{\partial y}(x,y)\right)
</mrow><mrow>
&amp;= \dblInt_{R}\dee{x}\dee{y}\
        \left(\frac{\partial F_2}{\partial x}(x,y)
                - \frac{\partial F_1}{\partial y}(x,y)\right)
</mrow>
</md>
because the integrand is independent of <m>z</m>. This is exactly the right
hand side of Green's theorem.
</p>

<p>Now for the left hand side. The boundary, <m>\partial V</m>, of <m>V</m> is the union
of the (flat) bottom, the (flat) top and the (curved) side.
The outward unit normal on the (horizontal, flat) top is <m>+\hk</m> and
the outward unit normal on the (horizontal, flat) bottom is <m>-\hk</m>  so that
<md>
<mrow>
\dblInt_{\partial V} \vG\cdot\hn\,\dee{S}
&amp;=\dblInt_{\text{top}} \vG\cdot\hk\,\dee{S}
   +\dblInt_{\text{bottom}} \vG\cdot(-\hk)\,\dee{S}
   +\dblInt_{\text{side}} \vG\cdot\hn\,\dee{S}
</mrow><mrow>
&amp;=\dblInt_{\text{side}} \vG\cdot\hn\,\dee{S}
</mrow>
</md>
We have used the fact that the <m>\hk</m> component of <m>\vG</m> is exactly zero
to discard the integrals over the top and bottom of <m>\partial V</m>.
To evaluate the integral over the side, we'll parametrize the side. Suppose that
<m>\vr(t)=x(t)\,\hi +y(t)\,\hj</m>, <m>a\le t\le b</m>,
is a parametrization of <m>C</m>, with the arrow in the figure above giving the
direction of increasing <m>t</m>. Then we can use
<md>
<mrow>
\vR(t,z)  = \vr(t) +z\,\hk
          = x(t)\,\hi +y(t)\,\hj +z\,\hk \qquad a\le t\le b,\ 0\le z\le 1
</mrow>
</md>
as a parametrization of the side. We'll use (<xref ref="eq_SUdSparam"/>) to determine
<m>\hn\,\dee{S}</m> for the side. Since
<md>
<mrow>
\frac{\partial\vR}{\partial t}(t,z) &amp; = x'(t)\,\hi +y'(t)\,\hj
</mrow><mrow>
\frac{\partial\vR}{\partial z}(t,z) &amp; = \hk
</mrow>
</md>
(<xref ref="eq_SUdSparam"/>) gives
<md>
<mrow>
\hn\,\dee{S} &amp;= \frac{\partial\vR}{\partial t}(t,z)\times
               \frac{\partial\vR}{\partial z}(t,z)\ \dee{t}\dee{z}
</mrow><mrow>
&amp;= \big(x'(t)\,\hi +y'(t)\,\hj\big)\times \hk\ \dee{t}\dee{z}
</mrow><mrow>
&amp;= \big(-x'(t)\,\hj +y'(t)\,\hi\big)\ \dee{t}\dee{z}
</mrow>
</md>
Note that with this choice of <m>\pm</m> sign (that is,
<m>\frac{\partial\vR}{\partial t}\times
               \frac{\partial\vR}{\partial z}\ \dee{t}\dee{z}</m>
rather than
<m>-\frac{\partial\vR}{\partial t}\times
               \frac{\partial\vR}{\partial z}\ \dee{t}\dee{z}</m>), the vector
<m>\hn</m> really is the <em>outward</em> pointing normal, as we see from the sketch
</p>

<sidebyside width="45%">
<image source="figs/greens3"/>
</sidebyside>

<p>
We can now compute the surface integral directly.
<md>
<mrow>
&amp;\dblInt_{\partial V} \vG\cdot\hn\,\dee{S}
=\dblInt_{\text{side}} \vG\cdot\hn\,\dee{S}
</mrow><mrow>
&amp;\hskip0.25in=\int_a^b\dee{t}\int_0^1\dee{z}\ \vG\big(\vR(t,z)\big)\cdot
          \big(-x'(t)\,\hj +y'(t)\,\hi\big)

</mrow><mrow>
&amp;\hskip0.25in=\int_a^b\dee{t}\int_0^1\dee{z}\
         \big(F_2(x(t),y(t))\,\hi -F_1(x(t),y(t))\,\hj\big)\cdot
          \big(-x'(t)\,\hj +y'(t)\,\hi\big)
</mrow><mrow>
&amp;\hskip0.25in=\int_a^b\dee{t}\
         \big[F_2(x(t),y(t))\,y'(t) +F_1(x(t),y(t))\,x'(t)\big]

</mrow><mrow>
&amp;\hskip2in \text{since the integrand is independent of } z

</mrow><mrow>
&amp;\hskip0.25in=\oint_{C} \big[F_1(x,y)\,\dee{x} +F_2(x,y)\,\dee{y}\big]
</mrow>
</md>
This is exactly the left
hand side of Green's theorem.
</p></proof>

<example xml:id="eg_greenA">
<statement>
<p>
Evaluate
<me>
\oint_C\big[(x-xy)\,\dee{x} + (y^3+1)\,\dee{y}
</me>
where <m>C</m> is the curve given in the figure
</p>
<sidebyside width="39%">
<image source="figs/greensSquare"/>
</sidebyside>

</statement>

<solution>
<p>
Let <m>R=\Set{(x,y)}{1\le x\le 2,\ 0\le y\le 1}</m>. By Green's theorem
<md>
<mrow>
\oint_C\big[(x-xy)\,\dee{x} + (y^3+1)\,\dee{y}
&amp;=\dblInt_R\Big[\frac{\partial }{\partial x}(y^3+1)
                - \frac{\partial }{\partial y}(x-xy)\Big]\dee{x}\dee{y}
</mrow><mrow>
&amp;=\int_1^2\dee{x}\int_0^1\dee{y}\ x
=\frac{x^2}{2}\bigg|_1^2
=\frac{3}{2}
</mrow>
</md>
</p>
</solution>
</example>


<p>Here is a simple corollary of Green's theorem that tells how to compute the area enclosed by a curve in the <m>xy</m>-plane.
</p>

<corollary xml:id="cor_greens">
<statement><p>
Let
<ul>
<li>
<m>R</m> be a finite region in the <m>xy</m>-plane whose boundary
</li>
<li>
<m>C</m> consists of a finite number of piecewise smooth, simple closed curves.
</li>
<li>
Orient <m>C</m> (i.e. put arrows on <m>C</m>) so that if you walk along
<m>C</m> in the direction of the arrows, then <m>R</m> is on your left.
</li>
</ul>
Then
<me>
\text{Area}(R)
 =\oint_C x\dee{y}
 =-\oint_C y\dee{x}
 =\frac{1}{2}\oint_C \big[x\dee{y} -y\dee{x}\big]
</me>
</p></statement>
</corollary>

<proof>
<p>
This is just Green's theorem applied first with
<m>\vF = x\,\hj</m>, then with <m>\vF= -y\,\hi</m> and finally with
<m>\vF = \frac{1}{2}\big[-y\,\hi +x\,\hj\big]</m>. For all three of these
<m>\vF</m>'s,
<me>
\frac{\partial F_2}{\partial x}
                - \frac{\partial F_1}{\partial y} = 1
</me>
so that Green's theorem gives
<md>
<mrow>
\oint_{C} \big[F_1(x,y)\,\dee{x} +F_2(x,y)\,\dee{y}\big]
 &amp;=\dblInt_{R}\Big(\frac{\partial F_2}{\partial x}
                - \frac{\partial F_1}{\partial y}\Big)\ \dee{x}\dee{y}
 =\dblInt_{R}\ \dee{x}\dee{y}
</mrow><mrow>
&amp; = \text{Area}(R)
</mrow>
</md>
</p>

</proof>

<example xml:id="eg_greenB">
<p>
In this example we will use Green's theorem to compute the area enclosed
by the astroid <m>x^{2/3} + y^{2/3} = a^{2/3}</m>.
</p>

<sidebyside width="29%">
<image source="figs/astroid6"/>
</sidebyside>

<p>
In Example <xref ref="eg_astroid"/> we found the parametrization
<me>
\vr(t) = x(t)\,\hi + y(t)\,\hj = a\cos^3t\,\hi + a\sin^3 t\,\hj
\qquad 0\le t\le 2\pi
</me>
for the astroid. So, by Corollary <xref ref="cor_greens"/>,
<md>
<mrow>
\text{Area}
&amp;=\frac{1}{2}\oint_C \big[x\dee{y} -y\dee{x}\big]
 =\frac{1}{2}\int_0^{2\pi} \big[x(t)y'(t) -y(t)x'(t)\big]\dee{t}
</mrow><mrow>
&amp;=\frac{3a^2}{2}\int_0^{2\pi} \big[\cos^3t\sin^2t\cos t
                                 +\sin^3t\cos^2 t\sin t\big]\dee{t}
</mrow><mrow>
&amp;=\frac{3a^2}{2}\int_0^{2\pi} \cos^2t\sin^2t\big[\cos^2t
                                 +\sin^2t\big]\dee{t}
</mrow><mrow>
&amp;=\frac{3a^2}{2}\int_0^{2\pi} \cos^2t\sin^2t\ \dee{t}
</mrow><mrow>
&amp;=\frac{3a^2}{8}\int_0^{2\pi} \sin^2(2t)\ \dee{t}
=\frac{3a^2}{16}\int_0^{2\pi} [1-\cos(4t)]\ \dee{t}
</mrow><mrow>
&amp;=\frac{3}{8}a^2\pi
</mrow>
</md>
</p></example>


<example xml:id="eg_greenC"><title>Trick Question</title>
<statement>
<p>
Evaluate
<me>
\oint_C\vB\cdot\dee{\vr}
</me>
where
<me>
\vB = \frac{-y\,\hi+x\,\hj}{x^2+y^2}
</me>
and <m>C</m> is the curve
<md>
<mrow>
x(t) &amp;= \sin(\cos t)
</mrow><mrow>
y(t) &amp;= \sin(\sin t)
</mrow><mrow>
z(t) &amp;= 0
</mrow>
</md>
with <m>0\le t\le 2\pi</m>.
</p>
</statement>

<solution>
<p>
First let's think about the curve <m>C</m>. If the curve were just
<m>X(t)=\cos t</m>, <m>Y(t)=\sin t</m>, <m>Z(t)=0</m>, it would be the unit circle
centred on the origin in the <m>xy</m>-plane, traversed counterclockwise.
For <m>-\frac{\pi}{2}\le u\le \frac{\pi}{2}</m>, the function <m>\sin u</m>
increases monotonically with  <m>u</m> and is of the same sign as <m>u</m> so that,
since <m>|\sin t|,|\cos t|\le 1 \lt \frac{\pi}{2}</m>,
<ul>
<li>
<m>x(t) = \sin\big(\cos t)</m> has the same sign as <m>X(t)=\cos t</m> and is increasing
at precisely the same <m>t</m>'s as is <m>X(t)</m>
</li>
<li>
<m>y(t) = \sin\big(\sin t)</m> has the same sign as <m>Y(t)=\sin t</m> and is increasing
at precisely the same <m>t</m>'s as is <m>Y(t)</m>
</li>
</ul>
So the extra sine in our
parametrization of <m>C</m> just distorts the circle, straightening the sides a little
as depicted here.
</p>

<sidebyside width="28%">
<image source="figs/dcircleA"/>
</sidebyside>

<p>
It looks like our problem is a straightforward Green's theorem problem
like Example<nbsp/><xref ref="eg_greenA"/>. Let's just try using the strategy of
Example <xref ref="eg_greenA"/>. Because
<md>
<mrow>
\frac{\partial \vB_2}{\partial x} - \frac{\partial \vB_1}{\partial y}
&amp;=\frac{\partial }{\partial x}\frac{x}{x^2+y^2}
                - \frac{\partial }{\partial y}\frac{-y}{x^2+y^2}
</mrow><mrow>
&amp;= \frac{1}{x^2+y^2} - \frac{2x^2}{{(x^2+y^2)}^2}
  +\frac{1}{x^2+y^2} - \frac{2y^2}{{(x^2+y^2)}^2}
</mrow><mrow>
&amp;= \frac{(x^2+y^2) - 2x^2 + (x^2+y^2) - 2y^2}{{(x^2+y^2)}^2}
</mrow><mrow>
&amp;=0
</mrow>
</md>
it looks like Green's theorem gives us, trivially,
<me>
\oint_C\vB\cdot\dee{\vr}
=\oint_C\big[\vB_1\,\dee{x} +\vB_2\,\dee{y}\big]
= \dblInt_{R}\left(\frac{\partial B_2}{\partial x}
                - \frac{\partial B_1}{\partial y}\right)\ \dee{x}\dee{y}
=0
</me>
where <m>R</m> is the region inside our curve <m>C</m>.
</p>

<p>That was easy <mdash/> but it's also very <alert>wrong</alert>!
Our next steps are to
<ul>
<li>
verify that <m>\oint_C\vB\cdot\dee{\vr}\ne 0</m>, and
</li>
<li>
explain why we got the wrong answer, and
</li>
<li>
modify our computation so as to give the correct answer.
We'll do this in Example <xref ref="eg_greenCC"/>.
</li>
</ul>
</p>

<p>
<em>Verification that <m>\oint_C\vB\cdot\dee{\vr}\ne 0</m>:}</em>
</p>

<p>
Since
<md>
<mrow>
x'(t) &amp;= -\cos(\cos t)\ \sin t
</mrow><mrow>
y'(t) &amp;= \cos(\sin t)\ \cos t
</mrow><mrow>
z'(t) &amp;= 0
</mrow>
</md>
our integral is
<md>
<mrow>
\oint_C\vB\cdot\dee{\vr}
&amp;=\oint_C\big[\vB_1\,\dee{x} +\vB_2\,\dee{y}\big]
</mrow><mrow>
&amp;=\int_0^{2\pi}\big[\vB_1\big(x(t),y(t)\big)\,x'(t)
            +\vB_2\,\big(x(t),y(t)\big)\,y'(t)\big]\dee{t}

</mrow><mrow>
&amp;=\int_0^{2\pi}
            \frac{\sin(\sin t)\,\cos(\cos t)\,\sin t
                  +\sin(\cos t)\,\cos(\sin t)\,\cos t}
                  {\sin^2(\cos t) +\sin^2(\sin t)}
            \dee{t}
</mrow>
</md>
This is a very ugly looking integral<fn>Indeed!</fn>.
But even if we can't evaluate the
integral, we can see that the integrand is strictly positive,
and that forces <m>\oint_C\vB\cdot\vr \gt 0</m>. Because
<me>
0\le|\sin t|,|\cos t|\le 1 \lt \frac{\pi}{2}
</me>
<ul>
<li>
<m>\cos(\cos t) \gt 0</m>, and <m>\sin(\sin t)</m> has the same sign as <m>\sin t</m>,
and <m>\sin(\sin t)</m> is zero if and only if <m>\sin t=0</m>.
So the first term in the numerator,
<me>
\cos(\cos t)\,\sin(\sin t)\,\sin t\ge 0
</me>
and is zero if and only if <m>\sin t=0</m>
</li>
<li>
<m>\cos(\sin t) \gt 0</m>, and <m>\sin(\cos t)</m> has the same sign as <m>\cos t</m>, and
<m>\sin(\cos t)</m> is zero if and only if <m>\cos t=0</m>. So the second term
in the numerator,
<me>
\cos(\sin t)\,\sin(\cos t)\,\cos t\ge 0
</me>
and is zero
if and only if <m>\cos t=0</m>.
</li>
<li>
There is no <m>t</m> for which both <m>\sin t</m> and <m>\cos t</m> are simultaneously
zero. So the whole numerator
<me>
\sin(\sin t)\,\cos(\cos t)\,\sin t
                  +\sin(\cos t)\,\cos(\sin t)\,\cos t \gt 0
</me>
is strictly positive.
</li>
</ul>
Since the integrand is strictly positive, the integral is strictly positive.
</p>

<p><em>Why we got the wrong answer:</em>
</p>

<p>
In our initial and wrong calculation above, we assumed that
<m>\frac{\partial B_2}{\partial x}(x,y)
                - \frac{\partial B_1}{\partial y}(x,y)=0</m>
at all points <m>(x,y)</m> of the region <m>R</m> inside <m>C</m>. That's not true.
While it is true for most points, it is not true for  <em>all</em> points.
The vector field <m>\vB(x,y)</m> is not defined at <m>(x,y)=(0,0)</m>.
So <m>\frac{\partial B_2}{\partial x}(x,y)
                - \frac{\partial B_1}{\partial y}(x,y)</m>
is also not defined at <m>(x,y)=(0,0)</m>. That's enough to invalidate
Green's theorem. Read the statement of Theorem <xref ref="thm_Green"/> again carefully.
</p>
</solution>
</example>

<example xml:id="eg_greenCC"><title>Example <xref ref="eg_greenC"/>, again.</title>
<statement>
<p>
Evaluate
<me>
\oint_C\vB\cdot\dee{\vr}
</me>
where
<me>
\vB = \frac{-y\,\hi+x\,\hj}{x^2+y^2}
</me>
and <m>C</m> is the curve
<md>
<mrow>
x(t) &amp;= \sin(\cos t)
</mrow><mrow>
y(t) &amp;= \sin(\sin t)
</mrow><mrow>
z(t) &amp;= 0
</mrow>
</md>
with <m>0\le t\le 2\pi</m>.
</p>
</statement>

<solution>
<p>
This is the same integral that we computed incorrectly in Example
 <xref ref="eg_greenC"/>.
We'll use two ingredients to compute <m>\oint_C\vB\cdot\dee{\vr}</m>
correctly.
</p>

<p><ul>
<li>
Let <m>a \gt 0</m> and denote by <m>C_a</m> the clockwise oriented circle in
the <m>xy</m>-plane that is of radius <m>a</m> and is centered on the origin.
We can explicitly compute
<m>\oint_{C_a}\vB\cdot\dee{\vr}</m>. To do so just parametrize
<m>C_a</m> by <m>x(t)=a\cos t</m>, <m>y(t) = a\sin t</m>, <m>z(t)=0</m>. Then
<m>x'(t)=-a\sin t</m>, <m>y(t) = a\cos t</m> and
<md>
<mrow>
\oint_{C_a}\vB\cdot\dee{\vr}
&amp;=\int_0^{2\pi}\Big[\frac{-a\sin t\,\hi+a\cos t\,\hj}
                            {a^2\cos^2t+a^2\sin^2t}\Big]
           \cdot\big[-a\sin t\,\hi+a\cos t\,\hj\big]
           \dee{t}
</mrow><mrow>
&amp;=\int_0^{2\pi}\dee{t}=2\pi
</mrow>
</md>
</li>
<li><p>
Pick an <m>a</m> that is small enough that <m>C_a</m> lies entirely inside <m>C</m> and
apply Green's theorem with the region, <m>R_a</m>, that is between <m>C</m> and <m>C_a</m>.
</p>

<sidebyside width="45%">
<image source="figs/dcircleB"/>
</sidebyside>

<p>
The curve bounding <m>R_a</m> has two components <mdash/> <m>C</m> and <m>C_a</m>, but now <m>C_a</m>
is oriented clockwise. (Recall that, in Green's theorem, when you walk along a boundary curve in the direction of the arrow, <m>R_a</m> has to be on your left.). Use
<m>-C_a</m> to denote <m>C_a</m> oriented clockwise.
<m>\frac{\partial B_2}{\partial x}(x,y)
                - \frac{\partial B_1}{\partial y}(x,y)</m> really is zero
at <em>all</em> points <m>(x,y)</m> of the region <m>R_a</m>. So Green's theorem gives
<md>
<mrow>
0&amp;= \dblInt_{R_a}\Big(\frac{\partial B_2}{\partial x}
                - \frac{\partial B_1}{\partial y}\Big)\ \dee{x}\dee{y}
  = \oint_{C}\vB\cdot\dee{\vr} + \oint_{-C_a}\vB\cdot\dee{\vr}
</mrow><mrow>
 &amp; = \oint_{C}\vB\cdot\dee{\vr} - \oint_{C_a}\vB\cdot\dee{\vr}
</mrow>
</md>
and so
<md>
<mrow>
\oint_{C}\vB\cdot\dee{\vr}
= \oint_{C_a}\vB\cdot\dee{\vr}
=2\pi
</mrow>
</md>
</p></li>
</ul>
</p>


</solution>
</example>

<xi:include href="../problems/prob_s4.3.ptx" />

</section>
