<?xml version="1.0" encoding="UTF-8" ?>
<section xmlns:xi="http://www.w3.org/2001/XInclude" xml:id="sec_tangentPlanes">

<!-- Copyright 2018-2020 Joel Feldman, Andrew Rechnitzer and Elyse Yeager -->
<!-- This work is licensed under the Creative Commons Attribution-NonCommercial-ShareAlike 4.0 International License-->
<!-- https://creativecommons.org/licenses/by-nc-sa/4.0 -->

<title>Tangent Planes</title>
<p>
If you are confronted with a complicated surface and want to get some
idea of what it looks like near a specific point, probably the first
thing that you will do is find the plane that best approximates the
surface near the point. That is, find the tangent plane to the surface at
the point.
In general, a good way to specify a plane is to supply
<ul>
<li>
a nonzero vector <m>\vn</m> (called a normal vector) perpendicular to the
plane<fn>Alternatively, you could find two vectors that are in the
plane (and not parallel to each other), and then construct a normal vector
by taking their cross product.
</fn> (to determine the orientation of the plane)
and
</li>
<li>
one point <m>(x_0,y_0,z_0)</m> on the plane.
</li>
</ul>
If <m>(x,y,z)</m> is any other point on the plane, then the vector
<me>
(x,y,z)-(x_0,y_0,z_0) = (x-x_0\,,\,y-y_0\,,\,z-z_0)
</me>
lies entirely in the plane and so is perpendicular to <m>\vn</m>. This gives
the following very neat the equation for the plane.
</p>

<sidebyside widths="45% 30%" valign="middle">
<p><me>
\vn\cdot(x-x_0\,,\,y-y_0\,,\,z-z_0) = 0
</me></p>
<image source="figs/plane"/>
</sidebyside>

<p>
The following theorem provides formulae for normal vectors <m>\vn</m> to
general surfaces, assuming first that the surface is parametrized,
second that the surface is a graph and finally the surface is given
by an implicit equation. The formulae are developed in the proof of the
theorem.
</p>

<theorem xml:id="thm_normalVectors"><title>Normal vectors to surfaces</title>
<statement><p>
<ol label="a">
<li>
Let
<md>
<mrow>
\vr&amp;: \cD\subset\bbbr^2 \rightarrow \bbbr^3
</mrow><mrow>
   &amp;(u,v) \in\cD \mapsto \vr(u,v) =\big(x(u,v)\,,\,y(u,v)\,,\,z(u,v)\big)
</mrow>
</md>
be a parametrized surface and let <m>(x_0,y_0,z_0)=\vr(u_0,v_0)</m>
be a point on the surface. Set
<md>
<mrow>
\vT_u &amp;= \frac{\partial\ }{\partial u}\vr(u,v_0)\Big|_{u=u_0}
=\Big(\frac{\partial x}{\partial u}(u_0,v_0)\,,\,
      \frac{\partial y}{\partial u}(u_0,v_0)\,,\,
      \frac{\partial z}{\partial u}(u_0,v_0)\Big)
</mrow><mrow>
\vT_v &amp;= \frac{\partial\ }{\partial v}\vr(u_0,v)\Big|_{v=v_0}
=\Big(\frac{\partial x}{\partial v}(u_0,v_0)\,,\,
      \frac{\partial y}{\partial v}(u_0,v_0)\,,\,
      \frac{\partial z}{\partial v}(u_0,v_0)\Big)
</mrow>
</md>
Then
<md>
<mrow>
\vn = \vT_u\times\vT_v
=\det\left|\begin{matrix}
            \hi &amp;  \hj &amp; \hk \\
            \frac{\partial x}{\partial u}(u_0,v_0) &amp;
                     \frac{\partial y}{\partial u}(u_0,v_0) &amp;
                     \frac{\partial z}{\partial u}(u_0,v_0) \\
           \frac{\partial x}{\partial v}(u_0,v_0) &amp;
                     \frac{\partial y}{\partial v}(u_0,v_0) &amp;
                     \frac{\partial z}{\partial v}(u_0,v_0)
           \end{matrix}\right|
</mrow>
</md>
is normal (i.e. perpendicular) to the surface at <m>(x_0,y_0,z_0)</m>.
</li>
<li>
Let <m>(x_0,y_0,z_0)=f(x_0,y_0)</m> be a point on the surface <m>z=f(x,y)</m>. Then,
<md>
<mrow>
\vn =-f_x(x_0,y_0)\,\hi - f_y(x_0,y_0)\,\hj + \hk
</mrow>
</md>
is normal to the surface at <m>(x_0,y_0,z_0)</m>.
</li>
<li>
Consider the surface given implicitly by the equation <m>G(x,y,z) = K</m>,
where <m>K</m> is a constant. Let <m>(x_0,y_0,z_0)</m> be a point on the surface and assume that the gradient <m>\vnabla G\big(x_0,y_0,z_0\big)\ne \vZero</m>. Then
<md>
<mrow>
\vn= \vnabla G\big(x_0,y_0,z_0\big)
</mrow>
</md>
is normal to the surface at <m>(x_0,y_0,z_0)</m>.
</li>
</ol>
</p>

<p>Note that none of the normal vectors <m>\vn</m> above need be of unit length.
</p></statement>
</theorem>

<p>
Note that if we apply part (c) to <m>G(x,y,z) = z - f(x,y)</m> we get
the normal vector <m>\vn=\vnabla G\big(x_0,y_0,z_0\big)
   =-f_x(x_0,y_0)\,\hi - f_y(x_0,y_0)\,\hj + \hk</m>, which is the same as the
normal vector provided by part (b). Of course they had to be at least
parallel.
</p>

<proof>
<p> (a)
First fix <m>v=v_0</m> and let <m>u</m> vary. Then
<me>
u\mapsto \vr(u,v_0) = \big(x(u,v_0)\,,\,y(u,v_0)\,,\,z(u,v_0)\big)
</me>
is a curve on the surface (the red curve in the figure on the right below) that
passes through <m>(x_0,y_0,z_0)</m> (the black dot in the figure) when <m>u=u_0</m>.
</p>

<sidebyside widths="48% 48%">
<image source="figs/surfaceSlice"/>
<image source="figs/saddleA"/>
</sidebyside>

<p>
The tangent vector to this curve at  <m>(x_0,y_0,z_0)</m>,
which is also a tangent vector to the surface at <m>(x_0,y_0,z_0)</m>,
is
<me>
\vT_u = \frac{\partial\ }{\partial u}\vr(u,v_0)\Big|_{u=u_0}
=\Big(\frac{\partial x}{\partial u}(u_0,v_0)\,,\,
      \frac{\partial y}{\partial u}(u_0,v_0)\,,\,
      \frac{\partial z}{\partial u}(u_0,v_0)\Big)
</me>
It is the red arrow in the figure on the right above.
</p>

<p>Next fix <m>u=u_0</m> and let <m>v</m> vary. Then
<me>
v\mapsto \vr(u_0,v) = \big(x(u_0,v)\,,\,y(u_0,v)\,,\,z(u_0,v)\big)
</me>
is a curve on the surface (the blue curve in the figure on the right above)
that passes through <m>(x_0,y_0,z_0)</m> when <m>v=v_0</m>.
The tangent vector to this curve at  <m>(x_0,y_0,z_0)</m>,
which is also a tangent vector to the surface at <m>(x_0,y_0,z_0)</m>,
is
<me>
\vT_v = \frac{\partial\ }{\partial v}\vr(u_0,v)\Big|_{v=v_0}
=\Big(\frac{\partial x}{\partial v}(u_0,v_0)\,,\,
      \frac{\partial y}{\partial v}(u_0,v_0)\,,\,
      \frac{\partial z}{\partial v}(u_0,v_0)\Big)
</me>
It is the blue arrow in the figure on the right above.
</p>

<p>We now have two vectors, namely <m>\vT_u</m> and <m>\vT_v</m>, that are tangent
to the surface at <m>(x_0,y_0,z_0)</m>. So their cross product
<md>
<mrow>
\vn = \vT_u\times\vT_v
=\det\left|\begin{matrix}
            \hi &amp;  \hj &amp; \hk \\
            \frac{\partial x}{\partial u}(u_0,v_0) &amp;
                     \frac{\partial y}{\partial u}(u_0,v_0) &amp;
                     \frac{\partial z}{\partial u}(u_0,v_0) \\
           \frac{\partial x}{\partial v}(u_0,v_0) &amp;
                     \frac{\partial y}{\partial v}(u_0,v_0) &amp;
                     \frac{\partial z}{\partial v}(u_0,v_0)
           \end{matrix}\right|
</mrow>
</md>
is normal (i.e. perpendicular) to the surface at <m>(x_0,y_0,z_0)</m>.
Note however that this vector need not be normalized. That is, it need not
be of unit length.
</p>

<p>(b)
Next assume that the surface is given by the equation
<m>z=f(x,y)</m>. Then, renaming <m>u</m> to <m>x</m> and <m>v</m> to <m>y</m>, we may reuse part (a):
<me>
\vr(x,y) = \big(x,y, f(x,y)\big)
</me>
parametrizes the surface and, at <m>\big(x_0,y_0,z_0\big)=f(x_0,y_0)\big)</m>,
<md>
<mrow>
\vT_x &amp;= \frac{\partial\vr }{\partial x}(x_0,y_0)
=\big(1\,,\,
      0\,,\,
      f_x(x_0,y_0)\big)
</mrow><mrow>
\vT_y &amp;= \frac{\partial\vr }{\partial y}(x_0,y_0)
=\big(0\,,\,
      1\,,\,
      f_y(x_0,y_0)\big)
</mrow>
</md>
and
<md>
<mrow>
\vn &amp;= \vT_x\times\vT_y
=\det\left|\begin{matrix}
            \hi &amp;  \hj &amp; \hk \\
            1 &amp; 0 &amp; f_x(x_0,y_0) \\
            0 &amp; 1 &amp; f_y(x_0,y_0)
           \end{matrix}\right|
=-f_x(x_0,y_0)\,\hi - f_y(x_0,y_0)\,\hj + \hk
</mrow>
</md>
</p>

<p> (c)
Finally assume that the surface is given implicitly by the equation
<m>G(x,y,z)=0</m> or, more generally by the equation, <m>G(x,y,z) = K</m>, where <m>K</m> is
a constant. If <m>\vr(t)=\big(x(t)\,\,y(t)\,,\,z(t)\big)</m> is any curve
with <m>\vr(0) = (x_0,y_0,z_0)</m> that lies on the surface, then
<md alignment="alignat">
<mrow>
&amp; &amp; G\big(\vr(t)\big)&amp;=K &amp;\qquad &amp;\text{for all } t
</mrow><mrow>
&amp;\implies &amp; \diff{\ }{t} G\big(x(t),y(t),z(t)\big)&amp;=0 &amp; &amp;\text{for all } t
</mrow>
</md>
Applying the chain rule gives
<md>
<mrow>
\frac{\partial G}{\partial x}\big(x(t),y(t),z(t)\big)\diff{x}{t}(t)
&amp;+\frac{\partial G}{\partial y}\big(x(t),y(t),z(t)\big)\diff{y}{t}(t)
</mrow><mrow>
&amp;+\frac{\partial G}{\partial z}\big(x(t),y(t),z(t)\big)\diff{z}{t}(t)
=0
</mrow>
</md>
The left hand side is exactly the dot product
of <m>\big(\frac{\partial G}{\partial x}
\,,\,\frac{\partial G}{\partial y}
\,,\,\frac{\partial G}{\partial z}\big)=\vnabla G</m>
with
<m>\big(\diff{x}{t}
\,,\,\diff{y}{t}
\,,\,\diff{z}{t}\big)
=\diff{\vr}{t}</m>, so that
<md>
<mrow>
\vnabla G\big(\vr(t)\big)\cdot\vr'(t)&amp;=0 \qquad
          \text{for all } t
</mrow><mrow>
\implies  \vnabla G\big(x_0,y_0,z_0\big)\cdot\vr'(0)&amp;=0 &amp;
</mrow>
</md>
This tell us that <m>\vnabla G\big(x_0,y_0,z_0\big)</m> is perpendicular
to <m>\vr'(0)</m>, which is a tangent vector to <m>G=K</m> at <m>(x_0,y_0,z_0)</m>.
This is true for all curves <m>\vr(t)</m> on <m>G=K</m> and so is true
for all tangent vectors to <m>G=K</m> at <m>(x_0,y_0,z_0)</m>.
So <m>\vnabla G\big(x_0,y_0,z_0\big)</m> is a normal vector to <m>G(x,y,z)=K</m>
at <m>(x_0,y_0,z_0)</m>.
</p>

</proof>

<example xml:id="eg_tangentPlaneA">
<p>
Consider the surface
<md>
<mrow>
x &amp;= x(u,v) = u\cos v
</mrow><mrow>
y &amp;=y(u,v) = u\sin v
</mrow><mrow>
z &amp;=z(u,v) = u
</mrow>
</md>
Observe that
<me>
x(u,v)^2 + y(u,v)^2 = u^2 = z(u,v)^2
</me>
So our surface is also
<me>
G(x,y,z) = x^2+y^2-z^2 = 0
</me>
We shall sketch it shortly. But first, let's find it's tangent plane
at <m>(x_0,y_0,z_0)=\vr(u_0,v_0)</m>.
In fact, let's do it twice. Once using the parametrization and once using its
implicit equation. First, using the parametrization
<m>\vr(u,v) = u\cos v\,\hi + u\sin v\,\hj + u\,\hk</m>, we have
<md>
<mrow>
\vT_u &amp;= \frac{\partial\vr}{\partial u}(u_0,v_0)
       =  \cos v_0\,\hi + \sin v_0\,\hj + \hk
</mrow><mrow>
\vT_v &amp;= \frac{\partial\vr}{\partial v}(u_0,v_0)
       =  -u_0\sin v_0\,\hi + u_0\cos v_0\,\hj
</mrow>
</md>
so that
<md>
<mrow>
\vn &amp;= \big(\cos v_0\,\hi + \sin v_0\,\hj + \hk\big)\times
      \big(-u_0\sin v_0\,\hi + u_0\cos v_0\,\hj\big)
</mrow><mrow>
    &amp;= \big(-u_0\cos v_0\,,\,-u_0\sin v_0\,,\, u_0)
      = (-x_0,-y_0,z_0)
</mrow>
</md>
Next using the implicit equation <m>G(x,y,z) = x^2+y^2-z^2=0</m>, we have
the normal vector
<me>
\vnabla G\big(x_0,y_0,z_0\big) = (2x_0,2y_0,-2z_0) =-2(-x_0,-y_0,z_0)
</me>
Of course the two vectors <m>(-x_0,-y_0,z_0)</m> and <m>-2(-x_0,-y_0,z_0)</m>
are parallel to each other. Either can be used as a normal vector and
the tangent plane to <m>x^2+y^2-z^2=0</m> at <m>(x_0,y_0,z_0)</m> is
<me>
0=\vn\cdot(x-x_0,y-y_0,z-z_0)
 = -x_0(x-x_0)-y_0(y-y_0) + z_0(z-z_0)
</me>
<em>provided</em> <m>(x_0,y_0,z_0)\ne \vZero</m>. In the event that
<m>(x_0,y_0,z_0) = \vZero</m> the <q>tangent plane equation</q> reduces to <m>0=0</m>
and there is clearly a problem.
</p>

<p>More generally, if
<m>\vT_u\times\vT_v=\vZero</m> (or <m>\vnabla G(x_0,y_0,z_0)=\vZero</m>), then
either<fn>We saw the same dichotomy when considering what happened
for a curve when <m>\vr'(t)=0</m>. See Example <xref ref="eg_zeroSpeed"/>.
</fn>
<ul>
<li>
the surface fails to have a tangent plane at <m>(x_0,y_0,z_0)</m>, or
</li>
<li>
our parametrization is screwy<fn>Of course <q>screwy</q> is not a mathematically precise word. One way a parametrization
<m>\vr(u,v)</m> could be <q>screwy</q> is if it failed to give a
one-to-one correspondence between parameter values <m>(u,v)</m> and points
on (part of) the surface. For example, polar coordinates
<m>\vr(u,v) = u\cos v\,\hi + u\sin v\,\hj</m> give <m>\vr(0,v)=(0,0)</m> for all
values of <m>v</m>.
</fn> there. For example, we can parametrize the
<m>xy</m>-plane, <m>z=0</m>, by <m>\vr(u,v) = u\cos v\,\hi + u\sin v\,\hj</m>. (This is just
polar coordinates.) Then
<m>\vT_u =  \cos v_0\,\hi + \sin v_0\,\hj </m> and
<m>\vT_v =  -u_0\sin v_0\,\hi + u_0\cos v_0\,\hj</m>, so that
<m>\vT_u\times\vT_v = u_0\hk</m> is <m>\vZero</m> when <m>u_0=0</m>. But the plane <m>z=0</m>
is its own tangent plane everywhere.
</li>
</ul>
The surface of current interest is <m>x^2+y^2=z^2</m>. The intersection of
this surface with the horizontal plane <m>z=z_0</m> is <m>x^2+y^2=z_0^2</m>, which is
the circle of radius <m>|z_0|</m> centred on <m>x=y=0</m>. So our surface is a stack of
circles. The radius of the circle in the <m>xy</m>-plane is zero. The radius
increases linearly as we move away from the <m>xy</m>-plane. Our surface
is a cone. It does not have a tangent plane at <m>(0,0,0)</m>.
</p>

<sidebyside width="16%">
<image source="figs/cone"/>
</sidebyside>

</example>


<example xml:id="eg_tangentPlaneB">
<p>
This time we shall find the tangent planes to the surface
<me>
x^2 + y^2 -z^2 = 1
</me>
As for the cone of the last example, the intersection of
this surface with the horizontal plane <m>z=z_0</m> is a circle <mdash/>
the circle of radius <m>\sqrt{1+z_0^2}</m>  centred on <m>x=y=0</m>.
Our surface is again a stack of circles. The radius of the circle
in the <m>xy</m>-plane is <m>1</m>. The radius increases as we move away from the <m>xy</m>-plane. Here is a sketch of the surface.
</p>

<sidebyside width="25%">
<image source="figs/hyperboloid1"/>
</sidebyside>

<p>
It is called a hyperboloid<fn>There are also hyperboloids of two sheets. See Appendix <xref ref="app_quadric"/>.
</fn> of one sheet.
</p>

<p>
Using the implicit equation <m>G(x,y,z) = x^2+y^2-z^2=1</m>, we have
<me>
\vnabla G\big(x_0,y_0,z_0\big) = (2x_0,2y_0,-2z_0) =2(x_0,y_0,-z_0)
</me>
and we may take <m>(x_0,y_0,-z_0)</m> as a normal vector at <m>(x_0,y_0,z_0)</m>.
So the tangent plane to <m>x^2+y^2-z^2=1</m> at <m>(x_0,y_0,z_0)</m> is
<me>
0=\vn\cdot(x-x_0,y-y_0,z-z_0)
 = x_0(x-x_0)+y_0(y-y_0) - z_0(z-z_0)
</me>
This time <m>\vn=(x_0,y_0,-z_0)\ne \vZero</m>, so that we have a tangent plane, at
every point of the surface. In particular, the vanishing of
<m>\vn=(x_0,y_0,-z_0)</m> at <m>(x_0,y_0,z_0)=(0,0,0)</m> is not a problem because
<m>(0,0,0)</m> is not on the surface.
</p>

</example>

<example xml:id="eg_tangentPlaneBB">
<title>Optional <mdash/> Parametrizing the Hyperboloid of One Sheet</title>


<p>The hyperboloid of one sheet, <m>x^2+y^2-z^2=1</m>, has a symmetry. It is
invariant under rotation about the <m>z</m>-axis.
So it is natural to parametrize the surface using cylindrical coordinates.
</p>

<sidebyside widths="45% 30%" valign="middle">
<p><md>
<mrow>
x &amp;= r\cos\theta
</mrow><mrow>
y &amp;= r\sin\theta
</mrow><mrow>
z &amp;= z
</mrow>
</md></p>
<image source="figs/cylindrical"/>
</sidebyside>

<p>
In cylindrical coordinates the surface <m>x^2+y^2-z^2=1</m> is <m>r^2-z^2=1</m>,
and we could parametrize it by
  <m>\vr(\theta,z) = \sqrt{1+z^2}\,\cos\theta\,\hi +\sqrt{1+z^2}\,\sin\theta\,\hj
      +z\,\hk</m>. Alternatively, we can eliminate the square roots in the
parametrization by exploiting the hyperbolic trig functions
<me>
\sinh u = \frac{1}{2}\big(e^u-e^{-u}\big) \qquad
\cosh u = \frac{1}{2}\big(e^u+e^{-u}\big)
</me>
The functions have properties<fn>
  This is no accident: <m>\cosh u = \cos(iu)</m> and <m>\sinh u = -i\sin(iu)</m>,
  where <m>i</m> is the usual complex number that obeys <m>i^2=-1</m>.  You can verify these formulae by just checking that <m>\cosh u</m> and <m>\cos(iu)</m> have the same Taylor expansions 
and that <m>\sinh u</m> and <m>-i\sin(iu)</m> have the same Taylor expansions.
</fn> that are very
similar to those of <m>\sin\theta</m> and <m>\cos\theta</m>.
<md>
<mrow>
\diff{}{u} \cosh u= \sinh u \qquad
\diff{}{u} \sinh u= \cosh u \qquad
\cosh^2 u -\sinh^2 u =1
</mrow>
</md>
We can set <m>r=\cosh u</m>, <m>z=\sinh u</m> to yield the parametrization
<md>
<mrow>
\vr(\theta,u) = \cosh u\,\cos\theta\,\hi +\cosh u\,\sin\theta\,\hj
      +\sinh u\,\hk
</mrow>
</md>
As an exercise in working with hyperbolic trig functions, we'll use this
parametrization to find <m>\hn</m>.
<md>
<mrow>
x&amp;=  \cosh u\,\cos\theta &amp;
x_u&amp;=  \sinh u\,\cos\theta &amp;
x_\theta&amp;=  -\cosh u\,\sin\theta

</mrow><mrow>

y&amp;= \cosh u\,\sin\theta &amp;
y_u&amp;= \sinh u\,\sin\theta &amp;
y_\theta&amp;= \phantom{-}\cosh u\,\cos\theta

</mrow><mrow>

z&amp;=\sinh u &amp;
z_u&amp;=\cosh u &amp;
z_\theta&amp;=0
</mrow>
</md>
So
<md>
<mrow>
\vn = \vT_u\times\vT_\theta
&amp;=\det\left|\begin{matrix}
            \hi &amp;  \hj &amp; \hk
            \\
            \sinh u\,\cos\theta &amp;
               \sinh u\,\sin\theta &amp;
               \cosh u
            \\
           -\cosh u\,\sin\theta  &amp;
            \cosh u\,\cos\theta &amp;
             0
           \end{matrix}\right|
</mrow><mrow>
&amp;=\big(-\cosh^2u\,\cos\theta\,,\,
       -\cosh^2u\,\sin\theta\,,\,
       \sinh u\cosh u\big)
</mrow>
</md>
</p></example>


<xi:include href="../problems/prob_s3.2.ptx" />

</section>
